First pass at modularizing grw.v

src/grw.v
@@ -9,2775 +9,2959 @@ Close Scope vector_scope.
 
 Require Import CrossCrypto.RewriteUtil.
 Require Import CrossCrypto.ListUtil.
+Require Import CrossCrypto.NatUtil.
 Require CrossCrypto.fmap.list_of_pairs.
 
-Local Existing Instance eq_subrelation | 5.
-
-Fixpoint optsub (n m : nat) {struct m} : option nat :=
-  match m with
-  | 0 => Some n
-  | S m => match n with
-           | 0 => None
-           | S n => optsub n m
-           end
-  end.
-
-Local Notation "a -? b" := (optsub a b) (left associativity, at level 50).
-
-Lemma optsub_plus a b :
-  match a -? b with
-  | Some c => a = b + c
-  | None => a < b
-  end.
-Proof.
-  revert a; induction b; intros a; cbn [optsub plus]; eauto.
-  destruct a; try omega.
-  specialize (IHb a).
-  destruct (a -? b); omega.
-Qed.
-
-Local Ltac destruct_decider k comparison lemma a b :=
-  pose proof (lemma a b); destruct (comparison a b);
+Ltac destruct_decider k comparison lemma a b :=
+  let H := fresh in
+  pose proof (lemma a b) as H; destruct (comparison a b);
   try k a;
-  try k b.
+  try k b;
+  let Ht := type of H in
+  try k Ht.
 
-Local Ltac crush_deciders_in x :=
+Ltac crush_deciders_in x :=
   lazymatch x with
-  | context[?a =? ?b] =>
-    destruct_decider crush_deciders_in Nat.eqb Nat.eqb_eq a b
+  | context[(@eqb ?T ?E ?a ?b)] =>
+    destruct_decider crush_deciders_in (@eqb T E) (@eqb_leibniz T E) a b
   | context[?a -? ?b] =>
     destruct_decider crush_deciders_in optsub optsub_plus a b
+  | context[?a =? ?b] =>
+    destruct_decider crush_deciders_in Nat.eqb Nat.eqb_eq a b
   | context[?a <=? ?b] =>
     destruct_decider crush_deciders_in Nat.leb Nat.leb_le a b
   | context[?a <? ?b] =>
     destruct_decider crush_deciders_in Nat.ltb Nat.ltb_lt a b
   end.
 
-Local Ltac crush_deciders t :=
+Ltac use_boolean_equalities :=
+  repeat match goal with
+         | H : true = true -> ?x |- _ => specialize (H eq_refl)
+         | H : _ -> true = true |- _ => clear H
+         | H : false = true -> _ |- _ => clear H
+         | H : ?x -> false = true |- _ =>
+           assert (~ x) by (let H' := fresh in
+                            intro H'; specialize (H H');
+                            congruence);
+           clear H
+         | H : _ = true <-> _ |- _ => destruct H
+         end.
+
+Ltac crush_deciders' t :=
   repeat (multimatch goal with
           | |- ?x => crush_deciders_in x
-          | H : ?x -> false = true |- _ =>
-            assert (~ x) by (let H' := fresh in
-                             intro H'; specialize (H H');
-                             congruence);
-            clear H
+          | _ => use_boolean_equalities
+          | _ => cbn [andb orb negb] in *
           | _ => intuition idtac
           | _ => congruence
           | _ => omega
           | _ => t
           end).
 
-Inductive type : Set :=
-| tunit : type
-| tnat : type
-| tbool : type
-| tprod : type -> type -> type.
+Tactic Notation "crush_deciders" tactic3(t) :=
+  crush_deciders' t.
 
-Lemma type_dec (t1 t2 : type) : {t1 = t2} + {t1 <> t2}.
-Proof. decide equality. Defined.
+Section Language.
+  Local Existing Instance eq_subrelation | 5.
 
-Fixpoint type_eqb (t1 t2 : type) : bool :=
-  match t1, t2 with
-  | tunit, tunit => true
-  | tnat, tnat => true
-  | tbool, tbool => true
-  | tprod t1a t1b, tprod t2a t2b => andb (type_eqb t1a t2a) (type_eqb t1b t2b)
-  | _, _ => false
-  end.
-Lemma type_eqb_eq t1 t2 : type_eqb t1 t2 = true <-> t1 = t2.
-Proof.
-  split.
-  - revert t2; induction t1; destruct t2; cbn [type_eqb];
-      intuition (try congruence).
-    rewrite andb_true_iff in *;
-      erewrite IHt1_1, IHt1_2; intuition eauto.
-  - intros; subst t2; induction t1; cbn [type_eqb]; try congruence.
-    rewrite andb_true_iff; intuition congruence.
-Qed.
+  Context {basetype : Set}
+          {basetype_eqdec : EqDec basetype}
+          {interp_basetype : basetype -> Set}
+          {interp_basetype_eqdec : forall b, EqDec (interp_basetype b)}
+          {interp_basetype_inhabited : forall {b}, interp_basetype b}
+          {basetype_transport :
+             forall {P : basetype -> Type} {a : basetype} (b : basetype),
+               P a -> option (P b)}
+          {basetype_transport_same :
+             forall {P b} (x : P b),
+               basetype_transport b x = Some x}
+          {basetype_transport_different :
+             forall {P b u} (x : P b),
+               u <> b -> basetype_transport u x = None}.
+  Arguments interp_basetype_inhabited {b}.
+  Arguments basetype_transport {P a}.
+  Arguments basetype_transport_same {P b}.
+  Arguments basetype_transport_different {P b u}.
 
-Bind Scope etype_scope with type.
-Delimit Scope etype_scope with etype.
-Local Notation "A * B" := (tprod A%etype B%etype) : etype_scope.
+  Inductive type : Set :=
+  | tbase : basetype -> type
+  | tunit : type
+  | tprod : type -> type -> type.
 
-Fixpoint interp_type (t : type) : Set :=
-  match t with
-  | tunit => unit
-  | tnat => nat
-  | tbool => bool
-  | tprod t1 t2 => interp_type t1 * interp_type t2
-  end.
+  Bind Scope etype_scope with type.
+  Delimit Scope etype_scope with etype.
+  Local Notation "A * B" := (tprod A%etype B%etype) : etype_scope.
 
-Lemma interp_type_dec {t} (x1 x2 : interp_type t) : {x1 = x2} + {x1 <> x2}.
-Proof. induction t; decide equality. Defined.
+  Fixpoint type_eqb (t1 t2 : type) : bool :=
+    match t1, t2 with
+    | tbase b1, tbase b2 => b1 ?= b2
+    | tunit, tunit => true
+    | tprod t1a t1b, tprod t2a t2b =>
+      (type_eqb t1a t2a) && (type_eqb t1b t2b)
+    | _, _ => false
+    end.
+  Lemma type_eqb_eq t1 t2 : type_eqb t1 t2 = true <-> t1 = t2.
+  Proof.
+    revert t2; induction t1; intros []; cbn [type_eqb];
+      crush_deciders rewrite ?andb_true_iff, ?IHt1_1, ?IHt1_2 in *.
+  Qed.
+  Local Instance type_eqdec : EqDec type := Build_EqDec type_eqb type_eqb_eq.
+  Lemma type_eq_or (t1 t2 : type) : t1 = t2 \/ t1 <> t2.
+  Proof. destruct (EqDec_dec _ t1 t2); eauto. Qed.
 
-(* necessary for ret *)
-Local Instance interp_type_eqdec {t} : EqDec (interp_type t).
-Proof. induction t; typeclasses eauto. Defined.
-
-Ltac type_head x :=
-  match x with
-  | tunit => idtac
-  | tnat => idtac
-  | tbool => idtac
-  | tprod _ _ => idtac
-  end.
-
-Fixpoint type_inhabited {t : type} : interp_type t :=
-  match t with
-  | tunit => tt
-  | tbool => false
-  | tnat => 0%nat
-  | tprod t1 t2 => (type_inhabited, type_inhabited)
-  end.
-
-Definition M t := Comp (interp_type t).
-Definition Mret {t : type} : interp_type t -> M t :=
-  Ret (EqDec_dec interp_type_eqdec).
-Definition Mbind {t1 t2 : type} :
-  M t1 ->
-  (interp_type t1 -> M t2) -> M t2 :=
-  @Bind _ _.
-Definition Mequiv {t} : M t -> M t -> Prop := Comp_eq.
-
-Inductive const : Type :=
-| coin.
-
-Lemma const_dec (c1 c2 : const) : {c1 = c2} + {c1 <> c2}.
-Proof. decide equality. Defined.
-
-Definition const_eqb (c1 c2 : const) : bool :=
-  match c1, c2 with
-  | coin, coin => true
-  end.
-Lemma const_eqb_eq (c1 c2 : const) : const_eqb c1 c2 = true <-> c1 = c2.
-Proof. destruct c1, c2; intuition eauto. Qed.
-
-Definition cdom c : type :=
-  match c with
-  | coin => tunit
-  end.
-
-Definition ccod c : type :=
-  match c with
-  | coin => tbool
-  end.
-
-Definition interp_const c : interp_type (cdom c) -> M (ccod c) :=
-  match c with
-  | coin => fun _ => x <-$ Rnd 1; ret (Vector.nth x Fin.F1)
-  end.
-
-Inductive ret_const : Type :=
-| xor'
-| zero
-| id (t : type).
-
-Lemma retconst_dec (c1 c2 : ret_const) : {c1 = c2} + {c1 <> c2}.
-Proof. repeat decide equality. Defined.
-
-Definition retconst_eqb (c c' : ret_const) : bool :=
-  match c, c' with
-  | xor', xor' => true
-  | zero, zero => true
-  | id t1, id t2 => type_eqb t1 t2
-  | _, _ => false
-  end.
-Lemma retconst_eqb_eq c1 c2 : retconst_eqb c1 c2 = true <-> c1 = c2.
-Proof.
-  destruct c1, c2; cbv [retconst_eqb]; rewrite ?type_eqb_eq;
-    intuition congruence.
-Qed.
-
-Definition rcdom c : type :=
-  match c with
-  | xor' => tbool * tbool
-  | zero => tunit
-  | id t => t
-  end.
-
-Definition rccod c : type :=
-  match c with
-  | xor' => tbool
-  | zero => tbool
-  | id t => t
-  end.
-
-Definition interp_retconst c :
-  interp_type (rcdom c) -> interp_type (rccod c) :=
-  match c with
-  | xor' => fun '(x, y) => xorb x y
-  | zero => fun _ => false
-  | id _ => fun x => x
-  end.
-
-(* De bruijn indices which can be paired together to get a tuple *)
-Inductive ref : Type :=
-| ref_index : nat -> ref
-| ref_pair : ref -> ref -> ref.
-
-Fixpoint ref_eqb (r r' : ref) : bool :=
-  match r, r' with
-  | ref_index i, ref_index i' => i =? i'
-  | ref_pair r1 r2, ref_pair r1' r2' => ref_eqb r1 r1' && ref_eqb r2 r2'
-  | _, _ => false
-  end.
-
-Lemma ref_eqb_eq r r' : ref_eqb r r' = true <-> r = r'.
-Proof.
-  revert r'; induction r; destruct r'; cbn [ref_eqb];
-    let t := (rewrite ?IHr1, ?IHr2, ?andb_true_iff, ?Nat.eqb_eq in * ) in
-    repeat (intuition idtac; t); congruence.
-Qed.
-
-Inductive operation : Type :=
-| op_unit : operation
-| op_app (c : const) : ref -> operation
-| op_retapp (c : ret_const) : ref -> operation.
-
-Lemma op_dec (o1 o2 : operation) : {o1 = o2} + {o1 <> o2}.
-Proof. repeat decide equality; congruence. Defined.
-
-Definition op_eqb (o o' : operation) : bool :=
-  match o, o' with
-  | op_unit, op_unit => true
-  | op_app c r, op_app c' r' => const_eqb c c' && ref_eqb r r'
-  | op_retapp c r, op_retapp c' r' => retconst_eqb c c' && ref_eqb r r'
-  | _, _ => false
-  end.
-
-Lemma op_eqb_eq o o' : op_eqb o o' = true <-> o = o'.
-Proof.
-  destruct o, o'; cbn [op_eqb];
-    rewrite ?andb_true_iff, ?const_eqb_eq, ?retconst_eqb_eq,
-    ?ref_eqb_eq in *; intuition congruence.
-Qed.
-
-Definition op_type o : type :=
-  match o with
-  | op_unit => tunit
-  | op_app c _ => ccod c
-  | op_retapp c _ => rccod c
-  end.
-
-Definition transport {P : type -> Type} {a : type} (b : type) (p : P a)
-  : option (P b).
-  destruct (type_dec a b).
-  - subst; exact (Some p).
-  - exact None.
-Defined.
-
-Fixpoint lookup (ctxt : type) (ctx : interp_type ctxt)
-         (n : nat) (t : type) {struct n} : option (interp_type t).
-  destruct ctxt; [exact None .. |].
-  refine match n, ctx with
-         | 0, (x, _) => transport t x
-         | S n, (_, ctx) => lookup ctxt2 ctx n t
-         end.
-Defined.
-
-Fixpoint lookup_ref ctxt ctx (r : ref) (t : type) {struct r}
-  : option (interp_type t) :=
-  match r with
-  | ref_index n => lookup ctxt ctx n t
-  | ref_pair r1 r2 =>
+  Fixpoint interp_type (t : type) : Set :=
     match t with
-    | (t1 * t2)%etype =>
-      match lookup_ref ctxt ctx r1 t1, lookup_ref ctxt ctx r2 t2 with
-      | Some x, Some y => Some (x, y)
-      | _, _ => None
-      end
-    | _ => None
-    end
-  end.
+    | tbase b => interp_basetype b
+    | tunit => unit
+    | tprod t1 t2 => interp_type t1 * interp_type t2
+    end.
 
-Definition interp_op ctxt ctx o : option (M (op_type o)) :=
-  match o with
-  | op_unit => Some (@Mret tunit tt)
-  | op_app c r => match lookup_ref ctxt ctx r (cdom c) with
+  Fixpoint interp_type_eqb {t} (x y : interp_type t) : bool :=
+    match t return interp_type t -> interp_type t -> bool with
+    | tbase b => fun x y => x ?= y
+    | tunit => fun _ _ => true
+    | tprod t1 t2 => fun x y =>
+                       match x, y with
+                       | (x1, x2), (y1, y2) =>
+                         interp_type_eqb x1 y1 && interp_type_eqb x2 y2
+                       end
+    end x y.
+  Lemma interp_type_eqb_eq {t} (x y : interp_type t) :
+    interp_type_eqb x y = true <-> x = y.
+  Proof.
+    induction t; cbn [interp_type interp_type_eqb] in *;
+      try solve [crush_deciders idtac];
+      destruct x, y; rewrite ?andb_true_iff, ?IHt1, ?IHt2;
+        intuition congruence.
+  Qed.
+  Definition interp_type_eqdec {t} : EqDec (interp_type t) :=
+    Build_EqDec interp_type_eqb interp_type_eqb_eq.
+
+  Fixpoint interp_type_inhabited {t : type} : interp_type t :=
+    match t with
+    | tbase _ => interp_basetype_inhabited
+    | tunit => tt
+    | tprod t1 t2 => (interp_type_inhabited, interp_type_inhabited)
+    end.
+
+  Context {M : type -> Type}
+          {Mret : forall {t}, interp_type t -> M t}
+          {Mbind : forall {t1 t2}, M t1 -> (interp_type t1 -> M t2) -> M t2}
+          {Mequiv : forall {t}, M t -> M t -> Prop}
+          {Mequiv_equiv : forall {t}, Equivalence (@Mequiv t)}
+          {Proper_Mbind :
+             forall {t1 t2},
+               Proper
+                 (Mequiv ==> (pointwise_relation _ Mequiv) ==>Mequiv)
+                 (@Mbind t1 t2)}
+          {Mbind_assoc :
+             forall {t1 t2 t3}
+                    (f : M t1)
+                    (g : interp_type t1 -> M t2)
+                    (h : interp_type t2 -> M t3),
+               Mequiv (Mbind (Mbind f g) h)
+                      (Mbind f (fun x => Mbind (g x) h))}
+          {Mbind_Mret_l :
+             forall {t1 t2} x (f : interp_type t1 -> M t2),
+               Mequiv (Mbind (Mret x) f) (f x)}
+          {Mbind_Mret_r :
+             forall {t} (x : M t),
+               Mequiv (Mbind x Mret) x}
+          {Mbind_comm :
+             forall {t1 t2 t3}
+                    (c1 : M t1) (c2 : M t2)
+                    (c3 : interp_type t1 -> interp_type t2 -> M t3),
+               Mequiv (Mbind c1 (fun a => Mbind c2 (fun b => c3 a b)))
+                      (Mbind c2 (fun b => Mbind c1 (fun a => c3 a b)))}.
+  Arguments Mret {t}.
+  Arguments Mbind {t1 t2}.
+  Arguments Mequiv {t}.
+  Arguments Mequiv_equiv {t}.
+  Arguments Proper_Mbind {t1 t2}.
+  Arguments Mbind_assoc {t1 t2 t3}.
+  Arguments Mbind_Mret_l {t1 t2}.
+  Arguments Mbind_Mret_r {t}.
+  Arguments Mbind_comm {t1 t2 t3}.
+
+  Local Create HintDb mbind discriminated.
+  Hint Rewrite
+       @Mbind_assoc
+       @Mbind_Mret_l
+       @Mbind_Mret_r
+    : mbind.
+
+  Ltac step_Mequiv :=
+    repeat multimatch goal with
+           | |- Mequiv (Mbind _ _) (Mbind _ _) =>
+             eapply Proper_Mbind; [try reflexivity | intros ?]
+           | |- Mequiv ?x ?y => change x with y; reflexivity
+           | |- _ => autorewrite with mbind
+           end.
+
+  Context {const : Set}
+          {const_eqdec : EqDec const}
+          {cdom ccod : const -> type}
+          {interp_const : forall c, interp_type (cdom c) -> M (ccod c)}
+          {retconst : Set}
+          {retconst_eqdec : EqDec retconst}
+          {rcdom rccod : retconst -> type}
+          {interp_retconst : forall c,
+              interp_type (rcdom c) -> interp_type (rccod c)}.
+
+  (* De bruijn indices which can be paired together to get a tuple *)
+  Inductive ref : Type :=
+  | ref_index : nat -> ref
+  | ref_pair : ref -> ref -> ref.
+
+  Fixpoint ref_eqb (r r' : ref) : bool :=
+    match r, r' with
+    | ref_index i, ref_index i' => i =? i'
+    | ref_pair r1 r2, ref_pair r1' r2' => ref_eqb r1 r1' && ref_eqb r2 r2'
+    | _, _ => false
+    end.
+  Lemma ref_eqb_eq r r' : ref_eqb r r' = true <-> r = r'.
+  Proof.
+    revert r'; induction r; destruct r'; cbn [ref_eqb];
+      let t := (rewrite ?IHr1, ?IHr2, ?andb_true_iff, ?Nat.eqb_eq in * ) in
+      repeat (intuition idtac; t); congruence.
+  Qed.
+  Local Instance ref_eqdec : EqDec ref := Build_EqDec ref_eqb ref_eqb_eq.
+
+  Inductive op : Type :=
+  | op_unit : op
+  | op_app (c : const) : ref -> op
+  | op_retapp (c : retconst) : ref -> op.
+
+  Definition op_eqb (o o' : op) : bool :=
+    match o, o' with
+    | op_unit, op_unit => true
+    | op_app c r, op_app c' r'
+    | op_retapp c r, op_retapp c' r' => (c ?= c') && (r ?= r')
+    | _, _ => false
+    end.
+  Lemma op_eqb_eq o o' : op_eqb o o' = true <-> o = o'.
+  Proof. destruct o, o'; cbn [op_eqb]; crush_deciders idtac. Qed.
+  Local Instance op_eqdec : EqDec op := Build_EqDec op_eqb op_eqb_eq.
+
+  Definition op_type o : type :=
+    match o with
+    | op_unit => tunit
+    | op_app c _ => ccod c
+    | op_retapp c _ => rccod c
+    end.
+
+  Fixpoint transport {P : type -> Type} {a : type} (b : type) :
+    P a -> option (P b) :=
+    match a, b with
+    | tbase a, tbase b => @basetype_transport
+                            (fun bt => P (tbase bt))
+                            _ b
+    | tunit, tunit => Some
+    | tprod a1 a2, tprod b1 b2 =>
+      fun p =>
+        match @transport (fun t => P (t * a2)%etype) _ b1 p with
+        | Some p' => @transport (fun t => P (b1 * t)%etype) _ b2 p'
+        | None => None
+        end
+    | _, _ => fun _ => None
+    end.
+
+  Fixpoint lookup (ctxt : type) (ctx : interp_type ctxt)
+           (n : nat) (t : type) {struct n} : option (interp_type t) :=
+    match ctxt return interp_type ctxt -> _ with
+    | (_ * _)%etype =>
+      fun ctx =>
+        match n, ctx with
+        | 0, (x, _) => transport t x
+        | S n, (_, ctx) => lookup _ ctx n t
+        end
+    | _ => fun _ => None
+    end ctx.
+
+  Fixpoint lookup_ref ctxt ctx (r : ref) (t : type) {struct r}
+    : option (interp_type t) :=
+    match r with
+    | ref_index n => lookup ctxt ctx n t
+    | ref_pair r1 r2 =>
+      match t with
+      | (t1 * t2)%etype =>
+        match lookup_ref ctxt ctx r1 t1, lookup_ref ctxt ctx r2 t2 with
+        | Some x, Some y => Some (x, y)
+        | _, _ => None
+        end
+      | _ => None
+      end
+    end.
+
+  Definition interp_op ctxt ctx o : option (M (op_type o)) :=
+    match o with
+    | op_unit => Some (@Mret tunit tt)
+    | op_app c r => match lookup_ref ctxt ctx r (cdom c) with
                     | Some x => Some (interp_const c x)
                     | None => None
                     end
-  | op_retapp c r => match lookup_ref ctxt ctx r (rcdom c) with
+    | op_retapp c r => match lookup_ref ctxt ctx r (rcdom c) with
                        | Some x => Some (Mret (interp_retconst c x))
                        | None => None
                        end
-  end.
+    end.
 
-Definition cast {a : type} (b : type) (x : interp_type a) : interp_type b :=
-  match transport b x with
-  | Some x => x
-  | None => type_inhabited
-  end.
+  Definition cast {a : type} (b : type) (x : interp_type a) : interp_type b :=
+    match transport b x with
+    | Some x => x
+    | None => interp_type_inhabited
+    end.
 
-Lemma transport_same {P t} (x : P t) : transport t x = Some x.
-Proof.
-  cbv [transport eq_rect_r]; destruct (type_dec t t); try congruence.
-  cbv [eq_rect_r]. rewrite <-eq_rect_eq_dec; eauto using type_dec.
-Qed.
+  Lemma transport_same {P t} (x : P t) : transport t x = Some x.
+  Proof.
+    revert P x; induction t; intros P x; cbn [transport].
+    - eapply (@basetype_transport_same (fun b => P (tbase b))).
+    - eauto.
+    - rewrite IHt1, IHt2; eauto.
+  Qed.
 
-Lemma cast_same {t} (x : interp_type t) : cast t x = x.
-Proof. cbv [cast]; rewrite transport_same; eauto. Qed.
+  Lemma cast_same {t} (x : interp_type t) : cast t x = x.
+  Proof. cbv [cast]; rewrite transport_same; eauto. Qed.
 
-Lemma transport_different {P t u} (x : P t) : u <> t -> transport u x = None.
-Proof.
-  intros; cbv [transport eq_rect_r]; destruct (type_dec t u); congruence.
-Qed.
+  Lemma transport_different {P t u} (x : P t) : u <> t -> transport u x = None.
+  Proof.
+    revert P x u; induction t as [| |t1 ? t2 ?]; intros P x [| |u1 u2];
+      intros NE; cbn [transport];
+      try congruence.
+    - eapply (@basetype_transport_different (fun b => P (tbase b))).
+      congruence.
+    - destruct (type_eq_or t1 u1).
+      + destruct (type_eq_or t2 u2).
+        * congruence.
+        * destruct transport; eauto.
+          rewrite IHt2; eauto.
+      + rewrite IHt1; eauto.
+  Qed.
 
-Lemma cast_different {t u} (x : interp_type t) :
-  u <> t -> cast u x = type_inhabited.
-Proof. intros; cbv [cast]; rewrite transport_different; eauto. Qed.
+  Lemma cast_different {t u} (x : interp_type t) :
+    u <> t -> cast u x = interp_type_inhabited.
+  Proof. intros; cbv [cast]; rewrite transport_different; eauto. Qed.
 
-Definition interp_op_silent ctxt ctx o : M (op_type o) :=
-  match interp_op ctxt ctx o with
-  | Some m => m
-  | None => Mret type_inhabited
-  end.
+  Definition interp_op_silent ctxt ctx o : M (op_type o) :=
+    match interp_op ctxt ctx o with
+    | Some m => m
+    | None => Mret interp_type_inhabited
+    end.
 
-Definition expr : Type := (list operation) * operation.
+  Definition expr : Set := (list op) * op.
 
-Definition expr_type '((_, p2) : expr) : type := op_type p2.
+  Definition expr_type '((_, p2) : expr) : type := op_type p2.
 
-(* Interpreter in continuation-passing style. This has several
-   advantages over direct style:
-   - No need to rewrite Bind_Ret_l (very slowly!) on binds of the
-     contexts to get the correct form and to eliminate
-     lookups/transports
-   - Good commutation relation with List.app
-   - Can refer to universally-quantified variables as free de Bruijn indices
-*)
-Fixpoint interp_bindings (ctxt : type) (ctx : interp_type ctxt)
-         (p : list operation)
-         (tk : type) (k : forall ctxt : type, interp_type ctxt -> M tk)
-         {struct p} : (M tk) :=
-  match p with
-  | nil => k ctxt ctx
-  | cons o p =>
-    Mbind (interp_op_silent ctxt ctx o)
-          (fun x => interp_bindings (op_type o * ctxt) (x, ctx) p tk k)
-  end.
+  (* Interpreter in continuation-passing style. This has several
+   * advantages over direct style:
+   * - No need to rewrite Bind_Ret_l (very slowly!) on binds of the
+   *   contexts to get the correct form and to eliminate
+   *   lookups/transports
+   * - Good commutation relation with List.app
+   * - Can refer to universally-quantified variables as free de Bruijn indices
+   *)
+  Fixpoint interp_bindings (ctxt : type) (ctx : interp_type ctxt)
+           (p : list op)
+           (tk : type) (k : forall ctxt : type, interp_type ctxt -> M tk)
+           {struct p} : (M tk) :=
+    match p with
+    | nil => k ctxt ctx
+    | cons o p =>
+      Mbind (interp_op_silent ctxt ctx o)
+            (fun x => interp_bindings (op_type o * ctxt) (x, ctx) p tk k)
+    end.
 
-Definition interp_expr ctxt ctx e : M (expr_type e) :=
-  let '(p, o) := e in
-  interp_bindings ctxt ctx p (op_type o)
-                  (fun ctxt ctx => interp_op_silent ctxt ctx o).
+  Definition interp_expr ctxt ctx e : M (expr_type e) :=
+    let '(p, o) := e in
+    interp_bindings ctxt ctx p (op_type o)
+                    (fun ctxt ctx => interp_op_silent ctxt ctx o).
 
-Definition interp_expr_cast ctxt ctx e t : M t :=
-  Mbind (interp_expr ctxt ctx e)
-        (fun x => Mret (cast t x)).
+  Definition interp_expr_cast ctxt ctx e t : M t :=
+    Mbind (interp_expr ctxt ctx e)
+          (fun x => Mret (cast t x)).
 
-Lemma Mequiv_Mbind {t1 t2 : type}
-      (c1 c1' : M t1) (c2 c2' : interp_type t1 -> M t2) :
-  Mequiv c1 c1' ->
-  (forall x, Mequiv (c2 x) (c2' x)) ->
-  Mequiv (Mbind c1 c2) (Mbind c1' c2').
-Proof. cbv [Mequiv Mbind]; intros; eapply Proper_Bind; eauto. Qed.
+  Lemma Mequiv_Mbind_cast {t1 t1' t2} (c1 : M t1) (c1' : M t1')
+        (c2 c2' : forall t, interp_type t -> M t2) :
+    t1 = t1' ->
+    (forall t, Mequiv (Mbind c1 (fun x => Mret (cast t x)))
+                      (Mbind c1' (fun x => Mret (cast t x)))) ->
+    (forall t (x : interp_type t), Mequiv (c2 _ x) (c2' _ x)) ->
+    Mequiv (Mbind c1 (c2 _)) (Mbind c1' (c2' _)).
+  Proof.
+    intros ? Hc1 Hc2; subst t1'.
+    eapply Proper_Mbind; cbv [pointwise_relation]; eauto.
+    specialize (Hc1 t1).
+    setoid_rewrite cast_same in Hc1.
+    setoid_rewrite Mbind_Mret_r in Hc1.
+    eauto.
+  Qed.
 
-Lemma Mbind_assoc {t1 t2 t3} (f : M t1)
-      (g : interp_type t1 -> M t2) (h : interp_type t2 -> M t3) :
-  Mequiv (Mbind (Mbind f g) h)
-         (Mbind f (fun x => Mbind (g x) h)).
-Proof. setoid_rewrite <-Bind_assoc; reflexivity. Qed.
+  Lemma interp_expr_cast_expr_type ctxt ctx e :
+    Mequiv (interp_expr_cast ctxt ctx e (expr_type e))
+           (interp_expr ctxt ctx e).
+  Proof.
+    cbv [interp_expr_cast].
+    setoid_rewrite <-(Mbind_Mret_r (interp_expr ctxt ctx e)) at 2.
+    step_Mequiv.
+    rewrite cast_same; reflexivity.
+  Qed.
 
-Lemma Mbind_comm (t1 t2 t3 : type) (c1 : M t1) (c2 : M t2)
-      (c3 : interp_type t1 -> interp_type t2 -> M t3) :
-  Mequiv (Mbind c1 (fun a => Mbind c2 (fun b => c3 a b)))
-         (Mbind c2 (fun b => Mbind c1 (fun a => c3 a b))).
-Proof. eapply Bind_comm. Qed.
+  Definition equiv_under ctxt ctx e1 e2 :=
+    forall t, Mequiv (interp_expr_cast ctxt ctx e1 t)
+                     (interp_expr_cast ctxt ctx e2 t).
 
-Lemma Mbind_Mret_l {t1 t2} x (f : interp_type t1 -> M t2) :
-  Mequiv (Mbind (Mret x) f) (f x).
-Proof. eapply Bind_Ret_l. Qed.
+  Definition equiv e1 e2 := forall ctxt ctx, equiv_under ctxt ctx e1 e2.
 
-Lemma Mbind_Mret_r {t} (x : M t) : Mequiv (Mbind x Mret) x.
-Proof. eapply Bind_Ret_r. Qed.
+  Instance equiv_equiv : Equivalence equiv.
+  Proof.
+    split; cbv [equiv equiv_under Reflexive Symmetric Transitive];
+      [reflexivity|symmetry; eauto|etransitivity; eauto].
+  Qed.
 
-Lemma Mequiv_Mbind_cast {t1 t1' t2} (c1 : M t1) (c1' : M t1')
-      (c2 c2' : forall t, interp_type t -> M t2) :
-  t1 = t1' ->
-  (forall t, Mequiv (Mbind c1 (fun x => Mret (cast t x)))
-                    (Mbind c1' (fun x => Mret (cast t x)))) ->
-  (forall t (x : interp_type t), Mequiv (c2 _ x) (c2' _ x)) ->
-  Mequiv (Mbind c1 (c2 _)) (Mbind c1' (c2' _)).
-Proof.
-  intros ? Hc1 Hc2; subst t1'.
-  eapply Mequiv_Mbind; eauto.
-  specialize (Hc1 t1).
-  setoid_rewrite cast_same in Hc1.
-  setoid_rewrite Mbind_Mret_r in Hc1.
-  eauto.
-Qed.
+  Lemma interp_bindings_app ctxt (ctx : interp_type ctxt)
+        (p1 p2 : list op) tk (k : forall ctxt, interp_type ctxt -> M tk) :
+    Mequiv
+      (interp_bindings ctxt ctx (p1 ++ p2) tk k)
+      (interp_bindings ctxt ctx p1 tk
+                       (fun ctxt ctx => interp_bindings ctxt ctx p2 tk k)).
+  Proof.
+    revert ctxt ctx p2 tk k;
+      induction p1 as [|o p1]; intros ctxt ctx p2 tk k;
+        [reflexivity|].
+    cbn [interp_bindings app].
+    step_Mequiv; eauto.
+  Qed.
 
-Local Create HintDb mbind discriminated.
-Hint Rewrite
-     @Mbind_assoc
-     @Mbind_Mret_l
-     @Mbind_Mret_r
-  : mbind.
+  Lemma bind_interp_bindings ctxt ctx p tk k
+        tf (f : interp_type tk -> M tf) :
+    Mequiv (Mbind (interp_bindings ctxt ctx p tk k) f)
+           (interp_bindings ctxt ctx p tf (fun ctxt ctx =>
+                                             Mbind (k ctxt ctx) f)).
+  Proof.
+    revert ctxt ctx; induction p as [|o p]; intros ctxt ctx;
+      cbn [interp_bindings]; [reflexivity|].
+    step_Mequiv; eauto.
+  Qed.
 
-Ltac step_Mequiv :=
-  repeat multimatch goal with
-         | |- Mequiv (Mbind _ _) (Mbind _ _) =>
-           eapply Mequiv_Mbind; [try reflexivity | intros]
-         | |- Mequiv ?x ?y => change x with y; reflexivity
-         | |- _ => autorewrite with mbind
-         end.
+  Definition continuation_compat tk
+             (k k' : forall ctxt : type, interp_type ctxt -> M tk) : Prop :=
+    forall ctxt (ctx : interp_type ctxt),
+      Mequiv (k ctxt ctx) (k' ctxt ctx).
 
-Lemma interp_expr_cast_expr_type ctxt ctx e :
-  Mequiv (interp_expr_cast ctxt ctx e (expr_type e))
-         (interp_expr ctxt ctx e).
-Proof.
-  cbv [interp_expr_cast].
-  setoid_rewrite <-(Mbind_Mret_r (interp_expr ctxt ctx e)) at 2.
-  eapply Mequiv_Mbind; [reflexivity|intros].
-  rewrite cast_same; reflexivity.
-Qed.
+  Fixpoint renumber_ref (f : nat -> nat) (r : ref) : ref :=
+    match r with
+    | ref_index n => ref_index (f n)
+    | ref_pair r1 r2 => ref_pair (renumber_ref f r1) (renumber_ref f r2)
+    end.
 
-Definition equiv_under ctxt ctx e1 e2 :=
-  forall t, Mequiv (interp_expr_cast ctxt ctx e1 t)
-                   (interp_expr_cast ctxt ctx e2 t).
+  Definition renumber_op (f : nat -> nat) (o : op) : op :=
+    match o with
+    | op_unit => op_unit
+    | op_app c r => op_app c (renumber_ref f r)
+    | op_retapp c r => op_retapp c (renumber_ref f r)
+    end.
 
-Definition equiv e1 e2 := forall ctxt ctx, equiv_under ctxt ctx e1 e2.
+  Definition offset_renumbering (offset : nat)
+             (f : nat -> nat) (n : nat) : nat :=
+    match n -? offset with
+    | Some k => offset + (f k)
+    | None => n
+    end.
 
-Local Instance equiv_equiv : Equivalence equiv.
-Proof.
-  split; cbv [equiv equiv_under Reflexive Symmetric Transitive];
-    [reflexivity|symmetry; eauto|etransitivity; eauto].
-Qed.
+  Lemma offset_id k i :
+    offset_renumbering k (fun x => x) i = i.
+  Proof.
+    cbv [offset_renumbering].
+    crush_deciders idtac.
+  Qed.
 
-Lemma interp_bindings_app ctxt (ctx : interp_type ctxt)
-      (p1 p2 : list operation) tk (k : forall ctxt, interp_type ctxt -> M tk) :
-  Mequiv
-    (interp_bindings ctxt ctx (p1 ++ p2) tk k)
-    (interp_bindings ctxt ctx p1 tk
-                     (fun ctxt ctx => interp_bindings ctxt ctx p2 tk k)).
-Proof.
-  revert ctxt ctx p2 tk k;
-    induction p1 as [|o p1]; intros ctxt ctx p2 tk k;
-      [reflexivity|].
-  cbn [interp_bindings app].
-  step_Mequiv; eauto.
-Qed.
+  Fixpoint renumber_bindings (f : nat -> nat) (p : list op)
+    : list op :=
+    match p with
+    | nil => nil
+    | cons o p =>
+      cons (renumber_op f o)
+           (renumber_bindings (offset_renumbering 1 f) p)
+    end.
 
-Lemma bind_interp_bindings ctxt ctx p tk k
-      tf (f : interp_type tk -> M tf) :
-  Mequiv (Mbind (interp_bindings ctxt ctx p tk k) f)
-         (interp_bindings ctxt ctx p tf (fun ctxt ctx =>
-                                           Mbind (k ctxt ctx) f)).
-Proof.
-  revert ctxt ctx; induction p as [|o p]; intros ctxt ctx;
-    cbn [interp_bindings]; [reflexivity|].
-  step_Mequiv; eauto.
-Qed.
+  Fixpoint renumber_expr' acc f p o' :=
+    match p with
+    | nil => (rev acc, renumber_op f o')
+    | o :: p => renumber_expr' (renumber_op f o :: acc)
+                               (offset_renumbering 1 f) p o'
+    end.
 
-Definition continuation_compat tk
-           (k k' : forall ctxt : type, interp_type ctxt -> M tk) : Prop :=
-  forall ctxt (ctx : interp_type ctxt),
-    Mequiv (k ctxt ctx) (k' ctxt ctx).
+  Definition renumber_expr (f : nat -> nat) '((p, o') : expr) : expr :=
+    renumber_expr' nil f p o'.
 
-Fixpoint renumber_ref (f : nat -> nat) (r : ref) : ref :=
-  match r with
-  | ref_index n => ref_index (f n)
-  | ref_pair r1 r2 => ref_pair (renumber_ref f r1) (renumber_ref f r2)
-  end.
+  Fixpoint refs (r : ref) (n : nat) :=
+    match r with
+    | ref_index k => n = k
+    | ref_pair r1 r2 => refs r1 n \/ refs r2 n
+    end.
 
-Definition renumber_op (f : nat -> nat) (o : operation) : operation :=
-  match o with
-  | op_unit => op_unit
-  | op_app c r => op_app c (renumber_ref f r)
-  | op_retapp c r => op_retapp c (renumber_ref f r)
-  end.
+  Definition op_refs (o : op) (n : nat) :=
+    match o with
+    | op_unit => False
+    | op_app _ r | op_retapp _ r => refs r n
+    end.
 
-Definition offset_renumbering (offset : nat)
-           (f : nat -> nat) (n : nat) : nat :=
-  match n -? offset with
-  | Some k => offset + (f k)
-  | None => n
-  end.
+  Fixpoint bindings_ref (p : list op) (n : nat) :=
+    match p with
+    | nil => False
+    | o :: p => op_refs o n \/ bindings_ref p (S n)
+    end.
 
-Lemma offset_id k i :
-  offset_renumbering k (fun x => x) i = i.
-Proof.
-  cbv [offset_renumbering].
-  crush_deciders idtac.
-Qed.
+  Definition expr_refs '((p, o) : expr) (n : nat) :=
+    bindings_ref p n \/ op_refs o (length p + n).
 
-Fixpoint renumber_bindings (f : nat -> nat) (p : list operation)
-  : list operation :=
-  match p with
-  | nil => nil
-  | cons o p =>
-    cons (renumber_op f o)
-         (renumber_bindings (offset_renumbering 1 f) p)
-  end.
+  Fixpoint refsb (r : ref) (n : nat) :=
+    match r with
+    | ref_index k => n =? k
+    | ref_pair r1 r2 => refsb r1 n || refsb r2 n
+    end.
 
-Fixpoint renumber_expr' acc f p o' :=
-  match p with
-  | nil => (rev acc, renumber_op f o')
-  | o :: p => renumber_expr' (renumber_op f o :: acc)
-                             (offset_renumbering 1 f) p o'
-  end.
+  Definition op_refsb (o : op) (n : nat) :=
+    match o with
+    | op_unit => false
+    | op_app _ r | op_retapp _ r => refsb r n
+    end.
 
-Definition renumber_expr (f : nat -> nat) '((p, o') : expr) : expr :=
-  renumber_expr' nil f p o'.
+  Fixpoint bindings_refb (p : list op) (n : nat) :=
+    match p with
+    | nil => false
+    | o :: p => op_refsb o n || bindings_refb p (S n)
+    end.
 
-Fixpoint refs (r : ref) (n : nat) :=
-  match r with
-  | ref_index k => n = k
-  | ref_pair r1 r2 => refs r1 n \/ refs r2 n
-  end.
+  Definition expr_refsb '((p, o) : expr) (n : nat) :=
+    bindings_refb p n || op_refsb o (length p + n).
 
-Definition op_refs (o : operation) (n : nat) :=
-  match o with
-  | op_unit => False
-  | op_app _ r | op_retapp _ r => refs r n
-  end.
+  Lemma refsb_ref r i :
+    refsb r i = true <-> refs r i.
+  Proof.
+    induction r; cbn [refs refsb].
+    - crush_deciders idtac.
+    - rewrite orb_true_iff; intuition idtac.
+  Qed.
 
-Fixpoint bindings_ref (p : list operation) (n : nat) :=
-  match p with
-  | nil => False
-  | o :: p => op_refs o n \/ bindings_ref p (S n)
-  end.
+  Lemma op_refsb_ref o i :
+    op_refsb o i = true <-> op_refs o i.
+  Proof.
+    destruct o; cbn [op_refs op_refsb];
+      eauto using refsb_ref;
+      intuition congruence.
+  Qed.
 
-Definition expr_refs '((p, o) : expr) (n : nat) :=
-  bindings_ref p n \/ op_refs o (length p + n).
+  Lemma bindings_refb_ref p i :
+    bindings_refb p i = true <-> bindings_ref p i.
+  Proof.
+    revert i; induction p as [|o p]; intros i;
+      cbn [bindings_refb bindings_ref];
+      try intuition congruence.
+    rewrite orb_true_iff;
+      rewrite op_refsb_ref;
+      specialize (IHp (S i));
+      intuition idtac.
+  Qed.
 
-Fixpoint refsb (r : ref) (n : nat) :=
-  match r with
-  | ref_index k => n =? k
-  | ref_pair r1 r2 => refsb r1 n || refsb r2 n
-  end.
+  Fixpoint all_refsb (f : nat -> bool) (r : ref) : bool :=
+    match r with
+    | ref_index n => f n
+    | ref_pair r1 r2 => all_refsb f r1 && all_refsb f r2
+    end.
 
-Definition op_refsb (o : operation) (n : nat) :=
-  match o with
-  | op_unit => false
-  | op_app _ r | op_retapp _ r => refsb r n
-  end.
+  Definition op_all_refsb (f : nat -> bool) (o : op) : bool :=
+    match o with
+    | op_unit => true
+    | op_app _ r | op_retapp _ r => all_refsb f r
+    end.
 
-Fixpoint bindings_refb (p : list operation) (n : nat) :=
-  match p with
-  | nil => false
-  | o :: p => op_refsb o n || bindings_refb p (S n)
-  end.
+  Fixpoint bindings_all_refb (f : nat -> bool) (p : list op) : bool :=
+    match p with
+    | nil => true
+    | o :: p =>
+      op_all_refsb f o && bindings_all_refb (fun n => match n with
+                                                      | 0 => true
+                                                      | S n => f n
+                                                      end) p
+    end.
 
-Definition expr_refsb '((p, o) : expr) (n : nat) :=
-  bindings_refb p n || op_refsb o (length p + n).
+  Definition expr_all_refsb (f : nat -> bool) '((p, o) : expr) : bool :=
+    (bindings_all_refb f p)
+      && op_all_refsb (fun n => match n -? length p with
+                                | Some k => f k
+                                | None => true
+                                end) o.
 
-Lemma refsb_ref r i :
-  refsb r i = true <-> refs r i.
-Proof.
-  induction r; cbn [refs refsb].
-  - crush_deciders idtac.
-  - rewrite orb_true_iff; intuition idtac.
-Qed.
+  Lemma all_refsb_correct f r :
+    all_refsb f r = true ->
+    forall n, refs r n -> f n = true.
+  Proof.
+    intros.
+    induction r; cbn [all_refsb refs] in *.
+    - congruence.
+    - rewrite andb_true_iff in *; intuition idtac.
+  Qed.
 
-Lemma op_refsb_ref o i :
-  op_refsb o i = true <-> op_refs o i.
-Proof.
-  destruct o; cbn [op_refs op_refsb];
-    eauto using refsb_ref;
-    intuition congruence.
-Qed.
+  Lemma op_all_refsb_correct f o :
+    op_all_refsb f o = true ->
+    forall n, op_refs o n -> f n = true.
+  Proof.
+    intros; destruct o; cbn [op_all_refsb op_refs] in *;
+      rewrite ?andb_true_iff in *; intuition idtac;
+        eapply all_refsb_correct; eauto with nocore.
+  Qed.
 
-Lemma bindings_refb_ref p i :
-  bindings_refb p i = true <-> bindings_ref p i.
-Proof.
-  revert i; induction p as [|o p]; intros i;
-    cbn [bindings_refb bindings_ref];
-    try intuition congruence.
-  rewrite orb_true_iff;
-    rewrite op_refsb_ref;
-    specialize (IHp (S i));
-    intuition idtac.
-Qed.
+  Lemma bindings_all_refb_correct f p :
+    bindings_all_refb f p = true ->
+    forall n, bindings_ref p n -> f n = true.
+  Proof.
+    intros; revert dependent f; revert dependent n; induction p;
+      intros n Hn f Hf;
+      cbn [bindings_all_refb bindings_ref] in *;
+      intuition idtac;
+      rewrite ?andb_true_iff in *;
+      solve [(eapply op_all_refsb_correct +
+              eapply (IHp (S n) ltac:(eauto) (fun n => match n with
+                                                       | 0 => true
+                                                       | S n => f n
+                                                       end)));
+             intuition eauto with nocore].
+  Qed.
 
-Fixpoint all_refsb (f : nat -> bool) (r : ref) : bool :=
-  match r with
-  | ref_index n => f n
-  | ref_pair r1 r2 => all_refsb f r1 && all_refsb f r2
-  end.
+  Lemma expr_all_refsb_correct f e :
+    expr_all_refsb f e = true ->
+    forall n, expr_refs e n -> f n = true.
+  Proof.
+    destruct e as [p o];
+      cbn [expr_refs expr_all_refsb] in *;
+      rewrite ?andb_true_iff in *;
+      intros [? Ho] ? [?|?].
+    - eapply bindings_all_refb_correct; eauto with nocore.
+    - eapply op_all_refsb_correct in Ho; eauto with nocore.
+      match goal with
+      | _ : context[?a + ?b -? ?a] |- _ =>
+        replace (a + b -? a) with (Some b) in * by
+            (crush_deciders f_equal)
+      end; eauto with nocore.
+  Qed.
 
-Definition op_all_refsb (f : nat -> bool) (o : operation) : bool :=
-  match o with
-  | op_unit => true
-  | op_app _ r | op_retapp _ r => all_refsb f r
-  end.
+  Lemma bindings_ref_app (p1 p2 : list op) n :
+    bindings_ref (p1 ++ p2) n <->
+    bindings_ref p1 n \/ bindings_ref p2 (length p1 + n).
+  Proof.
+    revert n; induction p1; intros n; cbn [bindings_ref length plus app].
+    - intuition idtac.
+    - replace (S (length p1 + n)) with (length p1 + S n) by omega.
+      setoid_rewrite IHp1; intuition idtac.
+  Qed.
 
-Fixpoint bindings_all_refb (f : nat -> bool) (p : list operation) : bool :=
-  match p with
-  | nil => true
-  | o :: p =>
-    op_all_refsb f o && bindings_all_refb (fun n => match n with
-                                                    | 0 => true
-                                                    | S n => f n
-                                                    end) p
-  end.
+  Lemma renumber_ref_ext_relevant f f' r :
+    (forall i, refs r i -> f i = f' i) ->
+    renumber_ref f r = renumber_ref f' r.
+  Proof.
+    intros Hf; induction r; cbn [renumber_ref refs] in *.
+    - rewrite Hf; eauto.
+    - rewrite IHr1, IHr2; eauto.
+  Qed.
 
-Definition expr_all_refsb (f : nat -> bool) '((p, o) : expr) : bool :=
-  (bindings_all_refb f p)
-    && op_all_refsb (fun n => match n -? length p with
-                              | Some k => f k
-                              | None => true
-                              end) o.
+  Lemma renumber_ref_ext f f' r :
+    (forall i, f i = f' i) ->
+    renumber_ref f r = renumber_ref f' r.
+  Proof. eauto using renumber_ref_ext_relevant. Qed.
 
-Lemma all_refsb_correct f r :
-  all_refsb f r = true ->
-  forall n, refs r n -> f n = true.
-Proof.
-  intros.
-  induction r; cbn [all_refsb refs] in *.
-  - congruence.
-  - rewrite andb_true_iff in *; intuition idtac.
-Qed.
+  Lemma renumber_op_ext_relevant f f' o :
+    (forall i, op_refs o i -> f i = f' i) ->
+    renumber_op f o = renumber_op f' o.
+  Proof.
+    intros Hf; induction o; cbn [renumber_op];
+      try erewrite renumber_ref_ext_relevant; eauto.
+  Qed.
 
-Lemma op_all_refsb_correct f o :
-  op_all_refsb f o = true ->
-  forall n, op_refs o n -> f n = true.
-Proof.
-  intros; destruct o; cbn [op_all_refsb op_refs] in *;
-    rewrite ?andb_true_iff in *; intuition idtac;
-      eapply all_refsb_correct; eauto with nocore.
-Qed.
+  Lemma renumber_op_ext f f' o :
+    (forall i, f i = f' i) ->
+    renumber_op f o = renumber_op f' o.
+  Proof. eauto using renumber_op_ext_relevant. Qed.
 
-Lemma bindings_all_refb_correct f p :
-  bindings_all_refb f p = true ->
-  forall n, bindings_ref p n -> f n = true.
-Proof.
-  intros; revert dependent f; revert dependent n; induction p;
-    intros n Hn f Hf;
-    cbn [bindings_all_refb bindings_ref] in *;
-    intuition idtac;
-    rewrite ?andb_true_iff in *;
-    solve [(eapply op_all_refsb_correct +
-            eapply (IHp (S n) ltac:(eauto) (fun n => match n with
-                                                     | 0 => true
-                                                     | S n => f n
-                                                     end)));
-           intuition eauto with nocore].
-Qed.
+  Lemma renumber_bindings_ext_relevant f f' p :
+    (forall i, bindings_ref p i -> f i = f' i) ->
+    renumber_bindings f p = renumber_bindings f' p.
+  Proof.
+    revert f f'; induction p as [|o p]; eauto.
+    intros; cbn [renumber_bindings bindings_ref] in *.
+    f_equal; try (erewrite renumber_op_ext_relevant; eauto).
+    apply IHp.
+    intros []; cbv [offset_renumbering optsub]; eauto.
+  Qed.
 
-Lemma expr_all_refsb_correct f e :
-  expr_all_refsb f e = true ->
-  forall n, expr_refs e n -> f n = true.
-Proof.
-  destruct e as [p o];
-    cbn [expr_refs expr_all_refsb] in *;
-    rewrite ?andb_true_iff in *;
-    intros [? Ho] ? [?|?].
-  - eapply bindings_all_refb_correct; eauto with nocore.
-  - eapply op_all_refsb_correct in Ho; eauto with nocore.
+  Lemma renumber_bindings_ext f f' p :
+    (forall i, f i = f' i) ->
+    renumber_bindings f p = renumber_bindings f' p.
+  Proof. eauto using renumber_bindings_ext_relevant. Qed.
+
+  Lemma offset_renumbering_plus a b n f :
+    offset_renumbering (a + b) f n =
+    offset_renumbering a (offset_renumbering b f) n.
+  Proof.
+    cbv [offset_renumbering] in *.
+    crush_deciders idtac.
+    subst.
     match goal with
-    | _ : context[?a + ?b -? ?a] |- _ =>
-      let t := f_equal in
-      replace (a + b -? a) with (Some b) in * by
-          (crush_deciders t)
-    end; eauto with nocore.
-Qed.
+    | _ : (_ + _ + ?x) = (_ + (_ + ?y)) |- _ => assert (x = y) by omega
+    end.
+    subst; omega.
+  Qed.
 
-Lemma bindings_ref_app (p1 p2 : list operation) n :
-  bindings_ref (p1 ++ p2) n <->
-  bindings_ref p1 n \/ bindings_ref p2 (length p1 + n).
-Proof.
-  revert n; induction p1; intros n; cbn [bindings_ref length plus app].
-  - intuition idtac.
-  - replace (S (length p1 + n)) with (length p1 + S n) by omega.
-    setoid_rewrite IHp1; intuition idtac.
-Qed.
+  Lemma renumber_expr'_renumber_bindings acc f p o' :
+    renumber_expr' acc f p o' =
+    (rev acc ++ renumber_bindings f p,
+     renumber_op (offset_renumbering (length p) f) o').
+  Proof.
+    revert acc f; induction p; intros acc f;
+      cbn [renumber_expr' renumber_bindings length].
+    - setoid_rewrite renumber_op_ext with (f' := f) at 2;
+        [|reflexivity].
+      listrew; eauto.
+    - rewrite IHp.
+      listrew.
+      f_equal.
+      eapply renumber_op_ext.
+      intros;
+        rewrite <-offset_renumbering_plus;
+        f_equal; omega.
+  Qed.
 
-Lemma renumber_ref_ext_relevant f f' r :
-  (forall i, refs r i -> f i = f' i) ->
-  renumber_ref f r = renumber_ref f' r.
-Proof.
-  intros Hf; induction r; cbn [renumber_ref refs] in *.
-  - rewrite Hf; eauto.
-  - rewrite IHr1, IHr2; eauto.
-Qed.
+  Lemma renumber_expr_renumber_bindings f p o' :
+    renumber_expr f (p, o') =
+    (renumber_bindings f p,
+     renumber_op (offset_renumbering (length p) f) o').
+  Proof. eapply renumber_expr'_renumber_bindings. Qed.
 
-Lemma renumber_ref_ext f f' r :
-  (forall i, f i = f' i) ->
-  renumber_ref f r = renumber_ref f' r.
-Proof. eauto using renumber_ref_ext_relevant. Qed.
+  Lemma renumber_expr_ext_relevant f f' e :
+    (forall i, expr_refs e i -> f i = f' i) ->
+    renumber_expr f e = renumber_expr f' e.
+  Proof.
+    destruct e as [p o];
+      repeat rewrite renumber_expr_renumber_bindings;
+      cbn [expr_refs].
+    intros.
+    rewrite renumber_bindings_ext_relevant with (f' := f') by
+        intuition eauto.
+    rewrite renumber_op_ext_relevant with
+        (f' := (offset_renumbering (length p) f')); eauto.
+    intros.
+    cbv [offset_renumbering];
+      crush_deciders (subst; eauto).
+  Qed.
 
-Lemma renumber_op_ext_relevant f f' o :
-  (forall i, op_refs o i -> f i = f' i) ->
-  renumber_op f o = renumber_op f' o.
-Proof.
-  intros Hf; induction o; cbn [renumber_op];
-    try erewrite renumber_ref_ext_relevant; eauto.
-Qed.
+  Lemma renumber_expr_ext f f' e :
+    (forall i, f i = f' i) ->
+    renumber_expr f e = renumber_expr f' e.
+  Proof. eauto using renumber_expr_ext_relevant. Qed.
 
-Lemma renumber_op_ext f f' o :
-  (forall i, f i = f' i) ->
-  renumber_op f o = renumber_op f' o.
-Proof. eauto using renumber_op_ext_relevant. Qed.
-
-Lemma renumber_bindings_ext_relevant f f' p :
-  (forall i, bindings_ref p i -> f i = f' i) ->
-  renumber_bindings f p = renumber_bindings f' p.
-Proof.
-  revert f f'; induction p as [|o p]; eauto.
-  intros; cbn [renumber_bindings bindings_ref] in *.
-  f_equal; try (erewrite renumber_op_ext_relevant; eauto).
-  apply IHp.
-  intros []; cbv [offset_renumbering optsub]; eauto.
-Qed.
-
-Lemma renumber_bindings_ext f f' p :
-  (forall i, f i = f' i) ->
-  renumber_bindings f p = renumber_bindings f' p.
-Proof. eauto using renumber_bindings_ext_relevant. Qed.
-
-Lemma offset_renumbering_plus a b n f :
-  offset_renumbering (a + b) f n =
-  offset_renumbering a (offset_renumbering b f) n.
-Proof.
-  cbv [offset_renumbering] in *.
-  crush_deciders idtac.
-  subst.
-  match goal with
-  | _ : (_ + _ + ?x) = (_ + (_ + ?y)) |- _ => assert (x = y) by omega
-  end.
-  subst; omega.
-Qed.
-
-Lemma renumber_expr'_renumber_bindings acc f p o' :
-  renumber_expr' acc f p o' =
-  (rev acc ++ renumber_bindings f p,
-   renumber_op (offset_renumbering (length p) f) o').
-Proof.
-  revert acc f; induction p; intros acc f;
-    cbn [renumber_expr' renumber_bindings length].
-  - setoid_rewrite renumber_op_ext with (f' := f) at 2;
-      [|reflexivity].
-    listrew; eauto.
-  - rewrite IHp.
+  Lemma renumber_bindings_app (f : nat -> nat) (p1 p2 : list op) :
+    renumber_bindings f (p1 ++ p2) =
+    (renumber_bindings f p1)
+      ++ renumber_bindings (offset_renumbering (length p1) f) p2.
+  Proof.
+    revert f; induction p1; intros f; eauto.
+    listrew.
+    cbn [renumber_bindings offset_renumbering optsub length].
     listrew.
     f_equal.
-    eapply renumber_op_ext.
-    intros;
-      rewrite <-offset_renumbering_plus;
-      f_equal; omega.
-Qed.
+    rewrite <-(Nat.add_1_r (length p1)).
+    erewrite (renumber_bindings_ext (offset_renumbering (length p1 + 1) f));
+      eauto using offset_renumbering_plus.
+  Qed.
 
-Lemma renumber_expr_renumber_bindings f p o' :
-  renumber_expr f (p, o') =
-  (renumber_bindings f p,
-   renumber_op (offset_renumbering (length p) f) o').
-Proof. eapply renumber_expr'_renumber_bindings. Qed.
+  Definition context_renumbered (f : nat -> nat)
+             ctxt (ctx : interp_type ctxt)
+             ctxt' (ctx' : interp_type ctxt') : Prop :=
+    forall i t, lookup ctxt' ctx' (f i) t = lookup ctxt ctx i t.
 
-Lemma renumber_expr_ext_relevant f f' e :
-  (forall i, expr_refs e i -> f i = f' i) ->
-  renumber_expr f e = renumber_expr f' e.
-Proof.
-  destruct e as [p o];
-    repeat rewrite renumber_expr_renumber_bindings;
-    cbn [expr_refs].
-  intros.
-  rewrite renumber_bindings_ext_relevant with (f' := f') by
-    intuition eauto.
-  rewrite renumber_op_ext_relevant with
-      (f' := (offset_renumbering (length p) f')); eauto.
-  intros.
-  cbv [offset_renumbering];
-    let t := (subst; eauto) in
-    crush_deciders t.
-Qed.
+  Lemma context_renumbered_ext f1 f2 ctxt ctx ctxt' ctx' :
+    (forall n, f1 n = f2 n) ->
+    context_renumbered f1 ctxt ctx ctxt' ctx' <->
+    context_renumbered f2 ctxt ctx ctxt' ctx'.
+  Proof. intuition congruence. Qed.
 
-Lemma renumber_expr_ext f f' e :
-  (forall i, f i = f' i) ->
-  renumber_expr f e = renumber_expr f' e.
-Proof. eauto using renumber_expr_ext_relevant. Qed.
+  Definition continuation_renumbered (f : nat -> nat) tk
+             (k k' : forall ctxt : type, interp_type ctxt -> M tk) :=
+    forall ctxt (ctx : interp_type ctxt) ctxt' (ctx' : interp_type ctxt'),
+      context_renumbered f ctxt ctx ctxt' ctx' ->
+      Mequiv (k ctxt ctx) (k' ctxt' ctx').
 
-Lemma renumber_bindings_app (f : nat -> nat) (p1 p2 : list operation) :
-  renumber_bindings f (p1 ++ p2) =
-  (renumber_bindings f p1)
-    ++ renumber_bindings (offset_renumbering (length p1) f) p2.
-Proof.
-  revert f; induction p1; intros f; eauto.
-  listrew.
-  cbn [renumber_bindings offset_renumbering optsub length].
-  listrew.
-  f_equal.
-  rewrite <-(Nat.add_1_r (length p1)).
-  erewrite (renumber_bindings_ext (offset_renumbering (length p1 + 1) f));
-    eauto using offset_renumbering_plus.
-Qed.
+  Lemma continuation_renumbered_ext f1 f2 tk k k' :
+    (forall i, f1 i = f2 i) ->
+    continuation_renumbered f1 tk k k' ->
+    continuation_renumbered f2 tk k k'.
+  Proof. intros ???????; rewrite context_renumbered_ext in *; eauto. Qed.
 
-Definition context_renumbered (f : nat -> nat)
-           ctxt (ctx : interp_type ctxt)
-           ctxt' (ctx' : interp_type ctxt') : Prop :=
-  forall i t, lookup ctxt' ctx' (f i) t = lookup ctxt ctx i t.
+  Local Instance continuation_renumbered_Mequiv f tk :
+    Proper ((forall_relation
+               (fun ctxt => pointwise_relation (interp_type ctxt) Mequiv)
+               ==>
+               (forall_relation
+                  (fun ctxt => pointwise_relation (interp_type ctxt) Mequiv))
+               ==> iff)) (continuation_renumbered f tk).
+  Proof.
+    cbv [Proper respectful forall_relation pointwise_relation Basics.impl].
+    cbv [continuation_renumbered].
+    intros k1 k1' Hk1 k2 k2' Hk2.
+    split; intros H ctxt ctx ctxt' ctx';
+      (etransitivity; [|etransitivity];
+       [|eapply H|]);
+      solve [eauto | symmetry; eauto].
+  Qed.
 
-Lemma context_renumbered_ext f1 f2 ctxt ctx ctxt' ctx' :
-  (forall n, f1 n = f2 n) ->
-  context_renumbered f1 ctxt ctx ctxt' ctx' <->
-  context_renumbered f2 ctxt ctx ctxt' ctx'.
-Proof. intuition congruence. Qed.
-
-Definition continuation_renumbered (f : nat -> nat) tk
-           (k k' : forall ctxt : type, interp_type ctxt -> M tk) :=
-  forall ctxt (ctx : interp_type ctxt) ctxt' (ctx' : interp_type ctxt'),
+  Lemma context_renumbered_1 f ctxt ctx ctxt' ctx' t
+        (x : interp_type t) :
     context_renumbered f ctxt ctx ctxt' ctx' ->
-    Mequiv (k ctxt ctx) (k' ctxt' ctx').
+    context_renumbered (offset_renumbering 1 f)
+                       (t * ctxt) (x, ctx) (t * ctxt') (x, ctx').
+  Proof.
+    cbv [context_renumbered].
+    intros ? n u.
+    destruct n; cbn [lookup offset_renumbering optsub].
+    - reflexivity.
+    - rewrite Nat.add_1_l.
+      cbn [lookup].
+      eauto.
+  Qed.
 
-Lemma continuation_renumbered_ext f1 f2 tk k k' :
-  (forall i, f1 i = f2 i) ->
-  continuation_renumbered f1 tk k k' ->
-  continuation_renumbered f2 tk k k'.
-Proof. intros ???????; rewrite context_renumbered_ext in *; eauto. Qed.
+  Lemma lookup_renumbered_ref ctxt ctx ctxt' ctx' f r t :
+    context_renumbered f ctxt ctx ctxt' ctx' ->
+    lookup_ref ctxt' ctx' (renumber_ref f r) t =
+    lookup_ref ctxt ctx r t.
+  Proof.
+    cbv [context_renumbered].
+    intros ?.
+    revert t; induction r; intros t;
+      cbn [lookup_ref renumber_ref] in *; eauto.
+    destruct t; eauto.
+    rewrite IHr1, IHr2; reflexivity.
+  Qed.
 
-Local Instance continuation_renumbered_Mequiv f tk :
-  Proper ((forall_relation
-             (fun ctxt => pointwise_relation (interp_type ctxt) Mequiv)
-             ==>
-             (forall_relation
-                (fun ctxt => pointwise_relation (interp_type ctxt) Mequiv))
-             ==> iff)) (continuation_renumbered f tk).
-Proof.
-  cbv [Proper respectful forall_relation pointwise_relation Basics.impl].
-  cbv [continuation_renumbered].
-  intros; split; intros.
-  - etransitivity; [symmetry; eauto|];
-      etransitivity; [|eauto]; eauto.
-  - etransitivity; [|symmetry; eauto];
-      etransitivity; [eauto|]; eauto.
-Qed.
+  Lemma interp_renumbered_op f o tk
+        (k k' : forall ctxt, interp_type ctxt -> M tk) :
+    continuation_renumbered (offset_renumbering 1 f) tk k k' ->
+    continuation_renumbered
+      f tk
+      (fun ctxt ctx =>
+         (Mbind (interp_op_silent ctxt ctx o)
+                (fun x => k (op_type o * ctxt)%etype (x, ctx))))
+      (fun ctxt ctx =>
+         (Mbind
+            (interp_op_silent ctxt ctx
+                              (renumber_op f o))
+            (fun x => k'
+                        (op_type (renumber_op f o) *
+                         ctxt)%etype (x, ctx)))).
+  Proof.
+    intros Hk ?????.
+    destruct o; cbn [renumber_op op_type op_refs] in *;
+      (step_Mequiv; [..|eapply Hk; eapply context_renumbered_1; eauto]);
+      cbv [interp_op_silent interp_op];
+      erewrite lookup_renumbered_ref by eauto;
+      reflexivity.
+  Qed.
 
-Lemma context_renumbered_1 f ctxt ctx ctxt' ctx' t
-      (x : interp_type t) :
-  context_renumbered f ctxt ctx ctxt' ctx' ->
-  context_renumbered (offset_renumbering 1 f)
-                     (t * ctxt) (x, ctx) (t * ctxt') (x, ctx').
-Proof.
-  cbv [context_renumbered].
-  intros ? n u.
-  destruct n; cbn [lookup offset_renumbering optsub].
-  - reflexivity.
-  - rewrite Nat.add_1_l.
-    cbn [lookup].
-    eauto.
-Qed.
+  Lemma interp_renumbered_op_no_ctx f o tk
+        (k k' : forall t, interp_type t -> M tk) :
+    (forall t x, Mequiv (k t x) (k' t x)) ->
+    continuation_renumbered
+      f tk
+      (fun ctxt ctx =>
+         (Mbind (interp_op_silent ctxt ctx o)
+                (fun x => k (op_type o) x)))
+      (fun ctxt ctx =>
+         (Mbind
+            (interp_op_silent ctxt ctx
+                              (renumber_op f o))
+            (fun x => k'
+                        (op_type (renumber_op f o)) x))).
+  Proof.
+    intros Hk ?????.
+    destruct o; cbn [renumber_op op_type op_refs] in *;
+      (step_Mequiv; [..|eapply Hk]);
+      cbv [interp_op_silent interp_op];
+      erewrite lookup_renumbered_ref by eauto;
+      reflexivity.
+  Qed.
 
-Lemma lookup_renumbered_ref ctxt ctx ctxt' ctx' f r t :
-  context_renumbered f ctxt ctx ctxt' ctx' ->
-  lookup_ref ctxt' ctx' (renumber_ref f r) t =
-  lookup_ref ctxt ctx r t.
-Proof.
-  cbv [context_renumbered].
-  intros ?.
-  revert t; induction r; intros t;
-    cbn [lookup_ref renumber_ref] in *; eauto.
-  destruct t; eauto.
-  rewrite IHr1, IHr2; reflexivity.
-Qed.
+  Lemma interp_renumbered_bindings (f : nat -> nat)
+        (p : list op)
+        tk (k k' : forall ctxt : type, interp_type ctxt -> M tk) :
+    continuation_renumbered (offset_renumbering (length p) f) tk k k' ->
+    continuation_renumbered
+      f tk
+      (fun ctxt ctx => interp_bindings ctxt ctx p tk k)
+      (fun ctxt ctx => interp_bindings ctxt ctx (renumber_bindings f p) tk k').
+  Proof.
+    revert tk k k'.
+    pattern p; revert p; eapply rev_ind;
+      cbn [renumber_bindings interp_bindings length offset_renumbering
+                             optsub plus]; eauto.
+    intros o p IHp tk k k' Hkk'.
+    rewrite renumber_bindings_app.
+    cbn [renumber_bindings].
+    setoid_rewrite interp_bindings_app.
+    eapply IHp; eauto.
+    cbn [interp_bindings].
+    intros ?????.
+    eapply interp_renumbered_op; eauto.
+    listrew.
+    replace (S (length p)) with (1 + length p) in * by omega.
+    eapply (continuation_renumbered_ext
+              _ _ _ _ _
+              ltac:(intros; eapply offset_renumbering_plus)) in Hkk'; eauto.
+  Qed.
 
-Lemma interp_renumbered_op f o tk
-      (k k' : forall ctxt, interp_type ctxt -> M tk) :
-  continuation_renumbered (offset_renumbering 1 f) tk k k' ->
-  continuation_renumbered
-    f tk
-    (fun ctxt ctx =>
-       (Mbind (interp_op_silent ctxt ctx o)
-              (fun x => k (op_type o * ctxt)%etype (x, ctx))))
-    (fun ctxt ctx =>
-       (Mbind
-          (interp_op_silent ctxt ctx
-                            (renumber_op f o))
-          (fun x => k'
-                      (op_type (renumber_op f o) *
-                       ctxt)%etype (x, ctx)))).
-Proof.
-  intros Hk ?????.
-  destruct o; cbn [renumber_op op_type op_refs] in *;
-    (step_Mequiv; [..|eapply Hk; eapply context_renumbered_1; eauto]);
-    cbv [interp_op_silent interp_op];
-    erewrite lookup_renumbered_ref by eauto;
-    reflexivity.
-Qed.
+  Lemma interp_renumbered_expr (f : nat -> nat) t (e : expr) :
+    continuation_renumbered
+      f t
+      (fun ctxt ctx => interp_expr_cast ctxt ctx e t)
+      (fun ctxt ctx => interp_expr_cast ctxt ctx (renumber_expr f e) t).
+  Proof.
+    intros ?????.
+    destruct e as [p o].
+    rewrite renumber_expr_renumber_bindings.
+    cbv [interp_expr_cast interp_expr].
+    setoid_rewrite bind_interp_bindings.
+    eapply interp_renumbered_bindings; eauto.
+    refine (interp_renumbered_op_no_ctx
+              _ _ _
+              (fun _ x => Mret (cast t x))
+              (fun _ x => Mret (cast t x)) _); reflexivity.
+  Qed.
 
-Lemma interp_renumbered_op_no_ctx f o tk
-      (k k' : forall t, interp_type t -> M tk) :
-  (forall t x, Mequiv (k t x) (k' t x)) ->
-  continuation_renumbered
-    f tk
-    (fun ctxt ctx =>
-       (Mbind (interp_op_silent ctxt ctx o)
-              (fun x => k (op_type o) x)))
-    (fun ctxt ctx =>
-       (Mbind
-          (interp_op_silent ctxt ctx
-                            (renumber_op f o))
-          (fun x => k'
-                      (op_type (renumber_op f o)) x))).
-Proof.
-  intros Hk ?????.
-  destruct o; cbn [renumber_op op_type op_refs] in *;
-    (step_Mequiv; [..|eapply Hk]);
-    cbv [interp_op_silent interp_op];
-    erewrite lookup_renumbered_ref by eauto;
-    reflexivity.
-Qed.
+  Lemma lookup_unref_0 ctxt (ctx : interp_type ctxt)
+        t (x : interp_type t) r u :
+    ~refs r 0 ->
+    lookup_ref (t * ctxt) (x, ctx) r u =
+    lookup_ref ctxt ctx (renumber_ref pred r) u.
+  Proof.
+    intros.
+    revert u; induction r; intros u; cbn [refs] in *.
+    - destruct n; cbn [lookup_ref lookup renumber_ref pred];
+        congruence.
+    - cbn [lookup_ref lookup renumber_ref].
+      destruct u; try reflexivity.
+      rewrite IHr1, IHr2 by intuition idtac.
+      reflexivity.
+  Qed.
 
-Lemma interp_renumbered_bindings (f : nat -> nat)
-      (p : list operation)
-      tk (k k' : forall ctxt : type, interp_type ctxt -> M tk) :
-  continuation_renumbered (offset_renumbering (length p) f) tk k k' ->
-  continuation_renumbered
-    f tk
-    (fun ctxt ctx => interp_bindings ctxt ctx p tk k)
-    (fun ctxt ctx => interp_bindings ctxt ctx (renumber_bindings f p) tk k').
-Proof.
-  revert tk k k'.
-  pattern p; revert p; eapply rev_ind;
-    cbn [renumber_bindings interp_bindings length offset_renumbering
-                           optsub plus]; eauto.
-  intros o p IHp tk k k' Hkk'.
-  rewrite renumber_bindings_app.
-  cbn [renumber_bindings].
-  setoid_rewrite interp_bindings_app.
-  eapply IHp; eauto.
-  cbn [interp_bindings].
-  intros ?????.
-  eapply interp_renumbered_op; eauto.
-  listrew.
-  replace (S (length p)) with (1 + length p) in * by omega.
-  eapply (continuation_renumbered_ext
-            _ _ _ _ _
-            ltac:(intros; eapply offset_renumbering_plus)) in Hkk'; eauto.
-Qed.
+  Lemma lookup_ref_S ctxt (ctx : interp_type ctxt)
+        t (x : interp_type t) r u :
+    lookup_ref (t * ctxt) (x, ctx) (renumber_ref S r) u =
+    lookup_ref ctxt ctx r u.
+  Proof.
+    intros.
+    revert u; induction r; intros u.
+    - reflexivity.
+    - cbn [renumber_ref lookup_ref lookup].
+      destruct u; try reflexivity.
+      rewrite IHr1, IHr2.
+      reflexivity.
+  Qed.
 
-Lemma interp_renumbered_expr (f : nat -> nat) t (e : expr) :
-  continuation_renumbered
-    f t
-    (fun ctxt ctx => interp_expr_cast ctxt ctx e t)
-    (fun ctxt ctx => interp_expr_cast ctxt ctx (renumber_expr f e) t).
-Proof.
-  intros ?????.
-  destruct e as [p o].
-  rewrite renumber_expr_renumber_bindings.
-  cbv [interp_expr_cast interp_expr].
-  setoid_rewrite bind_interp_bindings.
-  eapply interp_renumbered_bindings; eauto.
-  refine (interp_renumbered_op_no_ctx
-            _ _ _
-            (fun _ x => Mret (cast t x))
-            (fun _ x => Mret (cast t x)) _); reflexivity.
-Qed.
+  Lemma commute_ops ctxt (ctx : interp_type ctxt)
+        (o1 o2 : op)
+        tk (k k' : forall ctxt, interp_type ctxt -> M tk) :
+    ~op_refs o2 0 ->
+    continuation_renumbered (fun n => match n with
+                                      | 0 => 1
+                                      | 1 => 0
+                                      | _ => n
+                                      end) tk k k' ->
+    Mequiv (interp_bindings ctxt ctx (o1 :: o2 :: nil) tk k)
+           (interp_bindings ctxt ctx
+                            (renumber_op pred o2 :: renumber_op S o1 :: nil)
+                            tk k').
+  Proof.
+    intros Ho2 Hk.
+    cbn [interp_bindings].
 
-Lemma lookup_unref_0 ctxt (ctx : interp_type ctxt)
-      t (x : interp_type t) r u :
-  ~refs r 0 ->
-  lookup_ref (t * ctxt) (x, ctx) r u =
-  lookup_ref ctxt ctx (renumber_ref pred r) u.
-Proof.
-  intros.
-  revert u; induction r; intros u; cbn [refs] in *.
-  - destruct n; cbn [lookup_ref lookup renumber_ref pred];
-      congruence.
-  - cbn [lookup_ref lookup renumber_ref].
-    destruct u; try reflexivity.
-    rewrite IHr1, IHr2 by intuition idtac.
-    reflexivity.
-Qed.
+    transitivity
+      (Mbind (interp_op_silent ctxt ctx o1)
+             (fun x =>
+                Mbind (interp_op_silent (op_type o1 * ctxt) (x, ctx) o2)
+                      (fun y =>
+                         k' (op_type o1 * (op_type o2 * ctxt))%etype
+                            (x, (y, ctx))))).
+    { step_Mequiv.
+      eapply Hk.
+      intros [|[]] ?; reflexivity. }
 
-Lemma lookup_ref_S ctxt (ctx : interp_type ctxt)
-      t (x : interp_type t) r u :
-  lookup_ref (t * ctxt) (x, ctx) (renumber_ref S r) u =
-  lookup_ref ctxt ctx r u.
-Proof.
-  intros.
-  revert u; induction r; intros u.
-  - reflexivity.
-  - cbn [renumber_ref lookup_ref lookup].
-    destruct u; try reflexivity.
-    rewrite IHr1, IHr2.
-    reflexivity.
-Qed.
-
-Lemma commute_ops ctxt (ctx : interp_type ctxt)
-      (o1 o2 : operation)
-      tk (k k' : forall ctxt, interp_type ctxt -> M tk) :
-  ~op_refs o2 0 ->
-  continuation_renumbered (fun n => match n with
-                                    | 0 => 1
-                                    | 1 => 0
-                                    | _ => n
-                                    end) tk k k' ->
-  Mequiv (interp_bindings ctxt ctx (o1 :: o2 :: nil) tk k)
-         (interp_bindings ctxt ctx
-                          (renumber_op pred o2 :: renumber_op S o1 :: nil)
-                          tk k').
-Proof.
-  intros Ho2 Hk.
-  cbn [interp_bindings].
-
-  transitivity
+    transitivity
     (Mbind (interp_op_silent ctxt ctx o1)
            (fun x =>
-              Mbind (interp_op_silent (op_type o1 * ctxt) (x, ctx) o2)
+              Mbind (interp_op_silent ctxt ctx (renumber_op pred o2))
                     (fun y =>
-                       k' (op_type o1 * (op_type o2 * ctxt))%etype
+                       k' (op_type o1 *
+                           (op_type (renumber_op pred o2) * ctxt))%etype
                           (x, (y, ctx))))).
-  { step_Mequiv.
-    eapply Hk.
-    intros [|[]] ?; reflexivity. }
+    { step_Mequiv.
+      destruct o2; cbn [op_type renumber_op];
+        step_Mequiv;
+        cbn [op_refs] in Ho2; cbv [interp_op_silent interp_op];
+          rewrite lookup_unref_0 by eauto;
+          reflexivity. }
 
-  transitivity
-  (Mbind (interp_op_silent ctxt ctx o1)
-         (fun x =>
-            Mbind (interp_op_silent ctxt ctx (renumber_op pred o2))
-                  (fun y =>
-                     k' (op_type o1 *
-                         (op_type (renumber_op pred o2) * ctxt))%etype
-                        (x, (y, ctx))))).
-  { step_Mequiv.
-    destruct o2; cbn [op_type renumber_op];
-      step_Mequiv;
-      cbn [op_refs] in Ho2; cbv [interp_op_silent interp_op];
-        rewrite lookup_unref_0 by eauto;
-        reflexivity. }
+    transitivity
+    (Mbind (interp_op_silent ctxt ctx (renumber_op pred o2))
+           (fun y =>
+              Mbind (interp_op_silent ctxt ctx o1)
+                    (fun x =>
+                       k' (op_type o1 *
+                           (op_type (renumber_op pred o2) * ctxt))%etype
+                          (x, (y, ctx))))).
+    { eapply Mbind_comm. }
 
-  transitivity
-  (Mbind (interp_op_silent ctxt ctx (renumber_op pred o2))
-         (fun y =>
-            Mbind (interp_op_silent ctxt ctx o1)
-                  (fun x =>
-                     k' (op_type o1 *
-                         (op_type (renumber_op pred o2) * ctxt))%etype
-                        (x, (y, ctx))))).
-  { eapply Mbind_comm. }
+    { step_Mequiv.
+      destruct o1; cbn [op_type renumber_op];
+        step_Mequiv; try reflexivity;
+          cbv [interp_op_silent interp_op];
+          rewrite lookup_ref_S;
+          reflexivity. }
+  Qed.
 
-  { step_Mequiv.
-    destruct o1; cbn [op_type renumber_op];
-      step_Mequiv; try reflexivity;
-      cbv [interp_op_silent interp_op];
-      rewrite lookup_ref_S;
-      reflexivity. }
-Qed.
+  Section RenumberRenumber.
+    Context (h g f : nat -> nat)
+            (Ih : forall x, h x = g (f x)).
+    Lemma renumber_renumber_ref r :
+      renumber_ref h r = renumber_ref g (renumber_ref f r).
+    Proof. induction r; cbn [renumber_ref]; congruence. Qed.
+    Lemma renumber_renumber_op o :
+      renumber_op h o = renumber_op g (renumber_op f o).
+    Proof. destruct o; cbn [renumber_op];
+             repeat rewrite renumber_renumber_ref; eauto. Qed.
+  End RenumberRenumber.
 
-Section RenumberRenumber.
-  Context (h g f : nat -> nat)
-          (Ih : forall x, h x = g (f x)).
-  Lemma renumber_renumber_ref r :
-    renumber_ref h r = renumber_ref g (renumber_ref f r).
-  Proof. induction r; cbn [renumber_ref]; congruence. Qed.
-  Lemma renumber_renumber_op o :
-    renumber_op h o = renumber_op g (renumber_op f o).
-  Proof. destruct o; cbn [renumber_op];
-           repeat rewrite renumber_renumber_ref; eauto. Qed.
-End RenumberRenumber.
+  Lemma renumber_renumber_bindings (h g f : nat -> nat) p :
+    (forall x, h x = g (f x)) ->
+    renumber_bindings h p = renumber_bindings g (renumber_bindings f p).
+  Proof.
+    revert h g f; induction p; intros h g f Ih; cbn [renumber_bindings]; eauto.
+    erewrite (renumber_renumber_op h); eauto.
+    erewrite IHp; eauto.
+    intros []; cbn [offset_renumbering optsub plus]; eauto.
+  Qed.
 
-Lemma renumber_renumber_bindings (h g f : nat -> nat) p :
-  (forall x, h x = g (f x)) ->
-  renumber_bindings h p = renumber_bindings g (renumber_bindings f p).
-Proof.
-  revert h g f; induction p; intros h g f Ih; cbn [renumber_bindings]; eauto.
-  erewrite (renumber_renumber_op h); eauto.
-  erewrite IHp; eauto.
-  intros []; cbn [offset_renumbering optsub plus]; eauto.
-Qed.
+  Lemma length_renumber f p : length (renumber_bindings f p) = length p.
+  Proof. revert f; induction p; cbn [renumber_bindings length]; congruence. Qed.
 
-Lemma length_renumber f p : length (renumber_bindings f p) = length p.
-Proof. revert f; induction p; cbn [renumber_bindings length]; congruence. Qed.
+  Lemma offset_renumbering_ext n f f' :
+    (forall i, f i = f' i) ->
+    (forall i, offset_renumbering n f i = offset_renumbering n f' i).
+  Proof. cbv [offset_renumbering]; crush_deciders eauto. Qed.
 
-Lemma offset_renumbering_ext n f f' :
-  (forall i, f i = f' i) ->
-  (forall i, offset_renumbering n f i = offset_renumbering n f' i).
-Proof. cbv [offset_renumbering]; crush_deciders eauto. Qed.
-
-Lemma renumber_renumber_expr (h g f : nat -> nat) e :
-  (forall x, h x = g (f x)) ->
-  renumber_expr h e = renumber_expr g (renumber_expr f e).
-Proof.
-  intros Hh; destruct e.
-  repeat rewrite renumber_expr_renumber_bindings.
-  f_equal.
-  - eapply renumber_renumber_bindings; eauto.
-  - eapply renumber_renumber_op.
-    intros; rewrite length_renumber.
-    erewrite offset_renumbering_ext by eapply Hh.
-    cbv [offset_renumbering]; crush_deciders idtac.
-    match goal with
-    | H : ?a + ?b = ?a + ?c |- _ => assert (b = c) by omega
-    end;
-      subst; eauto.
-Qed.
-
-Lemma refs_renumber f r j :
-  refs (renumber_ref f r) j <-> exists i, f i = j /\ refs r i.
-Proof.
-  induction r; cbn [renumber_ref refs];
-    intuition repeat match goal with
-                     | H : exists _, _ |- _ => destruct H as (?&<-&?)
-                     | _ => intuition eauto
-                     end.
-Qed.
-
-Lemma op_refs_renumber f o j :
-  op_refs (renumber_op f o) j <-> exists i, f i = j /\ op_refs o i.
-Proof.
-  destruct o; cbn [renumber_op op_refs];
-    intuition repeat match goal with
-                     | H : exists _, _ |- _ => destruct H as (?&<-&?)
-                     | H : _ |- _ => setoid_rewrite refs_renumber in H
-                     | _ => setoid_rewrite refs_renumber
-                     | _ => intuition eauto
-                     end.
-Qed.
-
-Lemma bindings_ref_renumber f p j :
-  bindings_ref (renumber_bindings f p) j <->
-  exists i, f i = j /\ bindings_ref p i.
-Proof.
-  revert f j; induction p; intros;
-    intuition repeat multimatch goal with
-                     | H : exists _, _ |- _ => destruct H as (?&<-&?)
-                     | H : _ |- _ => setoid_rewrite op_refs_renumber in H
-                     | _ => setoid_rewrite op_refs_renumber
-                     | _ => cbn [bindings_ref renumber_bindings] in *
-                     | _ => intuition eauto
-                     end.
-  - rewrite IHp in *;
-      repeat match goal with
-             | H : exists _, _ |- _ =>
-               let x := fresh in
-               destruct H as ([]&?&?);
-                 cbv [offset_renumbering optsub] in *
-             | _ => congruence
-             | _ => intuition eauto
-             end.
-  - rewrite IHp;
-      right; eexists (S _); cbv [offset_renumbering optsub]; eauto.
-Qed.
-
-Lemma offset_eq_inv a f i j :
-  offset_renumbering a f i = a + j ->
-  i >= a /\ f (i - a) = j.
-Proof.
-  cbv [offset_renumbering]; crush_deciders subst.
-  match goal with
-  | |- context[?a + ?b - ?a] => replace (a + b - a) with b by omega
-  end; omega.
-Qed.
-
-Lemma expr_refs_renumber f e j :
-  expr_refs (renumber_expr f e) j <->
-  exists i, f i = j /\ expr_refs e i.
-Proof.
-  destruct e; rewrite renumber_expr_renumber_bindings;
-    cbn [expr_refs].
-  rewrite length_renumber.
-  setoid_rewrite bindings_ref_renumber.
-  setoid_rewrite op_refs_renumber.
-  split.
-  - intros [(?&?&?)|(?&?&?)].
-    + eexists.
-      intuition eauto.
-    + match goal with
-      | H : offset_renumbering _ _ _ = _ |- _ => eapply offset_eq_inv in H
-      end.
-      eexists; intuition eauto.
+  Lemma renumber_renumber_expr (h g f : nat -> nat) e :
+    (forall x, h x = g (f x)) ->
+    renumber_expr h e = renumber_expr g (renumber_expr f e).
+  Proof.
+    intros Hh; destruct e.
+    repeat rewrite renumber_expr_renumber_bindings.
+    f_equal.
+    - eapply renumber_renumber_bindings; eauto.
+    - eapply renumber_renumber_op.
+      intros; rewrite length_renumber.
+      erewrite offset_renumbering_ext by eapply Hh.
+      cbv [offset_renumbering]; crush_deciders idtac.
       match goal with
-      | |- context[?a + (?b - ?a)] =>
-        replace (a + (b - a)) with b by omega
-      end; eauto.
-  - intros (?&?&[?|?]); eauto.
-    right.
-    eexists; split; eauto.
-    cbv [offset_renumbering].
-    let t :=
-        idtac; match goal with
-               | H : ?a + ?x = ?a + ?y |- _ =>
-                 assert (x = y) by omega; subst
-               end in crush_deciders t.
-Qed.
+      | H : ?a + ?b = ?a + ?c |- _ => assert (b = c) by omega
+      end;
+        subst; eauto.
+  Qed.
 
-Lemma renumber_id_ref r :
-  renumber_ref (fun x => x) r = r.
-Proof. induction r; cbn [renumber_ref]; congruence. Qed.
+  Lemma refs_renumber f r j :
+    refs (renumber_ref f r) j <-> exists i, f i = j /\ refs r i.
+  Proof.
+    induction r; cbn [renumber_ref refs];
+      intuition repeat match goal with
+                       | H : exists _, _ |- _ => destruct H as (?&<-&?)
+                       | _ => intuition eauto
+                       end.
+  Qed.
 
-Lemma renumber_id_op o :
-  renumber_op (fun x => x) o = o.
-Proof.
-  destruct o; cbn [renumber_op]; try rewrite renumber_id_ref; congruence.
-Qed.
+  Lemma op_refs_renumber f o j :
+    op_refs (renumber_op f o) j <-> exists i, f i = j /\ op_refs o i.
+  Proof.
+    destruct o; cbn [renumber_op op_refs];
+      intuition repeat match goal with
+                       | H : exists _, _ |- _ => destruct H as (?&<-&?)
+                       | H : _ |- _ => setoid_rewrite refs_renumber in H
+                       | _ => setoid_rewrite refs_renumber
+                       | _ => intuition eauto
+                       end.
+  Qed.
 
-Lemma renumber_id_bindings p :
-  renumber_bindings (fun x => x) p = p.
-Proof.
-  induction p; cbn [renumber_bindings]; eauto.
-  rewrite renumber_id_op.
-  erewrite renumber_bindings_ext by (eapply offset_id).
-  rewrite IHp; eauto.
-Qed.
+  Lemma bindings_ref_renumber f p j :
+    bindings_ref (renumber_bindings f p) j <->
+    exists i, f i = j /\ bindings_ref p i.
+  Proof.
+    revert f j; induction p; intros;
+      intuition repeat multimatch goal with
+                       | H : exists _, _ |- _ => destruct H as (?&<-&?)
+                       | H : _ |- _ => setoid_rewrite op_refs_renumber in H
+                       | _ => setoid_rewrite op_refs_renumber
+                       | _ => cbn [bindings_ref renumber_bindings] in *
+                       | _ => intuition eauto
+                       end.
+    - rewrite IHp in *;
+        repeat match goal with
+               | H : exists _, _ |- _ =>
+                 let x := fresh in
+                 destruct H as ([]&?&?);
+                   cbv [offset_renumbering optsub] in *
+               | _ => congruence
+               | _ => intuition eauto
+               end.
+    - rewrite IHp;
+        right; eexists (S _); cbv [offset_renumbering optsub]; eauto.
+  Qed.
 
-Lemma renumber_id_expr e :
-  renumber_expr (fun x => x) e = e.
-Proof.
-  destruct e; rewrite renumber_expr_renumber_bindings.
-  rewrite renumber_id_bindings.
-  erewrite renumber_op_ext by (eapply offset_id);
-    rewrite renumber_id_op; eauto.
-Qed.
+  Lemma offset_eq_inv a f i j :
+    offset_renumbering a f i = a + j ->
+    i >= a /\ f (i - a) = j.
+  Proof.
+    cbv [offset_renumbering]; crush_deciders subst.
+    match goal with
+    | |- context[?a + ?b - ?a] => replace (a + b - a) with b by omega
+    end; omega.
+  Qed.
 
-Lemma commute_many ctxt (ctx : interp_type ctxt)
-      (o : operation) (p : list operation)
-      tk (ks : nat -> forall ctxt, interp_type ctxt -> M tk) :
-  ~bindings_ref p 0 ->
-  (forall j,
-      j < length p ->
-      continuation_renumbered
-        (offset_renumbering
-           j (fun n => match n with
-                       | 0 => 1
-                       | 1 => 0
-                       | _ => n
-                       end)) tk (ks (S j)) (ks j)) ->
-  Mequiv (interp_bindings ctxt ctx (o :: p) tk (ks (length p)))
-         (interp_bindings ctxt ctx
-                          ((renumber_bindings pred p)
-                             ++ renumber_op (plus (length p)) o :: nil)
-                          tk (ks 0)).
-Proof.
-  remember (length p) as lenp.
-  revert ctxt ctx o p Heqlenp;
-    induction lenp;
-    intros ctxt ctx o p Heqlenp Hp Hks;
-    destruct p as [|o' p]; try (cbn [length] in Heqlenp; congruence).
-  - cbn [interp_bindings renumber_bindings length plus].
+  Lemma expr_refs_renumber f e j :
+    expr_refs (renumber_expr f e) j <->
+    exists i, f i = j /\ expr_refs e i.
+  Proof.
+    destruct e; rewrite renumber_expr_renumber_bindings;
+      cbn [expr_refs].
+    rewrite length_renumber.
+    setoid_rewrite bindings_ref_renumber.
+    setoid_rewrite op_refs_renumber.
+    split.
+    - intros [(?&?&?)|(?&?&?)].
+      + eexists.
+        intuition eauto.
+      + match goal with
+        | H : offset_renumbering _ _ _ = _ |- _ => eapply offset_eq_inv in H
+        end.
+        eexists; intuition eauto.
+        match goal with
+        | |- context[?a + (?b - ?a)] =>
+          replace (a + (b - a)) with b by omega
+        end; eauto.
+    - intros (?&?&[?|?]); eauto.
+      right.
+      eexists; split; eauto.
+      cbv [offset_renumbering].
+      crush_deciders (idtac; match goal with
+                             | H : ?a + ?x = ?a + ?y |- _ =>
+                               assert (x = y) by omega; subst
+                             end).
+  Qed.
+
+  Lemma renumber_id_ref r :
+    renumber_ref (fun x => x) r = r.
+  Proof. induction r; cbn [renumber_ref]; congruence. Qed.
+
+  Lemma renumber_id_op o :
+    renumber_op (fun x => x) o = o.
+  Proof.
+    destruct o; cbn [renumber_op]; try rewrite renumber_id_ref; congruence.
+  Qed.
+
+  Lemma renumber_id_bindings p :
+    renumber_bindings (fun x => x) p = p.
+  Proof.
+    induction p; cbn [renumber_bindings]; eauto.
     rewrite renumber_id_op.
-    reflexivity.
-  - inversion Heqlenp; clear Heqlenp.
-    subst lenp.
-    cbn [bindings_ref] in *.
-    replace (o :: o' :: p) with ((o :: o' :: nil) ++ p)
-      by (eapply app_comm_cons).
-    rewrite interp_bindings_app.
-    etransitivity.
-    {
-      eapply commute_ops.
-      - cbn [bindings_ref] in Hp; eauto.
-      - eapply interp_renumbered_bindings.
-        eapply Hks; eauto.
-    }
+    erewrite renumber_bindings_ext by (eapply offset_id).
+    rewrite IHp; eauto.
+  Qed.
 
-    cbn [renumber_bindings length interp_bindings app] in IHlenp |- *.
+  Lemma renumber_id_expr e :
+    renumber_expr (fun x => x) e = e.
+  Proof.
+    destruct e; rewrite renumber_expr_renumber_bindings.
+    rewrite renumber_id_bindings.
+    erewrite renumber_op_ext by (eapply offset_id);
+      rewrite renumber_id_op; eauto.
+  Qed.
+
+  Lemma commute_many ctxt (ctx : interp_type ctxt)
+        (o : op) (p : list op)
+        tk (ks : nat -> forall ctxt, interp_type ctxt -> M tk) :
+    ~bindings_ref p 0 ->
+    (forall j,
+        j < length p ->
+        continuation_renumbered
+          (offset_renumbering
+             j (fun n => match n with
+                         | 0 => 1
+                         | 1 => 0
+                         | _ => n
+                         end)) tk (ks (S j)) (ks j)) ->
+    Mequiv (interp_bindings ctxt ctx (o :: p) tk (ks (length p)))
+           (interp_bindings ctxt ctx
+                            ((renumber_bindings pred p)
+                               ++ renumber_op (plus (length p)) o :: nil)
+                            tk (ks 0)).
+  Proof.
+    remember (length p) as lenp.
+    revert ctxt ctx o p Heqlenp;
+      induction lenp;
+      intros ctxt ctx o p Heqlenp Hp Hks;
+      destruct p as [|o' p]; try (cbn [length] in Heqlenp; congruence).
+    - cbn [interp_bindings renumber_bindings length plus].
+      rewrite renumber_id_op.
+      reflexivity.
+    - inversion Heqlenp; clear Heqlenp.
+      subst lenp.
+      cbn [bindings_ref] in *.
+      replace (o :: o' :: p) with ((o :: o' :: nil) ++ p)
+        by (eapply app_comm_cons).
+      rewrite interp_bindings_app.
+      etransitivity.
+      {
+        eapply commute_ops.
+        - cbn [bindings_ref] in Hp; eauto.
+        - eapply interp_renumbered_bindings.
+          eapply Hks; eauto.
+      }
+
+      cbn [renumber_bindings length interp_bindings app] in IHlenp |- *.
+      step_Mequiv.
+
+      etransitivity.
+      {
+        eapply IHlenp; eauto.
+        - rewrite length_renumber; eauto.
+        - setoid_rewrite bindings_ref_renumber.
+          intros ([|[]]&?&?); intuition congruence.
+      }
+
+      replace (renumber_op (plus (S (length p))) o) with
+          (renumber_op (plus (length p)) (renumber_op S o)) by
+          (erewrite <-renumber_renumber_op; eauto; intros; omega).
+      erewrite <-renumber_renumber_bindings by (intros; reflexivity).
+      rewrite renumber_bindings_ext_relevant with
+          (f' := (offset_renumbering 1 pred)); try reflexivity.
+      intros [|[]] ?; intuition idtac.
+  Qed.
+
+  Definition continuation_equiv tk
+             (k k' : forall ctxt, interp_type ctxt -> M tk) :=
+    forall ctxt ctx, Mequiv (k ctxt ctx) (k' ctxt ctx).
+
+  Local Instance interp_bindings_Mequiv ctxt ctx p tk :
+    Proper (continuation_equiv tk ==> Mequiv)
+           (interp_bindings ctxt ctx p tk).
+  Proof.
+    revert ctxt ctx; induction p;
+      cbn [interp_bindings]; intros ctxt ctx k k' ?; eauto.
     step_Mequiv.
+    eapply IHp; eauto.
+  Qed.
 
-    etransitivity.
-    {
-      eapply IHlenp; eauto.
-      - rewrite length_renumber; eauto.
-      - setoid_rewrite bindings_ref_renumber.
-        intros ([|[]]&?&?); intuition congruence.
-    }
+  Ltac crush_Mequiv :=
+    repeat multimatch goal with
+           | |- Mequiv (interp_bindings _ _ _ _ _)
+                       (interp_bindings _ _ _ _ _) =>
+             eapply interp_bindings_Mequiv; intros ??
+           | |- context[interp_bindings _ _ (_ ++ _) _ _] =>
+             rewrite interp_bindings_app
+           | |- context[Mbind (interp_bindings _ _ _ _ _) _] =>
+             rewrite bind_interp_bindings
+           | |- _ => cbn [interp_bindings]
+           | |- _ => step_Mequiv
+           end.
 
-    replace (renumber_op (plus (S (length p))) o) with
-        (renumber_op (plus (length p)) (renumber_op S o)) by
-        (erewrite <-renumber_renumber_op; eauto; intros; omega).
-    erewrite <-renumber_renumber_bindings by (intros; reflexivity).
-    rewrite renumber_bindings_ext_relevant with
-        (f' := (offset_renumbering 1 pred)); try reflexivity.
-    intros [|[]] ?; intuition idtac.
-Qed.
+  Definition cycle_to_here_renumbering (from j : nat) : nat :=
+    if j =? from
+    then 0
+    else if j <? from
+         then S j
+         else j.
 
-Definition continuation_equiv tk
-           (k k' : forall ctxt, interp_type ctxt -> M tk) :=
-  forall ctxt ctx, Mequiv (k ctxt ctx) (k' ctxt ctx).
+  Definition cycle (from to j : nat) : nat :=
+    if j =? from
+    then to
+    else if (to <=? j) && (j <? from)
+         then S j
+         else j.
 
-Local Instance interp_bindings_Mequiv ctxt ctx p tk :
-  Proper (continuation_equiv tk ==> Mequiv)
-         (interp_bindings ctxt ctx p tk).
-Proof.
-  revert ctxt ctx; induction p;
-    cbn [interp_bindings]; intros ctxt ctx k k' ?; eauto.
-  step_Mequiv.
-  eapply IHp; eauto.
-Qed.
-
-Ltac crush_Mequiv :=
-  repeat multimatch goal with
-         | |- Mequiv (interp_bindings _ _ _ _ _)
-                     (interp_bindings _ _ _ _ _) =>
-           eapply interp_bindings_Mequiv; intros ??
-         | |- context[interp_bindings _ _ (_ ++ _) _ _] =>
-           rewrite interp_bindings_app
-         | |- context[Mbind (interp_bindings _ _ _ _ _) _] =>
-           rewrite bind_interp_bindings
-         | |- _ => cbn [interp_bindings]
-         | |- _ => step_Mequiv
-         end.
-
-Definition cycle_to_here_renumbering (from j : nat) : nat :=
-  if j =? from
-  then 0
-  else if j <? from
-       then S j
-       else j.
-
-Definition cycle (from to j : nat) : nat :=
-  if j =? from
-  then to
-  else if (to <=? j) && (j <? from)
-       then S j
-       else j.
-
-Lemma cycle_trivial n j :
-  cycle n n j = j.
-Proof.
-  cbv [cycle].
-  crush_deciders idtac.
-Qed.
-
-Lemma offset_cycle a b c j :
-  offset_renumbering b (cycle a c) j =
-  cycle (a + b) (c + b) j.
-Proof.
-  cbv [offset_renumbering cycle].
-  let t := (cbn [andb]) in crush_deciders t.
-Qed.
-
-Lemma cycle_S from to :
-  to < from ->
-  forall i,
-    cycle from to i =
-    offset_renumbering to
-                       (fun n => match n with
-                                 | 0 => 1
-                                 | 1 => 0
-                                 | _ => n
-                                 end)
-                       (cycle from (S to) i).
-Proof.
-  cbv [cycle offset_renumbering].
-  let t := (cbn [andb] in * ) in
-  crush_deciders t;
-    repeat match goal with
-           | |- context[match ?x with _ => _ end] => destruct x
-           end;
+  Lemma cycle_trivial n j :
+    cycle n n j = j.
+  Proof.
+    cbv [cycle].
     crush_deciders idtac.
-Qed.
+  Qed.
 
-Definition cycle_expr_continuation ncommute e t j ctxt ctx :=
-  interp_expr_cast ctxt ctx
-                   (renumber_expr (cycle ncommute j) e)
-                   t.
+  Lemma offset_cycle a b c j :
+    offset_renumbering b (cycle a c) j =
+    cycle (a + b) (c + b) j.
+  Proof.
+    cbv [offset_renumbering cycle].
+    crush_deciders cbn [andb].
+  Qed.
 
-Lemma cycle_continuation_renumbered ncommute e t j :
-  j < ncommute ->
-  continuation_renumbered
-    (offset_renumbering j
-                        (fun n : nat => match n with
-                                        | 0 => 1
-                                        | 1 => 0
-                                        | S (S _) => n
-                                        end)) t
-    (cycle_expr_continuation ncommute e t (S j))
-    (cycle_expr_continuation ncommute e t j).
-Proof.
-  intros.
-  cbv [cycle_expr_continuation].
-  erewrite (renumber_expr_ext
-              _ _ _
-              ltac:(eapply (cycle_S ncommute j
-                                                ltac:(eauto)))).
-  rewrite renumber_renumber_expr with
-      (h :=
-         fun i =>
-           offset_renumbering j
-                              (fun n =>
-                                 match n with
-                                 | 0 => 1
-                                 | 1 => 0
-                                 | S (S _) => n
-                                 end)
-                              (cycle ncommute (S j) i))
-      (g := offset_renumbering j
-                               (fun n : nat => match n with
-                                               | 0 => 1
-                                               | 1 => 0
-                                               | S (S _) => n
-                                               end))
-      (f := cycle ncommute (S j))
-    by reflexivity.
-  eapply interp_renumbered_expr.
-Qed.
-
-Definition context_omits (f : nat -> option nat)
-           ctxt (ctx : interp_type ctxt)
-           ctxt' (ctx' : interp_type ctxt') : Prop :=
-  forall i t,
-    match f i with
-    | Some j => lookup ctxt' ctx' j t = lookup ctxt ctx i t
-    | None => True
-    end.
-
-Definition continuation_omits (f : nat -> option nat)
-           tk (k k' : forall ctxt, interp_type ctxt -> M tk) : Prop :=
-  forall ctxt (ctx : interp_type ctxt) ctxt' (ctx' : interp_type ctxt'),
-    context_omits f ctxt ctx ctxt' ctx' ->
-    Mequiv (k ctxt ctx) (k' ctxt' ctx').
-
-Lemma assoc_op ctxt (ctx : interp_type ctxt) o
-      tm (m : interp_type (op_type o * ctxt) -> M tm)
-      tk (k k' : forall ctxt, interp_type ctxt -> M tk) :
-  continuation_omits (fun n =>
-                        match n with
-                        | 0 => Some 0
-                        | 1 => None
-                        | S n => Some n
-                        end) tk k k' ->
-  Mequiv
-    (Mbind (interp_op_silent ctxt ctx o)
-           (fun x =>
-              Mbind (m (x, ctx))
-                    (fun y => k (tm * (op_type o * ctxt))%etype
-                                (y, (x, ctx)))))
-    (Mbind (Mbind (interp_op_silent ctxt ctx o)
-                  (fun x => m (x, ctx)))
-           (fun y => k' (tm * ctxt)%etype
-                        (y, ctx))).
-Proof.
-  intros Hkk'; crush_Mequiv; eapply Hkk'.
-  intros [|[|[]]] ?; reflexivity.
-Qed.
-
-Definition offset_omission offset f n :=
-  match n -? offset with
-  | Some k => match f k with
-              | Some k' => Some (offset + k')
-              | None => None
-              end
-  | None => Some n
-  end.
-
-Lemma assoc_many ctxt (ctx : interp_type ctxt) p
-      tm (m : forall ctxt, interp_type ctxt -> M tm)
-      tk (ks : nat -> forall ctxt, interp_type ctxt -> M tk) :
-  (forall j,
-      j < length p ->
-      continuation_omits
-        (fun n => match n with
-                  | 0 => Some 0
-                  | 1 => None
-                  | S n => Some n
-                  end) tk (ks (S j)) (ks j)) ->
-  Mequiv
-    (interp_bindings
-       ctxt ctx p tk
-       (fun ctxt ctx =>
-          Mbind (m ctxt ctx)
-                (fun y => (ks (length p) (tm * ctxt)%etype (y, ctx)))))
-    (Mbind (interp_bindings ctxt ctx p tm m)
-           (fun y => ks 0 (tm * ctxt)%etype (y, ctx))).
-Proof.
-  intros Hk.
-  rewrite bind_interp_bindings.
-  revert Hk m;
-    pattern p; revert p; eapply rev_ind; [|intros o p IHp];
-      intros Hk m.
-  { reflexivity. }
-  listrew.
-  specialize (IHp (ltac:(intros; eapply Hk; omega))
-                  (fun _ ctx =>
-                     Mbind (interp_op_silent _ ctx o)
-                           (fun x => m (_ * _)%etype (x, ctx)))).
-  specialize (Hk (length p) ltac:(omega)).
-  repeat rewrite interp_bindings_app; cbn [interp_bindings].
-  etransitivity; [|etransitivity]; [|eapply IHp|]; clear IHp;
-    [|solve [crush_Mequiv]].
-  eapply interp_bindings_Mequiv; intros ??.
-  eapply assoc_op; eauto.
-Qed.
-
-Definition ref_omits (f : nat -> option nat) r :=
-  forall i, refs r i -> f i <> None.
-
-Definition op_omits (f : nat -> option nat) o :=
-  forall i, op_refs o i -> f i <> None.
-
-Definition bindings_omit (f : nat -> option nat) p :=
-  forall i, bindings_ref p i -> f i <> None.
-
-Definition expr_omits (f : nat -> option nat) e :=
-  forall i, expr_refs e i -> f i <> None.
-
-Definition expr_omits_range n e :=
-  forall i, expr_refs e i -> i = 0 \/ S n <= i.
-
-Definition expr_omits_rangeb n e :=
-  expr_all_refsb (fun i => (i =? 0) ||
-                           (S n <=? i)) e.
-
-Lemma expr_omits_rangeb_correct n e :
-  expr_omits_rangeb n e = true -> expr_omits_range n e.
-Proof.
-  cbv [expr_omits_rangeb expr_omits_range]; intros He ??.
-  eapply expr_all_refsb_correct in He; eauto.
-  revert He; crush_deciders idtac.
-Qed.
-
-Definition silence_omission (f : nat -> option nat) j :=
-  match f j with
-  | Some x => x
-  | None => 0
-  end.
-
-Lemma lookup_omitted_ref ctxt ctx ctxt' ctx' f r t :
-  context_omits f ctxt ctx ctxt' ctx' ->
-  ref_omits f r ->
-  lookup_ref ctxt' ctx' (renumber_ref (silence_omission f) r) t =
-  lookup_ref ctxt ctx r t.
-Proof.
-  cbv [context_omits ref_omits silence_omission].
-  intros Hctx Hr.
-  revert t; induction r as [i|r1 IHr1 r2 IHr2]; intros t;
-    cbn [lookup_ref renumber_ref refs] in *.
-  - specialize (Hctx i t).
-    specialize (Hr _ ltac:(eauto)).
-    destruct (f i); congruence.
-  - destruct t; eauto.
-    erewrite IHr1, IHr2 by eauto; reflexivity.
-Qed.
-
-Lemma context_omits_1 f ctxt ctx ctxt' ctx' t (x : interp_type t) :
-  context_omits f ctxt ctx ctxt' ctx' ->
-  context_omits (offset_omission 1 f) (_ * _) (x, ctx) (_ * _) (x, ctx').
-Proof.
-  cbv [context_omits offset_omission]; intros Hf.
-  let t := (repeat multimatch goal with
-                   | |- context[f ?x] => specialize (Hf x); destruct (f x)
-                   | _ => change (1 + ?y) with (S y)
-                   | H : ?x < 1 |- _ => assert (x = 0) by omega; clear H
-                   | _ => cbn [lookup]
-                   | _ => subst
-                   end) in crush_deciders t.
-Qed.
-
-Lemma interp_omitted_op f o tk
-      (k k' : forall ctxt, interp_type ctxt -> M tk) :
-  op_omits f o ->
-  continuation_omits (offset_omission 1 f) tk k k' ->
-  continuation_omits
-    f tk
-    (fun _ ctx =>
-       (Mbind (interp_op_silent _ ctx o)
-              (fun x => k (_ * _)%etype (x, ctx))))
-    (fun _ ctx =>
-       (Mbind
-          (interp_op_silent _ ctx
-                            (renumber_op (silence_omission f) o))
-          (fun x => k' (_ * _)%etype (x, ctx)))).
-Proof.
-  intros ? Hk ?????.
-  destruct o; cbn [renumber_op op_type op_refs] in *;
-    (step_Mequiv; [..|eapply Hk; eapply context_omits_1; eauto]);
-      cbv [interp_op_silent interp_op];
-      erewrite lookup_omitted_ref by eauto;
-      reflexivity.
-Qed.
-
-Lemma interp_omitted_op_no_ctx f o tk
-      (k k' : forall t, interp_type t -> M tk) :
-  op_omits f o ->
-  (forall t x, Mequiv (k t x) (k' t x)) ->
-  continuation_omits
-    f tk
-    (fun ctxt ctx =>
-       (Mbind (interp_op_silent ctxt ctx o)
-              (fun x => k (op_type o) x)))
-    (fun ctxt ctx =>
-       (Mbind
-          (interp_op_silent ctxt ctx
-                            (renumber_op (silence_omission f) o))
-          (fun x => k'
-                      (op_type (renumber_op (silence_omission f) o)) x))).
-Proof.
-  intros ? Hk ?????.
-  destruct o; cbn [renumber_op op_type op_refs] in *;
-    (step_Mequiv; [..|eapply Hk; eapply context_omits_1; eauto]);
-      cbv [interp_op_silent interp_op];
-      erewrite lookup_omitted_ref by eauto;
-      reflexivity.
-Qed.
-
-Lemma offset_omission_0 f i : offset_omission 0 f i = f i.
-Proof.
-  cbv [offset_omission].
-  crush_deciders idtac.
-  subst; cbn [plus].
-  destruct (f _); eauto.
-Qed.
-
-Lemma context_omits_ext f1 f2 ctxt ctx ctxt' ctx' :
-  (forall i, f1 i = f2 i) ->
-  context_omits f1 ctxt ctx ctxt' ctx' <->
-  context_omits f2 ctxt ctx ctxt' ctx'.
-Proof. intros H; cbv [context_omits]; setoid_rewrite H; reflexivity. Qed.
-
-Lemma continuation_omits_ext f1 f2 tk k k' :
-  (forall i, f1 i = f2 i) ->
-  continuation_omits f1 tk k k' ->
-  continuation_omits f2 tk k k'.
-Proof.
-  intros H Hk ?????.
-  eapply Hk.
-  erewrite context_omits_ext; eauto.
-Qed.
-
-Local Instance continuation_omits_Mequiv f tk :
-  Proper
-    (forall_relation
-       (fun ctxt => pointwise_relation (interp_type ctxt) Mequiv) ==>
-     forall_relation
-       (fun ctxt => pointwise_relation (interp_type ctxt) Mequiv) ==>
-     iff) (continuation_omits f tk).
-Proof.
-  cbv [Proper respectful forall_relation pointwise_relation Basics.impl].
-  cbv [continuation_omits].
-  intros; split; intros.
-  - etransitivity; [symmetry; eauto|];
-      etransitivity; [|eauto]; eauto.
-  - etransitivity; [|symmetry; eauto];
-      etransitivity; [eauto|]; eauto.
-Qed.
-
-Lemma bindings_omit_app_invl f p1 p2 :
-  bindings_omit f (p1 ++ p2) -> bindings_omit f p1.
-Proof.
-  cbv [bindings_omit].
-  intros Ha.
-  setoid_rewrite bindings_ref_app in Ha.
-  intuition eauto.
-Qed.
-
-Lemma bindings_omit_app_invr f p1 p2 :
-  bindings_omit f (p1 ++ p2) ->
-  bindings_omit (offset_omission (length p1) f) p2.
-Proof.
-  cbv [bindings_omit offset_omission].
-  intros Ha.
-  setoid_rewrite bindings_ref_app in Ha.
-  intros i ?.
-  crush_deciders idtac.
-  match goal with
-  | _ : context[f ?x] |- _ => specialize (Ha x)
-  end.
-  subst.
-  destruct (f _); eauto; congruence.
-Qed.
-
-Lemma offset_silence n f i :
-  offset_omission n f i <> None ->
-  offset_renumbering n (silence_omission f) i =
-  silence_omission (offset_omission n f) i.
-Proof.
-  intros.
-  cbv [offset_renumbering silence_omission offset_omission] in *.
-  let t := (destruct (f _)) in crush_deciders t.
-Qed.
-
-Lemma offset_offset_omission a b f i :
-  offset_omission (a + b) f i =
-  offset_omission a (offset_omission b f) i.
-Proof.
-  cbv [offset_omission].
-  crush_deciders idtac.
-  subst.
-  match goal with
-  | H : ?x + ?y + ?z = ?x + (?y + ?z') |- _ =>
-    assert (z = z') by omega; clear H; subst
-  end.
-  destruct (f _); f_equal; omega.
-Qed.
-
-Lemma interp_omitted_bindings f p
-      tk (k k' : forall ctxt : type, interp_type ctxt -> M tk) :
-  bindings_omit f p ->
-  continuation_omits (offset_omission (length p) f) tk k k' ->
-  continuation_omits
-    f tk
-    (fun ctxt ctx => interp_bindings ctxt ctx p tk k)
-    (fun ctxt ctx =>
-       interp_bindings ctxt ctx
-                       (renumber_bindings (silence_omission f) p) tk k').
-Proof.
-  revert tk k k'.
-  pattern p; revert p; eapply rev_ind;
-    cbn [renumber_bindings interp_bindings length offset_renumbering
-                           optsub plus]; [|intros o p IHp];
-      intros tk k k' Hp Hkk'.
-  { eapply continuation_omits_ext in Hkk';
-      try solve [eapply offset_omission_0].
-      eapply Hkk'. }
-  rewrite renumber_bindings_app.
-  cbn [renumber_bindings].
-  setoid_rewrite interp_bindings_app.
-  pose proof (bindings_omit_app_invl _ _ _ Hp).
-  pose proof (bindings_omit_app_invr _ _ _ Hp).
-  cbv [bindings_omit] in *; cbn [bindings_ref] in *.
-  clear Hp.
-  eapply IHp; eauto; cbn [interp_bindings].
-  intros ?????.
-  rewrite renumber_op_ext_relevant with
-      (f := (offset_renumbering (length p) (silence_omission f)))
-      (f' := (silence_omission (offset_omission (length p) f)))
-      by (eauto using offset_silence).
-
-  eapply interp_omitted_op; try solve [eauto |
-                                       cbv [op_omits]; intuition eauto].
-  listrew.
-  eapply continuation_omits_ext;
-    try eapply offset_offset_omission; eauto.
-Qed.
-
-Lemma interp_omitted_expr f t (e : expr) :
-  expr_omits f e ->
-  continuation_omits
-    f t
-    (fun ctxt ctx => interp_expr_cast ctxt ctx e t)
-    (fun ctxt ctx =>
-       interp_expr_cast ctxt ctx (renumber_expr (silence_omission f) e) t).
-Proof.
-  intros He ?????.
-  destruct e as [p o].
-  cbv [expr_omits expr_refs] in *.
-  rewrite renumber_expr_renumber_bindings.
-  erewrite renumber_op_ext_relevant; cycle 1.
-  { intros i ?.
-    eapply offset_silence.
-    cbv [offset_omission].
-    crush_deciders subst.
-    match goal with
-    | _ : context[f ?x] |- _ => specialize (He x)
-    end.
-    destruct (f _); eauto; congruence. }
-  cbv [interp_expr_cast interp_expr].
-  setoid_rewrite bind_interp_bindings.
-  eapply interp_omitted_bindings;
-    try solve [eauto | cbv [bindings_omit]; intuition eauto].
-  refine (interp_omitted_op_no_ctx
-            _ _ _
-            (fun _ x => Mret (cast t x))
-            (fun _ x => Mret (cast t x))
-            _ _).
-  { intros i ?.
-    cbv [offset_omission].
-    crush_deciders subst.
+  Lemma cycle_S from to :
+    to < from ->
+    forall i,
+      cycle from to i =
+      offset_renumbering to
+                         (fun n => match n with
+                                   | 0 => 1
+                                   | 1 => 0
+                                   | _ => n
+                                   end)
+                         (cycle from (S to) i).
+  Proof.
+    cbv [cycle offset_renumbering].
     intros.
-    match goal with
-    | _ : context[f ?x] |- _ => specialize (He x)
+    crush_deciders (cbn [andb] in * );
+      repeat match goal with
+             | |- context[match ?x with _ => _ end] => destruct x
+             end;
+      crush_deciders idtac.
+  Qed.
+
+  Definition cycle_expr_continuation ncommute e t j ctxt ctx :=
+    interp_expr_cast ctxt ctx
+                     (renumber_expr (cycle ncommute j) e)
+                     t.
+
+  Lemma cycle_continuation_renumbered ncommute e t j :
+    j < ncommute ->
+    continuation_renumbered
+      (offset_renumbering j
+                          (fun n : nat => match n with
+                                          | 0 => 1
+                                          | 1 => 0
+                                          | S (S _) => n
+                                          end)) t
+      (cycle_expr_continuation ncommute e t (S j))
+      (cycle_expr_continuation ncommute e t j).
+  Proof.
+    intros.
+    cbv [cycle_expr_continuation].
+    erewrite (renumber_expr_ext
+                _ _ _
+                ltac:(eapply (cycle_S ncommute j
+                                      ltac:(eauto)))).
+    rewrite renumber_renumber_expr with
+        (h :=
+           fun i =>
+             offset_renumbering j
+                                (fun n =>
+                                   match n with
+                                   | 0 => 1
+                                   | 1 => 0
+                                   | S (S _) => n
+                                   end)
+                                (cycle ncommute (S j) i))
+        (g := offset_renumbering j
+                                 (fun n : nat => match n with
+                                                 | 0 => 1
+                                                 | 1 => 0
+                                                 | S (S _) => n
+                                                 end))
+        (f := cycle ncommute (S j))
+      by reflexivity.
+    eapply interp_renumbered_expr.
+  Qed.
+
+  Definition context_omits (f : nat -> option nat)
+             ctxt (ctx : interp_type ctxt)
+             ctxt' (ctx' : interp_type ctxt') : Prop :=
+    forall i t,
+      match f i with
+      | Some j => lookup ctxt' ctx' j t = lookup ctxt ctx i t
+      | None => True
+      end.
+
+  Definition continuation_omits (f : nat -> option nat)
+             tk (k k' : forall ctxt, interp_type ctxt -> M tk) : Prop :=
+    forall ctxt (ctx : interp_type ctxt) ctxt' (ctx' : interp_type ctxt'),
+      context_omits f ctxt ctx ctxt' ctx' ->
+      Mequiv (k ctxt ctx) (k' ctxt' ctx').
+
+  Lemma assoc_op ctxt (ctx : interp_type ctxt) o
+        tm (m : interp_type (op_type o * ctxt) -> M tm)
+        tk (k k' : forall ctxt, interp_type ctxt -> M tk) :
+    continuation_omits (fun n =>
+                          match n with
+                          | 0 => Some 0
+                          | 1 => None
+                          | S n => Some n
+                          end) tk k k' ->
+    Mequiv
+      (Mbind (interp_op_silent ctxt ctx o)
+             (fun x =>
+                Mbind (m (x, ctx))
+                      (fun y => k (tm * (op_type o * ctxt))%etype
+                                  (y, (x, ctx)))))
+      (Mbind (Mbind (interp_op_silent ctxt ctx o)
+                    (fun x => m (x, ctx)))
+             (fun y => k' (tm * ctxt)%etype
+                          (y, ctx))).
+  Proof.
+    intros Hkk'; crush_Mequiv; eapply Hkk'.
+    intros [|[|[]]] ?; reflexivity.
+  Qed.
+
+  Definition offset_omission offset f n :=
+    match n -? offset with
+    | Some k => match f k with
+                | Some k' => Some (offset + k')
+                | None => None
+                end
+    | None => Some n
     end.
-    destruct (f _); eauto; congruence. }
-  reflexivity.
-Qed.
 
-Definition shift from to i := if i <? from
-                              then 0
-                              else i - from + to.
-
-Definition shift_expr_continuation e t total j ctxt ctx :=
-  interp_expr_cast ctxt ctx (renumber_expr (shift (S (total - j)) 1) e) t.
-
-Lemma shift_S from i :
-  shift (S from) 1 i =
-  (silence_omission (fun n => match n with
-                              | 0 => Some 0
-                              | 1 => None
-                              | S n => Some n
-                              end))
-    (shift from 1 i).
-Proof.
-  cbv [shift silence_omission].
-  let t :=
-      idtac; multimatch goal with
-             | |- context[match ?x with _ => _ end] =>
-               lazymatch x with
-               | context[match _ with _ => _ end] => fail
-               | _ => idtac
-               end;
-               let x' := fresh "x" in remember x as x'; destruct x'
-             end in
-  crush_deciders t.
-Qed.
-
-Lemma shift_continuation_omitted e t total j :
-  j < total ->
-  expr_omits_range total e ->
-  continuation_omits
-    (fun n => match n with
-              | 0 => Some 0
-              | 1 => None
-              | S n => Some n
-              end) t
-    (shift_expr_continuation e t total (S j))
-    (shift_expr_continuation e t total j).
-Proof.
-  cbv [shift_expr_continuation]; intros ? He.
-  replace (S (total - j)) with (S (S (total - S j))) by omega.
-  erewrite (renumber_expr_ext
-              _ _ _ ltac:(eapply (shift_S (S (total - S j))))).
-  rewrite renumber_renumber_expr with
-      (h := (fun i =>
-               silence_omission
-                 (fun n =>
-                    match n with
+  Lemma assoc_many ctxt (ctx : interp_type ctxt) p
+        tm (m : forall ctxt, interp_type ctxt -> M tm)
+        tk (ks : nat -> forall ctxt, interp_type ctxt -> M tk) :
+    (forall j,
+        j < length p ->
+        continuation_omits
+          (fun n => match n with
                     | 0 => Some 0
                     | 1 => None
                     | S n => Some n
-                    end) (shift (S (total - S j)) 1 i)))
-      (g := silence_omission
-              (fun n =>
-                 match n with
-                 | 0 => Some 0
-                 | 1 => None
-                 | S n => Some n
-                 end))
-      (f := (shift (S (total - S j)) 1))
-      by reflexivity.
-  eapply interp_omitted_expr.
-  cbv [expr_omits expr_omits_range].
-  intros i Hi.
-  eapply expr_refs_renumber in Hi; destruct Hi as (x&?&?).
-  subst.
-  enough (shift (S (total - S j)) 1 x <> 1) by
-      (destruct (shift (S (total - S j)) 1 x) as [|[|]]; congruence).
-  destruct e; cbv [expr_omits_range] in *.
-  specialize (He _ ltac:(eauto)).
-  cbv [shift].
-  destruct He; crush_deciders idtac.
-Qed.
-
-Lemma equiv_prefix l p o p' o' :
-  equiv (p, o) (p', o') ->
-  equiv (l ++ p, o) (l ++ p', o').
-Proof.
-  cbv [equiv equiv_under interp_expr_cast interp_expr].
-  intros H ???.
-  crush_Mequiv.
-  etransitivity; [|etransitivity]; [|eapply H|];
-    crush_Mequiv.
-Qed.
-
-Lemma shift_trivial i : shift 1 1 i = i.
-Proof. cbv [shift]; crush_deciders idtac. Qed.
-
-Lemma offset_1_shift from to i :
-  i = 0 \/ i > from ->
-  offset_renumbering 1 (shift from to) i = shift (S from) (S to) i.
-Proof. cbv [shift offset_renumbering]; crush_deciders idtac. Qed.
-
-Lemma shift_shift a b c i :
-  b <> 0 ->
-  shift b c (shift a b i) = shift a c i.
-Proof.
-  cbv [shift]; crush_deciders idtac.
-Qed.
-
-Lemma shift_expr_continuation_shift t ctxt ctx s so n n' :
-  expr_omits_range n (s, so) ->
-  Mequiv
-    (shift_expr_continuation (s, so) t n 0 ctxt ctx)
-    (shift_expr_continuation
-       (renumber_expr (offset_renumbering 1 (shift n n')) (s, so))
-       t n' 0 ctxt ctx).
-Proof.
-  intros.
-  erewrite (renumber_expr_ext_relevant
-              _ _ _ ltac:(intros; rewrite offset_1_shift; eauto)).
-  cbv [shift_expr_continuation].
-  repeat (evar (x : nat); subst x; replace (?x - 0) with (?x) by omega).
-  erewrite <-renumber_renumber_expr.
-  - reflexivity.
-  - intros.
-    rewrite shift_shift; omega.
-Qed.
-
-Lemma omit_range_shift n n' e :
-  expr_omits_range n e ->
-  expr_omits_range n' (renumber_expr (offset_renumbering 1 (shift n n')) e).
-Proof.
-  cbv [expr_omits_range].
-  setoid_rewrite expr_refs_renumber.
-  intros H ?(?&?&?); subst.
-  specialize (H _ ltac:(eauto)).
-  cbv [offset_renumbering shift]; crush_deciders idtac.
-Qed.
-
-Lemma equiv_suffix p o p' o' s so s' so' :
-  op_type o = op_type o' ->
-  expr_omits_range (length p) (s, so) ->
-  (s', so') = renumber_expr
-                (offset_renumbering 1 (shift (length p) (length p')))
-                (s, so) ->
-  equiv (p, o) (p', o') ->
-  equiv (p ++ o :: s, so) (p' ++ o' :: s', so').
-  intros ???.
-  intros Hpp'.
-  assert (expr_omits_range (length p') (s', so'))
-         by (replace (s', so'); eauto using omit_range_shift).
-  cbv [equiv equiv_under interp_expr_cast interp_expr].
-  intros.
-  crush_Mequiv.
-
-  etransitivity; etransitivity; [..|etransitivity];
-    [|
-     solve [eapply assoc_many
-              with (p := p)
-                   (m := (fun ctxt ctx => interp_op_silent ctxt ctx o))
-                   (ks := shift_expr_continuation (s, so) t
-                                                  (length p));
-            intros; eapply shift_continuation_omitted; eauto]
-     | |
-     solve [symmetry;
-            eapply assoc_many
-              with (p := p')
-                   (m := (fun ctxt ctx => interp_op_silent ctxt ctx o'))
-                   (ks := shift_expr_continuation (s', so') t
-                                                  (length p'));
-            intros; eapply shift_continuation_omitted; eauto]
-     |]; cycle 1;
-      [|cbv [shift_expr_continuation interp_expr_cast interp_expr];
-        replace (length _ - length _) with 0 by omega;
-        erewrite renumber_expr_ext by (eapply shift_trivial);
-        rewrite renumber_id_expr;
-        crush_Mequiv ..].
-
-  etransitivity; [|etransitivity];
-    [|eapply Mequiv_Mbind_cast
-             with
-               (c2 :=
-                  fun tx (x : interp_type tx) =>
-                    (shift_expr_continuation (s, so) t (length p) 0
-                                             (tx * ctxt) (x, ctx)))
-               (c2' :=
-                  fun tx (x : interp_type tx) =>
-                    (shift_expr_continuation (s', so') t (length p') 0
-                                             (tx * ctxt) (x, ctx)));
-      [eauto|eapply Hpp'|]|]; cycle 1;
-      [|solve [cbv [interp_expr_cast interp_expr expr_type];
-               crush_Mequiv] ..].
-  intros.
-  replace (s', so').
-  eapply shift_expr_continuation_shift; eauto.
-Qed.
-
-Module Rewriter.
-  Inductive error :=
-  | E_debug {t : Type} (_ : t)
-  | E_trace {t u : Type} (_ : t) (_ : u + error)
-  | E_todo (_ : string)
-  | E_msg (_ : string).
-
-  Local Notation ok := inl.
-  Local Notation raise := inr.
-  Definition err_bind {t1 t2} (a : t1 + error) (b : t1 -> t2 + error)
-    : t2 + error :=
-    match a with
-    | ok x => b x
-    | raise e => raise e
-    end.
-  Local Notation "x <-! a ; b" := (err_bind a (fun x => b))
-                                    (right associativity,
-                                     at level 100).
-  Local Notation "' x <-! a ; b" := (err_bind a (fun 'x => b))
-                                      (x strict pattern,
-                                       right associativity,
-                                       at level 100).
-
-  Section WithMap.
-    Context (map_operations : fmap.operations nat nat).
-    Local Notation map := (map_operations.(fmap.M)).
-    Local Notation empty := (map_operations.(fmap.empty)).
-    Local Notation add := (map_operations.(fmap.add)).
-    Local Notation find := (map_operations.(fmap.find)).
-    Local Notation fold_ac := (map_operations.(fmap.fold_ac)).
-
-    Definition op_matches (o1 o2 : operation) :=
-      match o1, o2 with
-      | op_unit, op_unit => true
-      | op_app c _, op_app c' _ =>
-        if const_eqb c c' then true else false
-      | op_retapp c _, op_retapp c' _ =>
-        if retconst_eqb c c' then true else false
-      | _, _ => false
-      end.
-
-    (* TODO
-     * - matching rewrite
-     *   + (normalize lemma by removing any unused bindings)
-     *   X find a match (inverse maps which line up program and lemma)
-     *   + (renumber the lemma's free variables)
-     *   X check that the match isn't captured by the program's tail
-     *   X generate a sequence of cycles
-     *   X check the legality of the cycles
-     *   X prove the cycle-checker correct
-     *   X run the cycles individually
-     *   X run the strict matcher
-     *     (could prove that it always succeeds but that would be hard)
-     *   X rewrite the lemma
-     * - reification
-     *   + reify to PHOAS first, then to flat structure
-     * - support for ret
-     *   + duplicating/deduplicating rets
-     * - support for free variables
-     *   + need to renumber them on both sides of the lemma to match the
-     *     program
-     * - support for unused bindings
-     *)
-
-    Definition update_maps_ind (lem2prog prog2lem : map) (li pi : nat)
-      : map * map + error :=
-      match find li lem2prog with
-      | Some pi' => if pi =? pi'
-                    then ok (lem2prog, prog2lem)
-                    else raise (E_msg "map_match: lem2prog mismatch")
-      | None =>
-        let lem2prog := add li pi lem2prog in
-        match find pi prog2lem with
-        | Some li' => if li =? li'
-                      then ok (lem2prog, prog2lem)
-                      else raise (E_msg "map_match: prog2lem mismatch")
-        | None =>
-          let prog2lem := add pi li prog2lem in
-          ok (lem2prog, prog2lem)
-        end
-      end.
-
-    Fixpoint update_maps_ref (loff poff : nat) (lem2prog prog2lem : map)
-             (lr pr : ref) {struct lr} :
-      map * map + error :=
-      match lr, pr with
-      | ref_index ln, ref_index pn =>
-        update_maps_ind lem2prog prog2lem (loff + ln) (poff + pn)
-      | ref_pair lr1 lr2, ref_pair pr1 pr2 =>
-        '(lem2prog, prog2lem) <-!
-         update_maps_ref loff poff lem2prog prog2lem lr1 pr1;
-          update_maps_ref loff poff lem2prog prog2lem lr2 pr2
-      | _, _ => raise (E_msg "map_match: ref mismatch")
-      end.
-
-    Definition update_maps_op
-               (lop pop : operation)
-               (loff poff : nat) (lem2prog prog2lem : map)
-      : map * map + error :=
-      match lop, pop with
-      | op_unit, op_unit => ok (lem2prog, prog2lem)
-      | op_app lc lr, op_app pc pr =>
-        if const_eqb lc pc
-        then update_maps_ref loff poff lem2prog prog2lem lr pr
-        else raise (E_msg "map_match: op const mismatch")
-      | op_retapp lc lr, op_retapp pc pr =>
-        if retconst_eqb lc pc
-        then update_maps_ref loff poff lem2prog prog2lem lr pr
-        else raise (E_msg "map_match: op retconst mismatch")
-      | _, _ => raise (E_msg "map_match: operation mismatch")
-      end.
-
-    (* iterate over lbinds, using the map found so far to index into
-     * pbinds.  lbinds gets shorter, pbinds stays the same.
-     * The "empty lem2prog entry" error occurs if the lemma has unused
-     * bindings; "bad lem2prog entry" occurs if the program refers to a
-     * free variable but that variable is not free in the lemma. *)
-    Fixpoint map_match'
-             (lbinds pbinds : list operation) (lhead phead : operation)
-             (loff poff : nat) (lem2prog prog2lem : map) {struct lbinds}
-      : map * map + error :=
-      '(lem2prog, prog2lem) <-!
-       update_maps_op lhead phead loff poff lem2prog prog2lem;
-        match lbinds with
-        | nil => ok (lem2prog, prog2lem)
-        | cons lhead lbinds =>
-          match find loff lem2prog with
-          | Some pi =>
-            match List.nth_error pbinds pi with
-            | Some phead => map_match' lbinds pbinds
-                                        lhead phead
-                                        (S loff) (S pi)
-                                        lem2prog prog2lem
-            | None => raise (E_msg "map_match: bad lem2prog entry")
-            end
-          | None => raise (E_msg "map_match: empty lem2prog entry")
-          end
-        end.
-
-    (* binds and lbinds are in reversed order from their usual order in
-     * expr.  returns lemma-to-program and program-to-lemma maps of de
-     * Bruijn indices relative to the head
-     *)
-    Definition map_match (lbinds pbinds : list operation)
-               (lhead phead : operation) : map * map + error :=
-      map_match' lbinds pbinds lhead phead 0 0 empty empty.
-
-    Definition check_no_capturing_tail (ptail : list operation)
-               (prog_end : operation)
-               (prog2lem : map) : unit + error :=
-      fold_ac _ (fun n _ acc =>
-                   _ <-! acc;
-                     if bindings_refb ptail (S n)
-                        || op_refsb prog_end (S (length ptail) + n)
-                     then raise (E_msg "check_no_capturing_tail: capture")
-                     else ok tt)
-              (ok tt) prog2lem.
-
-    Definition renumber_lem2prog (lem2prog : map) (pi li : nat) :=
-      fold_ac _ (fun lj pj lem2prog =>
-                   if pj =? pi
-                   then lem2prog
-                   else add lj (cycle pi li pj) lem2prog)
-              empty lem2prog.
-
-    Fixpoint generate_cycles' lem2prog (cycles : list (nat * nat))
-             (li : nat) (n : nat) :=
-      match n with
-      | 0 => ok cycles
-      | S n =>
-        match find li lem2prog with
-        | Some pi =>
-          if pi <? li
-          then raise (E_msg "generate_cycles: pi < li")
-          else generate_cycles' (renumber_lem2prog lem2prog pi li)
-                                ((pi, li) :: cycles)
-                                (S li) n
-        | None => raise (E_msg "generate_cycles: bad li")
-        end
-      end.
-
-    Definition generate_cycles lem2prog (len_lbinds : nat)
-      : list (nat * nat) + error :=
-      cycles <-! generate_cycles' lem2prog nil 0 len_lbinds;
-        ok (rev cycles).
-
-    Lemma generate_cycles'_correct lem2prog cycles li n :
-      Forall (fun '(from, to) => to <= from) cycles ->
-      match generate_cycles' lem2prog cycles li n with
-      | ok cycles => Forall (fun '(from, to) => to <= from) cycles
-      | raise _ => True
-      end.
-    Proof.
-      revert lem2prog cycles li; induction n;
-        intros lem2prog cycles li ?;
-               cbn [generate_cycles' err_bind]; eauto.
-      destruct (find li lem2prog) as [pi|]; eauto.
-      crush_deciders idtac.
-      eapply IHn.
-      eapply Forall_cons; eauto.
-      omega.
-    Qed.
-
-    Lemma generate_cycles_correct lem2prog n :
-      match generate_cycles lem2prog n with
-      | ok cycles => Forall (fun '(from, to) => to <= from) cycles
-      | raise _ => True
-      end.
-    Proof.
-      cbv [generate_cycles].
-      pose proof (generate_cycles'_correct lem2prog nil 0 n).
-      destruct (generate_cycles' lem2prog nil 0 n); cbn [err_bind]; eauto.
-      rewrite Forall_forall.
-      setoid_rewrite <-in_rev.
-      rewrite <-Forall_forall.
-      eauto using Forall_nil.
-    Qed.
-
-    Definition cycle_pbinds (from to : nat) (pbinds : list operation)
-      : list operation + error :=
-      match Decompose.index pbinds to with
-      | Some (coda, to_op, tmp) =>
-        let distance := from - to in
-        match Decompose.index (to_op :: tmp) distance with
-        | Some (middle, from_op, prelude) =>
-          if bindings_refb middle 0
-          then raise (E_msg "middle references from")
-          else
-            ok (rev_append
-                  (renumber_bindings (cycle_to_here_renumbering distance) coda)
-                  ((renumber_op (plus distance) from_op)
-                     :: (rev_append (renumber_bindings pred middle)
-                                    prelude)))
-        | None => raise (E_msg "to out of range")
-        end
-      | None => raise (E_msg "from out of range")
-      end.
-
-    Fixpoint cycles_pbinds (cycles : list (nat * nat))
-             (pbinds : list operation) : list operation + error :=
-      match cycles with
-      | nil => ok pbinds
-      | (from, to) :: cycles => pbinds <-! cycle_pbinds from to pbinds;
-                                 cycles_pbinds cycles pbinds
-      end.
-
-    Fixpoint cycles_phead_ptail (cycles : list (nat * nat))
-             (phead : operation) (ptail : list operation)
-      : operation * list operation :=
-      match cycles with
-      | nil => (phead, ptail)
-      | (from, to) :: cycles =>
-        cycles_phead_ptail
-          cycles
-          (renumber_op (cycle from to) phead)
-          (renumber_bindings
-             (offset_renumbering 1 (cycle from to)) ptail)
-      end.
-
-    Fixpoint cycles_prog_end (len_ptail : nat) (cycles : list (nat * nat))
-             (prog_end : operation) : operation :=
-      match cycles with
-      | nil => prog_end
-      | (from, to) :: cycles =>
-        cycles_prog_end len_ptail
-          cycles (renumber_op (offset_renumbering (S len_ptail)
-                                                 (cycle from to))
-                             prog_end)
-      end.
-
-    Definition assemble (pbinds : list operation)
-               (phead : operation) (ptail : list operation)
-               (prog_end : operation) :=
-      (rev_append pbinds (phead :: ptail), prog_end).
-
-    Definition commute_matches (lbinds : list operation)
-               (lhead : operation) (e : expr) :
-      (* returns pbinds, phead, ptail, prog_end *)
-      list (nat * ((list operation * operation *
-                    list operation * operation) + error)) :=
-      (* match base has the form:
-       * (tail (normal order), head, binds (reversed order)) *)
-      let '(prog, prog_end) := e in
-      let match_bases :=
-          Decompose.find_all (fun _ => op_matches lhead) (rev prog) in
-      let len_lbinds := length lbinds in
-      List.map
-        (fun '(ptail, phead, pbinds) =>
-           let len_ptail := length ptail in
-           (len_ptail,
-            '(lem2prog, prog2lem) <-! map_match lbinds pbinds lhead phead;
-              _ <-! check_no_capturing_tail ptail prog_end prog2lem;
-              cycles <-! generate_cycles lem2prog len_lbinds;
-              new_pbinds <-! cycles_pbinds cycles pbinds;
-              let '(new_phead, new_ptail) :=
-                  cycles_phead_ptail cycles phead ptail in
-              ok (new_pbinds, new_phead, new_ptail,
-                  cycles_prog_end len_ptail cycles prog_end)))
-        match_bases.
-
-    Ltac step_err_bind :=
-      lazymatch goal with
-      | H : raise _ = ok _ |- _ => congruence
-      | H : ?e = ok _ |- _ =>
-        lazymatch e with
-        | x <-! ?y; ?z =>
-          let y' := fresh in
-          remember y as y';
-          destruct y' as [x|];
-          cbn [err_bind] in H;
-          [|congruence];
-          match type of x with
-          | unit => destruct x
-          | _ => idtac
-          end
-        | ok _ => inversion H; clear H
-        end
-      | H : ok _ = ?e |- _ =>
-        symmetry in H
-      end.
-
-    Lemma commute_matches_correct lbinds lhead e :
-      Forall (fun '(_, err) =>
-                match err with
-                | ok (new_pbinds, new_phead, new_ptail, new_prog_end) =>
-                  equiv e
-                        (assemble new_pbinds new_phead new_ptail new_prog_end)
-                | raise _ => True
-                end)
-             (commute_matches lbinds lhead e).
-      destruct e as [prog prog_end].
-      cbv [commute_matches].
-      rewrite Forall_forall.
-      setoid_rewrite in_map_iff.
-      intros [n [[[[new_pbinds' new_phead'] new_ptail'] new_prog_end']|]]
-             ([[ptail phead] pbinds]&H&?); eauto.
-      inversion H; clear dependent n.
-
-      destruct (map_match lbinds pbinds lhead phead) as [[lem2prog prog2lem]|];
-        cbn [err_bind] in *; [|congruence].
-
-      repeat step_err_bind.
-      let c := constr:(cycles_phead_ptail cycles phead ptail) in
-      replace c with (fst c, snd c) in * by (destruct c; eauto).
-      repeat step_err_bind.
-      subst new_pbinds' new_phead' new_ptail' new_prog_end'.
-      cbv [assemble].
-
-      match goal with
-      | H : context[check_no_capturing_tail] |- _ => clear H
-      end.
-
-      pose proof (Decompose.find_all_correct (fun _ => op_matches lhead)
-                                             (rev prog)) as F;
-        rewrite Forall_forall in F;
-        specialize (F _ ltac:(eauto)); cbn iota beta in F;
-          match goal with
-          | H : In (ptail, phead, pbinds) _ |- _ => clear H
-          end;
-          cbv [Decompose.found] in F;
-          destruct F as [Hprog _];
-          eapply (f_equal (@rev _)) in Hprog;
-          listrew;
-          subst prog.
-
-      pose proof generate_cycles_correct lem2prog (length lbinds) as G;
-        replace (generate_cycles lem2prog (length lbinds)) in G;
-        match goal with
-        | H : context[generate_cycles] |- _ => clear H
-        end.
-
-      cbv [equiv equiv_under interp_expr_cast interp_expr];
-        intros ctxt ctx t;
-        crush_Mequiv.
-
-      revert dependent new_pbinds;
-        revert pbinds phead ptail prog_end;
-        induction cycles as [|[from to] cycles];
-        intros pbinds phead ptail prog_end
-               new_pbinds Hnew_pbinds;
-        cbn [cycles_phead_ptail fst snd cycles_prog_end cycles_pbinds] in *.
-      { inversion_clear Hnew_pbinds; reflexivity. }
-
-      match goal with
-      | H : Forall _ (_ :: _) |- _ => inversion_clear H
-      end.
-
-      remember (cycle_pbinds from to pbinds) as e eqn:Hpbinds';
-        destruct e as [pbinds'|]; cbn [err_bind] in *; [|congruence].
-      cbv [cycle_pbinds] in Hpbinds'.
-      pose proof (Decompose.index_correct pbinds to);
-        destruct (Decompose.index pbinds to) as [[[coda to_op] tmp]|];
-        [|congruence].
-      pose proof (Decompose.index_correct (to_op :: tmp) (from - to));
-        destruct (Decompose.index (to_op :: tmp) (from - to))
-        as [[[middle from_op] prelude]|]; [|congruence].
-      remember (bindings_refb middle 0) as e;
-        destruct e; [congruence|].
-      inversion Hpbinds'; clear Hpbinds'; subst pbinds'.
-      repeat match goal with
-             | H : _ /\ _ |- _ => destruct H
-             end.
-      match goal with
-      | H : to_op :: tmp = _ |- _ => rewrite H in *; clear tmp H
-      end.
-      subst pbinds.
-      specialize (IHcycles (ltac:(eauto))
-                           (rev
-                              ((rev prelude)
-                                 ++ (renumber_bindings pred middle)
-                                 ++ renumber_op (plus (length middle)) from_op
-                                 :: (renumber_bindings
-                                       (cycle (length middle) 0)
-                                       coda)))
-                           (renumber_op
-                              (offset_renumbering
-                                 (length coda)
-                                 (cycle (length middle) 0))
-                              phead)
-                           (renumber_bindings
-                              (offset_renumbering
-                                 (S (length coda))
-                                 (cycle (length middle) 0))
-                              ptail)
-                           (renumber_op
-                              (offset_renumbering
-                                 (S (length coda) + length ptail)
-                                 (cycle (length middle) 0))
-                              prog_end)
-                           new_pbinds).
-      listrew.
-
-      replace (length middle) in *.
-      specialize (IHcycles Hnew_pbinds).
-
-      etransitivity; [|etransitivity];
-        [clear IHcycles|eapply IHcycles|clear IHcycles].
-
-      - etransitivity.
-        + clear dependent cycles.
-          clear new_pbinds.
-
-          crush_Mequiv.
-          eapply interp_bindings_Mequiv; intros ??.
-          change (from_op :: middle ++ coda)
-            with ((from_op :: middle) ++ coda).
-          setoid_rewrite interp_bindings_app at 1.
-
-          set (ks j ctxt ctx :=
-                 interp_expr_cast ctxt ctx
-                                  (renumber_expr
-                                     (cycle (length middle) j)
-                                     (coda ++ phead :: ptail, prog_end))
-                                  t).
-
-          etransitivity; [|eapply commute_many with
-                               (ks := cycle_expr_continuation
-                                        (length middle)
-                                        (coda ++ phead :: ptail, prog_end)
-                                        t)].
-          * cbv [cycle_expr_continuation].
-
-            crush_Mequiv.
-            erewrite renumber_expr_ext by (eapply cycle_trivial).
-            rewrite renumber_id_expr.
-            cbv [interp_expr_cast interp_expr].
-            crush_Mequiv.
-          * pose proof bindings_refb_ref middle 0;
-              intuition congruence.
-          * intros.
-            eapply cycle_continuation_renumbered; eauto.
-        + cbv [cycle_expr_continuation].
-          replace (length middle).
-          crush_Mequiv.
-          cbv [interp_expr_cast interp_expr].
-
-          rewrite renumber_expr_renumber_bindings.
-
-          crush_Mequiv.
-          rewrite renumber_bindings_app.
-          crush_Mequiv.
-          cbn [renumber_bindings interp_bindings].
-          crush_Mequiv.
-
-          erewrite renumber_bindings_ext
-            by (intros; rewrite <-offset_renumbering_plus; eauto).
-          cbn [plus].
-          crush_Mequiv.
-          listrew.
-          crush_Mequiv.
-      - crush_Mequiv.
-        replace (length coda).
-        cbn [renumber_bindings].
-        erewrite renumber_op_ext by (eapply offset_cycle).
-        repeat erewrite
-               (renumber_bindings_ext _ _ _
-                                      ltac:(eapply offset_cycle)).
-        cbn [plus].
-        replace (from - to + to) with from by omega.
-        replace (from - to + S to) with (S from) by omega.
-        replace (from + 1) with (S from) by omega.
-        replace (to + 1) with (S to) by omega.
-        crush_Mequiv.
-        rewrite length_renumber.
-        repeat erewrite
-               (renumber_op_ext _ _ _
-                                ltac:(eapply offset_cycle)).
-        cbn [plus].
-        replace (from - to + S (to + length ptail))
-                with (from + S (length ptail)) by omega.
-        replace (to + S (length ptail))
-                with (S (to + length ptail)) by omega.
-        crush_Mequiv.
-    Qed.
-
-    Definition replace_lemma
-               (lbinds fwd_rbinds : list operation)
-               (lhead rhead : operation)
-               (pbinds : list operation) (phead : operation)
-               (ptail : list operation) (prog_end : operation)
-      : list operation * operation * list operation * operation + error :=
-      let len_lbinds := length lbinds in
-      let len_rbinds := length fwd_rbinds in
-      _ <-! if expr_omits_rangeb len_lbinds (ptail, prog_end)
-            then ok tt
-            else raise (E_msg "replace_lemma: lbinds not omitted in tail");
-        match Decompose.prefix op_eqb (lhead :: lbinds) (phead :: pbinds) with
-        | Some rest =>
-          let f := shift len_lbinds len_rbinds in
-          ok (rev_append fwd_rbinds rest,
-              rhead,
-              renumber_bindings (offset_renumbering 1 f) ptail,
-              renumber_op (offset_renumbering (S (length ptail)) f)
-                          prog_end)
-        | None =>
-          raise (E_msg "replace_lemma: match failed")
-        end.
-
-    Lemma replace_lemma_correct lbinds fwd_rbinds lhead rhead
-      pbinds phead ptail prog_end :
-      op_type lhead = op_type rhead ->
-      equiv (rev lbinds, lhead) (fwd_rbinds, rhead) ->
-      match replace_lemma lbinds fwd_rbinds lhead rhead
-                          pbinds phead ptail prog_end with
-      | ok (new_pbinds, new_phead, new_ptail, new_prog_end) =>
-        equiv (assemble pbinds phead ptail prog_end)
-              (assemble new_pbinds new_phead new_ptail new_prog_end)
-      | raise _ => True
-      end.
-    Proof.
-      intros L ?.
-      remember (replace_lemma lbinds fwd_rbinds lhead rhead
-                              pbinds phead ptail prog_end) as err;
-        destruct err as
-          [[[[new_pbinds' new_phead'] new_ptail'] new_prog_end']|];
-        eauto.
-      cbv [replace_lemma] in *.
-      pose proof (Decompose.prefix_correct op_eqb op_eqb_eq
-                                           (lhead :: lbinds)
-                                           (phead :: pbinds));
-        destruct (Decompose.prefix op_eqb
-                                   (lhead :: lbinds)
-                                   (phead :: pbinds)) as [rest|];
-        repeat step_err_bind.
-      listrew.
-      match goal with
-      | H : _ :: _ = _ :: _ |- _ => inversion H; clear H
-      end.
-      subst new_pbinds' new_phead' new_ptail' new_prog_end' pbinds phead.
-      cbv [assemble]; listrew.
-
-      eapply equiv_prefix.
-      remember (rev lbinds) as fwd_lbinds.
-      eapply (f_equal (@rev _)) in Heqfwd_lbinds; listrew.
-      subst lbinds; listrew.
-      eapply equiv_suffix; eauto.
-      - pose proof (expr_omits_rangeb_correct (length fwd_lbinds)
-                                              (ptail, prog_end));
-          destruct (expr_omits_rangeb (length fwd_lbinds) (ptail, prog_end));
-          eauto; congruence.
-      - rewrite renumber_expr_renumber_bindings.
-        f_equal.
-        eapply renumber_op_ext.
-        intros.
-        rewrite <-offset_renumbering_plus.
-        f_equal.
-        omega.
-    Qed.
-  End WithMap.
-End Rewriter.
-
-(** Reification *)
-Ltac reify_type t :=
-  lazymatch t with
-  | prod ?ta ?tb =>
-    let ta := reify_type ta in
-    let tb := reify_type tb in
-    uconstr:(tprod ta tb)
-  | bool => tbool
-  | unit => tunit
-  | interp_type ?t => t
-  | _ => fail "UNKNOWN TYPE" t
-  end.
-
-Ltac pindexof x ctx :=
-  lazymatch ctx with
-  | (x, _) => uconstr:(O)
-  | (_, ?ctx) =>
-    let i := pindexof x ctx in
-    uconstr:(S i)
-  | _ => fail "NOT FOUND" x
-  end.
-
-Ltac reify_ref ctx r :=
-  lazymatch r with
-  | pair ?a ?b =>
-    let a := reify_ref ctx a in
-    let b := reify_ref ctx b in
-    uconstr:(ref_pair a b)
-  | ?x =>
-    let r := pindexof r ctx in
-    uconstr:(ref_index r)
-  end.
-
-Ltac reify_op ctx o :=
-  lazymatch o with
-  | ret tt => uconstr:(op_unit)
-  | interp_const coin ?a =>
-    let a := pindexof a ctx in
-    uconstr:(op_app coin (ref_index a))
-  | ret xorb ?a ?b =>
-    let a := pindexof a ctx in
-    let b := pindexof b ctx in
-    uconstr:(op_retapp xor' (ref_pair (ref_index a) (ref_index b)))
-  | ret ?x =>
-    let t := lazymatch type of x with ?T => reify_type T end in
-    let x := reify_ref ctx x in
-    uconstr:(op_retapp (id t) x)
-  | ?O => fail "UNKNOWN OP" O
-  end.
-
-Ltac reify_to_list ctx e :=
-  lazymatch e with
-  | (x <-$ ?o; ?f) =>
-    let T := lazymatch type of o with Comp ?T => T | M ?T => constr:(interp_type T) | ?X => fail "XX" X end in
-    let o := reify_op ctx o in
-    let _y := fresh in let y := fresh in (* andres thinks this might work around a coq bug but does not remember which one :( *)
-    lazymatch constr:(fun (y:T) => ltac:(
-        let r := reify_to_list
-          constr:(pair y ctx)
-          constr:(match y return _ with x => f end) in
-        exact r
-     )) with fun _ => ?r => uconstr:(@cons operation o r) | _ => fail "FUNDEP" end
-  | ?o =>
-    let o := reify_op ctx o in
-    uconstr:(@cons operation o (@nil operation))
-  | ?O => fail "UNKNOWN EXPR" O
-  end.
-Ltac reify e :=
-  let e := reify_to_list tt e in
-  let e := eval cbv in (List.removelast e, List.last e op_unit) in
-  constr:(e).
-
-Section ExampleCoins.
-  Import CrossCrypto.fmap.list_of_pairs.
-  Local Notation map := (list_of_pairs Nat.eqb).
-
-  Definition example_coin_lemma_lhs :=
-    (op_unit
-       :: op_unit
-       :: (op_app coin (ref_index 1))
-       :: (op_app coin (ref_index 1))
-       :: nil,
-     op_retapp xor' (ref_pair (ref_index 0) (ref_index 1))).
-
-  Definition example_coin_lemma_rhs :=
-    ((op_unit :: nil), op_app coin (ref_index 0)).
-
-  Lemma Mbind_unused {t1 t2} (a : M t1) (b : M t2) :
-    Mequiv (Mbind a (fun _ => b)) b.
-  Proof. eapply Bind_unused. Qed.
-
-  Lemma interp_expr_cast_different ctxt ctx e t :
-    t <> expr_type e ->
-    Mequiv (interp_expr_cast ctxt ctx e t)
-           (Mret type_inhabited).
+                    end) tk (ks (S j)) (ks j)) ->
+    Mequiv
+      (interp_bindings
+         ctxt ctx p tk
+         (fun ctxt ctx =>
+            Mbind (m ctxt ctx)
+                  (fun y => (ks (length p) (tm * ctxt)%etype (y, ctx)))))
+      (Mbind (interp_bindings ctxt ctx p tm m)
+             (fun y => ks 0 (tm * ctxt)%etype (y, ctx))).
   Proof.
-    intros; cbv [interp_expr_cast].
-    setoid_rewrite <-(Mbind_unused (interp_expr ctxt ctx e)
-                                   (Mret type_inhabited)).
-    eapply Mequiv_Mbind; [reflexivity|intros].
-    rewrite cast_different by eauto; reflexivity.
+    intros Hk.
+    rewrite bind_interp_bindings.
+    revert Hk m;
+      pattern p; revert p; eapply rev_ind; [|intros o p IHp];
+        intros Hk m.
+    { reflexivity. }
+    listrew.
+    specialize (IHp (ltac:(intros; eapply Hk; omega))
+                    (fun _ ctx =>
+                       Mbind (interp_op_silent _ ctx o)
+                             (fun x => m (_ * _)%etype (x, ctx)))).
+    specialize (Hk (length p) ltac:(omega)).
+    repeat rewrite interp_bindings_app; cbn [interp_bindings].
+    etransitivity; [|etransitivity]; [|eapply IHp|]; clear IHp;
+      [|solve [crush_Mequiv]].
+    eapply interp_bindings_Mequiv; intros ??.
+    eapply assoc_op; eauto.
   Qed.
 
-  Lemma equiv_under_same_type ctxt ctx e1 e2 :
-    expr_type e1 = expr_type e2 ->
-    Mequiv (interp_expr ctxt ctx e1)
-           (interp_expr_cast ctxt ctx e2 _) ->
-    equiv_under ctxt ctx e1 e2.
+  Definition ref_omits (f : nat -> option nat) r :=
+    forall i, refs r i -> f i <> None.
+
+  Definition op_omits (f : nat -> option nat) o :=
+    forall i, op_refs o i -> f i <> None.
+
+  Definition bindings_omit (f : nat -> option nat) p :=
+    forall i, bindings_ref p i -> f i <> None.
+
+  Definition expr_omits (f : nat -> option nat) e :=
+    forall i, expr_refs e i -> f i <> None.
+
+  Definition expr_omits_range n e :=
+    forall i, expr_refs e i -> i = 0 \/ S n <= i.
+
+  Definition expr_omits_rangeb n e :=
+    expr_all_refsb (fun i => (i =? 0) ||
+                             (S n <=? i)) e.
+
+  Lemma expr_omits_rangeb_correct n e :
+    expr_omits_rangeb n e = true -> expr_omits_range n e.
   Proof.
-    setoid_rewrite <-interp_expr_cast_expr_type.
-    cbv [equiv_under].
-    intros.
-    destruct (type_dec t (expr_type e1)).
-    - subst; eauto.
-    - setoid_rewrite interp_expr_cast_different; try congruence.
+    cbv [expr_omits_rangeb expr_omits_range]; intros He ??.
+    eapply expr_all_refsb_correct in He; eauto.
+    revert He; crush_deciders idtac.
+  Qed.
+
+  Definition silence_omission (f : nat -> option nat) j :=
+    match f j with
+    | Some x => x
+    | None => 0
+    end.
+
+  Lemma lookup_omitted_ref ctxt ctx ctxt' ctx' f r t :
+    context_omits f ctxt ctx ctxt' ctx' ->
+    ref_omits f r ->
+    lookup_ref ctxt' ctx' (renumber_ref (silence_omission f) r) t =
+    lookup_ref ctxt ctx r t.
+  Proof.
+    cbv [context_omits ref_omits silence_omission].
+    intros Hctx Hr.
+    revert t; induction r as [i|r1 IHr1 r2 IHr2]; intros t;
+      cbn [lookup_ref renumber_ref refs] in *.
+    - specialize (Hctx i t).
+      specialize (Hr _ ltac:(eauto)).
+      destruct (f i); congruence.
+    - destruct t; eauto.
+      erewrite IHr1, IHr2 by eauto; reflexivity.
+  Qed.
+
+  Lemma context_omits_1 f ctxt ctx ctxt' ctx' t (x : interp_type t) :
+    context_omits f ctxt ctx ctxt' ctx' ->
+    context_omits (offset_omission 1 f) (_ * _) (x, ctx) (_ * _) (x, ctx').
+  Proof.
+    cbv [context_omits offset_omission]; intros Hf.
+    crush_deciders (idtac;
+                    multimatch goal with
+                    | |- context[f ?x] => specialize (Hf x); destruct (f x)
+                    | _ => change (1 + ?y) with (S y)
+                    | H : ?x < 1 |- _ => assert (x = 0) by omega; clear H
+                    | _ => cbn [lookup]
+                    | _ => subst
+                    end).
+  Qed.
+
+  Lemma interp_omitted_op f o tk
+        (k k' : forall ctxt, interp_type ctxt -> M tk) :
+    op_omits f o ->
+    continuation_omits (offset_omission 1 f) tk k k' ->
+    continuation_omits
+      f tk
+      (fun _ ctx =>
+         (Mbind (interp_op_silent _ ctx o)
+                (fun x => k (_ * _)%etype (x, ctx))))
+      (fun _ ctx =>
+         (Mbind
+            (interp_op_silent _ ctx
+                              (renumber_op (silence_omission f) o))
+            (fun x => k' (_ * _)%etype (x, ctx)))).
+  Proof.
+    intros ? Hk ?????.
+    destruct o; cbn [renumber_op op_type op_refs] in *;
+      (step_Mequiv; [..|eapply Hk; eapply context_omits_1; eauto]);
+      cbv [interp_op_silent interp_op];
+      erewrite lookup_omitted_ref by eauto;
       reflexivity.
   Qed.
 
-  Lemma example_coin_lemma :
-    equiv example_coin_lemma_lhs example_coin_lemma_rhs.
+  Lemma interp_omitted_op_no_ctx f o tk
+        (k k' : forall t, interp_type t -> M tk) :
+    op_omits f o ->
+    (forall t x, Mequiv (k t x) (k' t x)) ->
+    continuation_omits
+      f tk
+      (fun ctxt ctx =>
+         (Mbind (interp_op_silent ctxt ctx o)
+                (fun x => k (op_type o) x)))
+      (fun ctxt ctx =>
+         (Mbind
+            (interp_op_silent ctxt ctx
+                              (renumber_op (silence_omission f) o))
+            (fun x => k'
+                        (op_type (renumber_op (silence_omission f) o)) x))).
   Proof.
-    intros ??.
-    eapply equiv_under_same_type; eauto.
-    cbv -[Comp_eq interp_const interp_retconst];
-      cbn [interp_const interp_retconst].
-    repeat (setoid_rewrite Bind_Ret_l || setoid_rewrite <-Bind_assoc).
-    cbv [Comp_eq image_relation pointwise_relation evalDist getSupport
-                 getAllBvectors].
-    cbn [List.map app sumList fold_left
-                  Vector.nth xorb Vector.caseS
-                  expnat Nat.mul Nat.add].
-    generalize (@EqDec_dec bool (@interp_type_eqdec tbool)); intros d0.
-    generalize (EqDec_dec bool_EqDec); intros d1.
-    intros a.
-    destruct (d0 true a), (d0 false a); try congruence;
-      destruct (d1 true a), (d1 false a); try congruence;
-        reflexivity.
+    intros ? Hk ?????.
+    destruct o; cbn [renumber_op op_type op_refs] in *;
+      (step_Mequiv; [..|eapply Hk; eapply context_omits_1; eauto]);
+      cbv [interp_op_silent interp_op];
+      erewrite lookup_omitted_ref by eauto;
+      reflexivity.
   Qed.
 
-  Definition coins_example :=
-    (op_unit :: op_app coin (ref_index 0)
-  :: op_unit :: op_app coin (ref_index 0)
-  :: op_unit :: op_app coin (ref_index 0)
-  :: op_retapp xor' (ref_pair (ref_index 4) (ref_index 0))
-       :: nil,
-     op_retapp
-       (id ((tbool * tbool) * tbool))
-       (ref_pair (ref_pair (ref_index 0) (ref_index 3)) (ref_index 3))).
-  Derive coins_endpoint
-         SuchThat (equiv coins_example coins_endpoint)
-         As coins_example_rewrite.
+  Lemma offset_omission_0 f i : offset_omission 0 f i = f i.
   Proof.
-    set (lbinds := rev (fst example_coin_lemma_lhs)).
-    set (lhead := snd example_coin_lemma_lhs).
-    pose proof (Rewriter.commute_matches_correct
-                  map lbinds lhead coins_example) as HC.
-    set (C := Rewriter.commute_matches map lbinds lhead coins_example) in HC;
-      cbv in C.
-    cbv [C Rewriter.assemble] in HC.
-    eapply Forall_inv in HC.
-    cbv [rev_append] in HC.
-    setoid_rewrite HC; clear HC.
-
-    set (fwd_rbinds := fst example_coin_lemma_rhs).
-    set (rhead := snd example_coin_lemma_rhs).
-
-    set (HR := Rewriter.replace_lemma_correct
-                 lbinds fwd_rbinds lhead rhead
-                 (op_app coin (ref_index 1)
-                         :: op_app coin (ref_index 1)
-                         :: op_unit :: op_unit
-                         :: op_app coin (ref_index 0) :: op_unit :: nil)
-                 (op_retapp xor' (ref_pair (ref_index 0) (ref_index 1)))
-                 nil
-                 (op_retapp (id (tbool * tbool * tbool))
-                            (ref_pair (ref_pair (ref_index 0)
-                                                (ref_index 5))
-                                      (ref_index 5)))
-                 eq_refl
-                 example_coin_lemma).
-    set (R := Rewriter.replace_lemma
-                lbinds fwd_rbinds lhead rhead
-                (op_app coin (ref_index 1)
-                        :: op_app coin (ref_index 1)
-                        :: op_unit :: op_unit
-                        :: op_app coin (ref_index 0) :: op_unit :: nil)
-                (op_retapp xor' (ref_pair (ref_index 0) (ref_index 1)))
-                nil
-                (op_retapp (id (tbool * tbool * tbool))
-                           (ref_pair (ref_pair (ref_index 0)
-                                               (ref_index 5))
-                                     (ref_index 5)))) in HR;
-      cbv in R;
-      cbv [R Rewriter.assemble rev_append] in HR.
-    setoid_rewrite HR; clear HR.
-    subst coins_endpoint; reflexivity.
+    cbv [offset_omission].
+    crush_deciders idtac.
+    subst; cbn [plus].
+    destruct (f _); eauto.
   Qed.
-  Print coins_endpoint.
 
-  (*
-  Eval cbv [interp_expr coins_example interp_bindings Mbind Mret interp_op_silent interp_op lookup_ref lookup transport type_dec type_rec type_rect op_type cdom eq_rect_r eq_rect eq_sym rcdom ccod rccod interp_retconst] in
-      interp_expr tunit tt coins_example.
-   *)
+  Lemma context_omits_ext f1 f2 ctxt ctx ctxt' ctx' :
+    (forall i, f1 i = f2 i) ->
+    context_omits f1 ctxt ctx ctxt' ctx' <->
+    context_omits f2 ctxt ctx ctxt' ctx'.
+  Proof. intros H; cbv [context_omits]; setoid_rewrite H; reflexivity. Qed.
 
-  Definition coins_example' :=
-    x <-$ ret tt;
-    x0 <-$ interp_const coin x;
-    x1 <-$ ret tt;
-    x2 <-$ interp_const coin x1;
-    x3 <-$ ret tt;
-    x4 <-$ interp_const coin x3;
-    x5 <-$ ret xorb x0 x4;
-    ret (x5, x2, x2).
-  Derive reified_coins_example
-  SuchThat (reified_coins_example = coins_example')
-  As reified_coins_example'_correct.
+  Lemma continuation_omits_ext f1 f2 tk k k' :
+    (forall i, f1 i = f2 i) ->
+    continuation_omits f1 tk k k' ->
+    continuation_omits f2 tk k k'.
   Proof.
-    cbv [coins_example'].
+    intros H Hk ?????.
+    eapply Hk.
+    erewrite context_omits_ext; eauto.
+  Qed.
 
-    let x := reified_coins_example in
-    let x := eval unfold x in x in
-    let e := match goal with |- ?LHS = ?RHS => RHS end in
-    let e := reify e in
-    unify x (interp_expr tunit tt e).
+  Local Instance continuation_omits_Mequiv f tk :
+    Proper
+      (forall_relation
+         (fun ctxt => pointwise_relation (interp_type ctxt) Mequiv) ==>
+         forall_relation
+         (fun ctxt => pointwise_relation (interp_type ctxt) Mequiv) ==>
+         iff) (continuation_omits f tk).
+  Proof.
+    cbv [Proper respectful forall_relation pointwise_relation Basics.impl].
+    cbv [continuation_omits].
+    intros k1 k1' Hk1 k2 k2' Hk2.
+    split; intros H ctxt ctx ctxt' ctx';
+      (etransitivity; [|etransitivity];
+       [|eapply H|]);
+      solve [eauto | symmetry; eauto].
+  Qed.
 
+  Lemma bindings_omit_app_invl f p1 p2 :
+    bindings_omit f (p1 ++ p2) -> bindings_omit f p1.
+  Proof.
+    cbv [bindings_omit].
+    intros Ha.
+    setoid_rewrite bindings_ref_app in Ha.
+    intuition eauto.
+  Qed.
+
+  Lemma bindings_omit_app_invr f p1 p2 :
+    bindings_omit f (p1 ++ p2) ->
+    bindings_omit (offset_omission (length p1) f) p2.
+  Proof.
+    cbv [bindings_omit offset_omission].
+    intros Ha.
+    setoid_rewrite bindings_ref_app in Ha.
+    intros i ?.
+    crush_deciders idtac.
+    match goal with
+    | _ : context[f ?x] |- _ => specialize (Ha x)
+    end.
+    subst.
+    destruct (f _); eauto; congruence.
+  Qed.
+
+  Lemma offset_silence n f i :
+    offset_omission n f i <> None ->
+    offset_renumbering n (silence_omission f) i =
+    silence_omission (offset_omission n f) i.
+  Proof.
+    intros.
+    cbv [offset_renumbering silence_omission offset_omission] in *.
+    crush_deciders (destruct (f _)).
+  Qed.
+
+  Lemma offset_offset_omission a b f i :
+    offset_omission (a + b) f i =
+    offset_omission a (offset_omission b f) i.
+  Proof.
+    cbv [offset_omission].
+    crush_deciders idtac.
+    subst.
+    match goal with
+    | H : ?x + ?y + ?z = ?x + (?y + ?z') |- _ =>
+      assert (z = z') by omega; clear H; subst
+    end.
+    destruct (f _); f_equal; omega.
+  Qed.
+
+  Lemma interp_omitted_bindings f p
+        tk (k k' : forall ctxt : type, interp_type ctxt -> M tk) :
+    bindings_omit f p ->
+    continuation_omits (offset_omission (length p) f) tk k k' ->
+    continuation_omits
+      f tk
+      (fun ctxt ctx => interp_bindings ctxt ctx p tk k)
+      (fun ctxt ctx =>
+         interp_bindings ctxt ctx
+                         (renumber_bindings (silence_omission f) p) tk k').
+  Proof.
+    revert tk k k'.
+    pattern p; revert p; eapply rev_ind;
+      cbn [renumber_bindings interp_bindings length offset_renumbering
+                             optsub plus]; [|intros o p IHp];
+        intros tk k k' Hp Hkk'.
+    { eapply continuation_omits_ext in Hkk';
+        try solve [eapply offset_omission_0].
+      eapply Hkk'. }
+    rewrite renumber_bindings_app.
+    cbn [renumber_bindings].
+    setoid_rewrite interp_bindings_app.
+    pose proof (bindings_omit_app_invl _ _ _ Hp).
+    pose proof (bindings_omit_app_invr _ _ _ Hp).
+    cbv [bindings_omit] in *; cbn [bindings_ref] in *.
+    clear Hp.
+    eapply IHp; eauto; cbn [interp_bindings].
+    intros ?????.
+    rewrite renumber_op_ext_relevant with
+        (f := (offset_renumbering (length p) (silence_omission f)))
+        (f' := (silence_omission (offset_omission (length p) f)))
+      by (eauto using offset_silence).
+
+    eapply interp_omitted_op; try solve [eauto |
+                                         cbv [op_omits]; intuition eauto].
+    listrew.
+    eapply continuation_omits_ext;
+      try eapply offset_offset_omission; eauto.
+  Qed.
+
+  Lemma interp_omitted_expr f t (e : expr) :
+    expr_omits f e ->
+    continuation_omits
+      f t
+      (fun ctxt ctx => interp_expr_cast ctxt ctx e t)
+      (fun ctxt ctx =>
+         interp_expr_cast ctxt ctx (renumber_expr (silence_omission f) e) t).
+  Proof.
+    intros He ?????.
+    destruct e as [p o].
+    cbv [expr_omits expr_refs] in *.
+    rewrite renumber_expr_renumber_bindings.
+    erewrite renumber_op_ext_relevant; cycle 1.
+    { intros i ?.
+      eapply offset_silence.
+      cbv [offset_omission].
+      crush_deciders subst.
+      match goal with
+      | _ : context[f ?x] |- _ => specialize (He x)
+      end.
+      destruct (f _); eauto; congruence. }
+    cbv [interp_expr_cast interp_expr].
+    setoid_rewrite bind_interp_bindings.
+    eapply interp_omitted_bindings;
+      try solve [eauto | cbv [bindings_omit]; intuition eauto].
+    refine (interp_omitted_op_no_ctx
+              _ _ _
+              (fun _ x => Mret (cast t x))
+              (fun _ x => Mret (cast t x))
+              _ _).
+    { intros i ?.
+      cbv [offset_omission].
+      crush_deciders subst.
+      intros.
+      match goal with
+      | _ : context[f ?x] |- _ => specialize (He x)
+      end.
+      destruct (f _); eauto; congruence. }
     reflexivity.
   Qed.
-  Print reified_coins_example.
-End ExampleCoins.
+
+  Definition shift from to i := if i <? from
+                                then 0
+                                else i - from + to.
+
+  Definition shift_expr_continuation e t total j ctxt ctx :=
+    interp_expr_cast ctxt ctx (renumber_expr (shift (S (total - j)) 1) e) t.
+
+  Lemma shift_S from i :
+    shift (S from) 1 i =
+    (silence_omission (fun n => match n with
+                                | 0 => Some 0
+                                | 1 => None
+                                | S n => Some n
+                                end))
+      (shift from 1 i).
+  Proof.
+    cbv [shift silence_omission].
+    crush_deciders (idtac;
+                    multimatch goal with
+                    | |- context[match ?x with _ => _ end] =>
+                      lazymatch x with
+                      | context[match _ with _ => _ end] => fail
+                      | _ => idtac
+                      end;
+                      let x' := fresh "x" in remember x as x'; destruct x'
+                    end).
+  Qed.
+
+  Lemma shift_continuation_omitted e t total j :
+    j < total ->
+    expr_omits_range total e ->
+    continuation_omits
+      (fun n => match n with
+                | 0 => Some 0
+                | 1 => None
+                | S n => Some n
+                end) t
+      (shift_expr_continuation e t total (S j))
+      (shift_expr_continuation e t total j).
+  Proof.
+    cbv [shift_expr_continuation]; intros ? He.
+    replace (S (total - j)) with (S (S (total - S j))) by omega.
+    erewrite (renumber_expr_ext
+                _ _ _ ltac:(eapply (shift_S (S (total - S j))))).
+    rewrite renumber_renumber_expr with
+        (h := (fun i =>
+                 silence_omission
+                   (fun n =>
+                      match n with
+                      | 0 => Some 0
+                      | 1 => None
+                      | S n => Some n
+                      end) (shift (S (total - S j)) 1 i)))
+        (g := silence_omission
+                (fun n =>
+                   match n with
+                   | 0 => Some 0
+                   | 1 => None
+                   | S n => Some n
+                   end))
+        (f := (shift (S (total - S j)) 1))
+      by reflexivity.
+    eapply interp_omitted_expr.
+    cbv [expr_omits expr_omits_range].
+    intros i Hi.
+    eapply expr_refs_renumber in Hi; destruct Hi as (x&?&?).
+    subst.
+    enough (shift (S (total - S j)) 1 x <> 1) by
+        (destruct (shift (S (total - S j)) 1 x) as [|[|]]; congruence).
+    destruct e; cbv [expr_omits_range] in *.
+    specialize (He _ ltac:(eauto)).
+    cbv [shift].
+    destruct He; crush_deciders idtac.
+  Qed.
+
+  Lemma equiv_prefix l p o p' o' :
+    equiv (p, o) (p', o') ->
+    equiv (l ++ p, o) (l ++ p', o').
+  Proof.
+    cbv [equiv equiv_under interp_expr_cast interp_expr].
+    intros H ???.
+    crush_Mequiv.
+    etransitivity; [|etransitivity]; [|eapply H|];
+      crush_Mequiv.
+  Qed.
+
+  Lemma shift_trivial i : shift 1 1 i = i.
+  Proof. cbv [shift]; crush_deciders idtac. Qed.
+
+  Lemma offset_1_shift from to i :
+    i = 0 \/ i > from ->
+    offset_renumbering 1 (shift from to) i = shift (S from) (S to) i.
+  Proof. cbv [shift offset_renumbering]; crush_deciders idtac. Qed.
+
+  Lemma shift_shift a b c i :
+    b <> 0 ->
+    shift b c (shift a b i) = shift a c i.
+  Proof.
+    cbv [shift]; crush_deciders idtac.
+  Qed.
+
+  Lemma shift_expr_continuation_shift t ctxt ctx s so n n' :
+    expr_omits_range n (s, so) ->
+    Mequiv
+      (shift_expr_continuation (s, so) t n 0 ctxt ctx)
+      (shift_expr_continuation
+         (renumber_expr (offset_renumbering 1 (shift n n')) (s, so))
+         t n' 0 ctxt ctx).
+  Proof.
+    intros.
+    erewrite (renumber_expr_ext_relevant
+                _ _ _ ltac:(intros; rewrite offset_1_shift; eauto)).
+    cbv [shift_expr_continuation].
+    repeat (evar (x : nat); subst x; replace (?x - 0) with (?x) by omega).
+    erewrite <-renumber_renumber_expr.
+    - reflexivity.
+    - intros.
+      rewrite shift_shift; omega.
+  Qed.
+
+  Lemma omit_range_shift n n' e :
+    expr_omits_range n e ->
+    expr_omits_range n' (renumber_expr (offset_renumbering 1 (shift n n')) e).
+  Proof.
+    cbv [expr_omits_range].
+    setoid_rewrite expr_refs_renumber.
+    intros H ?(?&?&?); subst.
+    specialize (H _ ltac:(eauto)).
+    cbv [offset_renumbering shift]; crush_deciders idtac.
+  Qed.
+
+  Lemma equiv_suffix p o p' o' s so s' so' :
+    op_type o = op_type o' ->
+    expr_omits_range (length p) (s, so) ->
+    (s', so') = renumber_expr
+                  (offset_renumbering 1 (shift (length p) (length p')))
+                  (s, so) ->
+    equiv (p, o) (p', o') ->
+    equiv (p ++ o :: s, so) (p' ++ o' :: s', so').
+    intros ???.
+    intros Hpp'.
+    assert (expr_omits_range (length p') (s', so'))
+      by (replace (s', so'); eauto using omit_range_shift).
+    cbv [equiv equiv_under interp_expr_cast interp_expr].
+    intros.
+    crush_Mequiv.
+
+    etransitivity; etransitivity; [..|etransitivity];
+      [|
+       solve [eapply assoc_many
+                with (p := p)
+                     (m := (fun ctxt ctx => interp_op_silent ctxt ctx o))
+                     (ks := shift_expr_continuation (s, so) t
+                                                    (length p));
+              intros; eapply shift_continuation_omitted; eauto]
+       | |
+       solve [symmetry;
+              eapply assoc_many
+                with (p := p')
+                     (m := (fun ctxt ctx => interp_op_silent ctxt ctx o'))
+                     (ks := shift_expr_continuation (s', so') t
+                                                    (length p'));
+              intros; eapply shift_continuation_omitted; eauto]
+       |]; cycle 1;
+        [|cbv [shift_expr_continuation interp_expr_cast interp_expr];
+          replace (length _ - length _) with 0 by omega;
+          erewrite renumber_expr_ext by (eapply shift_trivial);
+          rewrite renumber_id_expr;
+          crush_Mequiv ..].
+
+    etransitivity; [|etransitivity];
+      [|eapply Mequiv_Mbind_cast
+          with
+            (c2 :=
+               fun tx (x : interp_type tx) =>
+                 (shift_expr_continuation (s, so) t (length p) 0
+                                          (tx * ctxt) (x, ctx)))
+            (c2' :=
+               fun tx (x : interp_type tx) =>
+                 (shift_expr_continuation (s', so') t (length p') 0
+                                          (tx * ctxt) (x, ctx)));
+        [eauto|eapply Hpp'|]|]; cycle 1;
+        [|solve [cbv [interp_expr_cast interp_expr expr_type];
+                 crush_Mequiv] ..].
+    intros.
+    replace (s', so').
+    eapply shift_expr_continuation_shift; eauto.
+  Qed.
+
+  Section Rewriter.
+    Inductive error :=
+    | E_debug {t : Type} (_ : t)
+    | E_trace {t u : Type} (_ : t) (_ : u + error)
+    | E_todo (_ : string)
+    | E_msg (_ : string).
+
+    Local Notation ok := inl.
+    Local Notation raise := inr.
+    Definition err_bind {t1 t2} (a : t1 + error) (b : t1 -> t2 + error)
+      : t2 + error :=
+      match a with
+      | ok x => b x
+      | raise e => raise e
+      end.
+    Local Notation "x <-! a ; b" := (err_bind a (fun x => b))
+                                      (right associativity,
+                                       at level 100).
+    Local Notation "' x <-! a ; b" := (err_bind a (fun 'x => b))
+                                        (x strict pattern,
+                                         right associativity,
+                                         at level 100).
+
+    Section WithMap.
+      Context (map_ops : CrossCrypto.fmap.operations nat nat).
+      Local Notation map := (map_ops.(fmap.M)).
+      Local Notation empty := (map_ops.(fmap.empty)).
+      Local Notation add := (map_ops.(fmap.add)).
+      Local Notation find := (map_ops.(fmap.find)).
+      Local Notation fold_ac := (map_ops.(fmap.fold_ac)).
+
+      Definition op_matches (o1 o2 : op) :=
+        match o1, o2 with
+        | op_unit, op_unit => true
+        | op_app c _, op_app c' _ =>
+          if c ?= c' then true else false
+        | op_retapp c _, op_retapp c' _ =>
+          if c ?= c' then true else false
+        | _, _ => false
+        end.
+
+      (* TODO
+       * - matching rewrite
+       *   + (normalize lemma by removing any unused bindings)
+       *   X find a match (inverse maps which line up program and lemma)
+       *   + (renumber the lemma's free variables)
+       *   X check that the match isn't captured by the program's tail
+       *   X generate a sequence of cycles
+       *   X check the legality of the cycles
+       *   X prove the cycle-checker correct
+       *   X run the cycles individually
+       *   X run the strict matcher
+       *     (could prove that it always succeeds but that would be hard)
+       *   X rewrite the lemma
+       * - reification
+       *   + reify to PHOAS first, then to flat structure
+       * - support for ret
+       *   + duplicating/deduplicating rets
+       * - support for free variables
+       *   + need to renumber them on both sides of the lemma to match the
+       *     program
+       * - support for unused bindings
+       *)
+
+      Definition update_maps_ind (lem2prog prog2lem : map) (li pi : nat)
+        : map * map + error :=
+        match find li lem2prog with
+        | Some pi' => if pi =? pi'
+                      then ok (lem2prog, prog2lem)
+                      else raise (E_msg "map_match: lem2prog mismatch")
+        | None =>
+          let lem2prog := add li pi lem2prog in
+          match find pi prog2lem with
+          | Some li' => if li =? li'
+                        then ok (lem2prog, prog2lem)
+                        else raise (E_msg "map_match: prog2lem mismatch")
+          | None =>
+            let prog2lem := add pi li prog2lem in
+            ok (lem2prog, prog2lem)
+          end
+        end.
+
+      Fixpoint update_maps_ref (loff poff : nat) (lem2prog prog2lem : map)
+               (lr pr : ref) {struct lr} :
+        map * map + error :=
+        match lr, pr with
+        | ref_index ln, ref_index pn =>
+          update_maps_ind lem2prog prog2lem (loff + ln) (poff + pn)
+        | ref_pair lr1 lr2, ref_pair pr1 pr2 =>
+          '(lem2prog, prog2lem) <-!
+           update_maps_ref loff poff lem2prog prog2lem lr1 pr1;
+            update_maps_ref loff poff lem2prog prog2lem lr2 pr2
+        | _, _ => raise (E_msg "map_match: ref mismatch")
+        end.
+
+      Definition update_maps_op
+                 (lop pop : op)
+                 (loff poff : nat) (lem2prog prog2lem : map)
+        : map * map + error :=
+        match lop, pop with
+        | op_unit, op_unit => ok (lem2prog, prog2lem)
+        | op_app lc lr, op_app pc pr =>
+          if lc ?= pc
+          then update_maps_ref loff poff lem2prog prog2lem lr pr
+          else raise (E_msg "map_match: op const mismatch")
+        | op_retapp lc lr, op_retapp pc pr =>
+          if lc ?= pc
+          then update_maps_ref loff poff lem2prog prog2lem lr pr
+          else raise (E_msg "map_match: op retconst mismatch")
+        | _, _ => raise (E_msg "map_match: op mismatch")
+        end.
+
+      (* iterate over lbinds, using the map found so far to index into
+       * pbinds.  lbinds gets shorter, pbinds stays the same.
+       * The "empty lem2prog entry" error occurs if the lemma has unused
+       * bindings; "bad lem2prog entry" occurs if the program refers to a
+       * free variable but that variable is not free in the lemma. *)
+      Fixpoint map_match'
+               (lbinds pbinds : list op) (lhead phead : op)
+               (loff poff : nat) (lem2prog prog2lem : map) {struct lbinds}
+        : map * map + error :=
+        '(lem2prog, prog2lem) <-!
+         update_maps_op lhead phead loff poff lem2prog prog2lem;
+          match lbinds with
+          | nil => ok (lem2prog, prog2lem)
+          | cons lhead lbinds =>
+            match find loff lem2prog with
+            | Some pi =>
+              match List.nth_error pbinds pi with
+              | Some phead => map_match' lbinds pbinds
+                                         lhead phead
+                                         (S loff) (S pi)
+                                         lem2prog prog2lem
+              | None => raise (E_msg "map_match: bad lem2prog entry")
+              end
+            | None => raise (E_msg "map_match: empty lem2prog entry")
+            end
+          end.
+
+      (* binds and lbinds are in reversed order from their usual order in
+       * expr.  returns lemma-to-program and program-to-lemma maps of de
+       * Bruijn indices relative to the head
+       *)
+      Definition map_match (lbinds pbinds : list op)
+                 (lhead phead : op) : map * map + error :=
+        map_match' lbinds pbinds lhead phead 0 0 empty empty.
+
+      Definition check_no_capturing_tail (ptail : list op)
+                 (prog_end : op)
+                 (prog2lem : map) : unit + error :=
+        fold_ac _ (fun n _ acc =>
+                     _ <-! acc;
+                       if bindings_refb ptail (S n)
+                          || op_refsb prog_end (S (length ptail) + n)
+                       then raise (E_msg "check_no_capturing_tail: capture")
+                       else ok tt)
+                (ok tt) prog2lem.
+
+      Definition renumber_lem2prog (lem2prog : map) (pi li : nat) :=
+        fold_ac _ (fun lj pj lem2prog =>
+                     if pj =? pi
+                     then lem2prog
+                     else add lj (cycle pi li pj) lem2prog)
+                empty lem2prog.
+
+      Fixpoint generate_cycles' lem2prog (cycles : list (nat * nat))
+               (li : nat) (n : nat) :=
+        match n with
+        | 0 => ok cycles
+        | S n =>
+          match find li lem2prog with
+          | Some pi =>
+            if pi <? li
+            then raise (E_msg "generate_cycles: pi < li")
+            else generate_cycles' (renumber_lem2prog lem2prog pi li)
+                                  ((pi, li) :: cycles)
+                                  (S li) n
+          | None => raise (E_msg "generate_cycles: bad li")
+          end
+        end.
+
+      Definition generate_cycles lem2prog (len_lbinds : nat)
+        : list (nat * nat) + error :=
+        cycles <-! generate_cycles' lem2prog nil 0 len_lbinds;
+          ok (rev cycles).
+
+      Lemma generate_cycles'_correct lem2prog cycles li n :
+        Forall (fun '(from, to) => to <= from) cycles ->
+        match generate_cycles' lem2prog cycles li n with
+        | ok cycles => Forall (fun '(from, to) => to <= from) cycles
+        | raise _ => True
+        end.
+      Proof.
+        revert lem2prog cycles li; induction n;
+          intros lem2prog cycles li ?;
+                 cbn [generate_cycles' err_bind]; eauto.
+        destruct (find li lem2prog) as [pi|]; eauto.
+        crush_deciders idtac.
+        eapply IHn.
+        eapply Forall_cons; eauto.
+        omega.
+      Qed.
+
+      Lemma generate_cycles_correct lem2prog n :
+        match generate_cycles lem2prog n with
+        | ok cycles => Forall (fun '(from, to) => to <= from) cycles
+        | raise _ => True
+        end.
+      Proof.
+        cbv [generate_cycles].
+        pose proof (generate_cycles'_correct lem2prog nil 0 n).
+        destruct (generate_cycles' lem2prog nil 0 n); cbn [err_bind]; eauto.
+        rewrite Forall_forall.
+        setoid_rewrite <-in_rev.
+        rewrite <-Forall_forall.
+        eauto using Forall_nil.
+      Qed.
+
+      Definition cycle_pbinds (from to : nat) (pbinds : list op)
+        : list op + error :=
+        match Decompose.index pbinds to with
+        | Some (coda, to_op, tmp) =>
+          let distance := from - to in
+          match Decompose.index (to_op :: tmp) distance with
+          | Some (middle, from_op, prelude) =>
+            if bindings_refb middle 0
+            then raise (E_msg "middle references from")
+            else
+              ok (rev_append
+                    (renumber_bindings (cycle_to_here_renumbering distance) coda)
+                    ((renumber_op (plus distance) from_op)
+                       :: (rev_append (renumber_bindings pred middle)
+                                      prelude)))
+          | None => raise (E_msg "to out of range")
+          end
+        | None => raise (E_msg "from out of range")
+        end.
+
+      Fixpoint cycles_pbinds (cycles : list (nat * nat))
+               (pbinds : list op) : list op + error :=
+        match cycles with
+        | nil => ok pbinds
+        | (from, to) :: cycles => pbinds <-! cycle_pbinds from to pbinds;
+                                    cycles_pbinds cycles pbinds
+        end.
+
+      Fixpoint cycles_phead_ptail (cycles : list (nat * nat))
+               (phead : op) (ptail : list op)
+        : op * list op :=
+        match cycles with
+        | nil => (phead, ptail)
+        | (from, to) :: cycles =>
+          cycles_phead_ptail
+            cycles
+            (renumber_op (cycle from to) phead)
+            (renumber_bindings
+               (offset_renumbering 1 (cycle from to)) ptail)
+        end.
+
+      Fixpoint cycles_prog_end (len_ptail : nat) (cycles : list (nat * nat))
+               (prog_end : op) : op :=
+        match cycles with
+        | nil => prog_end
+        | (from, to) :: cycles =>
+          cycles_prog_end len_ptail
+                          cycles (renumber_op (offset_renumbering (S len_ptail)
+                                                                  (cycle from to))
+                                              prog_end)
+        end.
+
+      Definition assemble (pbinds : list op)
+                 (phead : op) (ptail : list op)
+                 (prog_end : op) :=
+        (rev_append pbinds (phead :: ptail), prog_end).
+
+      Definition commute_matches (lbinds : list op)
+                 (lhead : op) (e : expr) :
+        (* returns pbinds, phead, ptail, prog_end *)
+        list (nat * ((list op * op *
+                      list op * op) + error)) :=
+        (* match base has the form:
+         * (tail (normal order), head, binds (reversed order)) *)
+        let '(prog, prog_end) := e in
+        let match_bases :=
+            Decompose.find_all (fun _ => op_matches lhead) (rev prog) in
+        let len_lbinds := length lbinds in
+        List.map
+          (fun '(ptail, phead, pbinds) =>
+             let len_ptail := length ptail in
+             (len_ptail,
+              '(lem2prog, prog2lem) <-! map_match lbinds pbinds lhead phead;
+                _ <-! check_no_capturing_tail ptail prog_end prog2lem;
+                cycles <-! generate_cycles lem2prog len_lbinds;
+                new_pbinds <-! cycles_pbinds cycles pbinds;
+                let '(new_phead, new_ptail) :=
+                    cycles_phead_ptail cycles phead ptail in
+                ok (new_pbinds, new_phead, new_ptail,
+                    cycles_prog_end len_ptail cycles prog_end)))
+          match_bases.
+
+      Ltac step_err_bind :=
+        lazymatch goal with
+        | H : raise _ = ok _ |- _ => congruence
+        | H : ?e = ok _ |- _ =>
+          lazymatch e with
+          | x <-! ?y; ?z =>
+            let y' := fresh in
+            remember y as y';
+            destruct y' as [x|];
+            cbn [err_bind] in H;
+            [|congruence];
+            match type of x with
+            | unit => destruct x
+            | _ => idtac
+            end
+          | ok _ => inversion H; clear H
+          end
+        | H : ok _ = ?e |- _ =>
+          symmetry in H
+        end.
+
+      Lemma commute_matches_correct lbinds lhead e :
+        Forall (fun '(_, err) =>
+                  match err with
+                  | ok (new_pbinds, new_phead, new_ptail, new_prog_end) =>
+                    equiv e
+                          (assemble new_pbinds new_phead new_ptail new_prog_end)
+                  | raise _ => True
+                  end)
+               (commute_matches lbinds lhead e).
+        destruct e as [prog prog_end].
+        cbv [commute_matches].
+        rewrite Forall_forall.
+        setoid_rewrite in_map_iff.
+        intros [n [[[[new_pbinds' new_phead'] new_ptail'] new_prog_end']|]]
+               ([[ptail phead] pbinds]&H&?); eauto.
+        inversion H; clear dependent n.
+
+        destruct (map_match lbinds pbinds lhead phead) as [[lem2prog prog2lem]|];
+          cbn [err_bind] in *; [|congruence].
+
+        repeat step_err_bind.
+        let c := constr:(cycles_phead_ptail cycles phead ptail) in
+        replace c with (fst c, snd c) in * by (destruct c; eauto).
+        repeat step_err_bind.
+        subst new_pbinds' new_phead' new_ptail' new_prog_end'.
+        cbv [assemble].
+
+        match goal with
+        | H : context[check_no_capturing_tail] |- _ => clear H
+        end.
+
+        pose proof (Decompose.find_all_correct (fun _ => op_matches lhead)
+                                               (rev prog)) as F;
+          rewrite Forall_forall in F;
+          specialize (F _ ltac:(eauto)); cbn iota beta in F;
+            match goal with
+            | H : In (ptail, phead, pbinds) _ |- _ => clear H
+            end;
+            cbv [Decompose.found] in F;
+            destruct F as [Hprog _];
+            eapply (f_equal (@rev _)) in Hprog;
+            listrew;
+            subst prog.
+
+        pose proof generate_cycles_correct lem2prog (length lbinds) as G;
+          replace (generate_cycles lem2prog (length lbinds)) in G;
+          match goal with
+          | H : context[generate_cycles] |- _ => clear H
+          end.
+
+        cbv [equiv equiv_under interp_expr_cast interp_expr];
+          intros ctxt ctx t;
+          crush_Mequiv.
+
+        revert dependent new_pbinds;
+          revert pbinds phead ptail prog_end;
+          induction cycles as [|[from to] cycles];
+          intros pbinds phead ptail prog_end
+                 new_pbinds Hnew_pbinds;
+          cbn [cycles_phead_ptail fst snd cycles_prog_end cycles_pbinds] in *.
+        { inversion_clear Hnew_pbinds; reflexivity. }
+
+        match goal with
+        | H : Forall _ (_ :: _) |- _ => inversion_clear H
+        end.
+
+        remember (cycle_pbinds from to pbinds) as e eqn:Hpbinds';
+          destruct e as [pbinds'|]; cbn [err_bind] in *; [|congruence].
+        cbv [cycle_pbinds] in Hpbinds'.
+        pose proof (Decompose.index_correct pbinds to);
+          destruct (Decompose.index pbinds to) as [[[coda to_op] tmp]|];
+          [|congruence].
+        pose proof (Decompose.index_correct (to_op :: tmp) (from - to));
+          destruct (Decompose.index (to_op :: tmp) (from - to))
+          as [[[middle from_op] prelude]|]; [|congruence].
+        remember (bindings_refb middle 0) as e;
+          destruct e; [congruence|].
+        inversion Hpbinds'; clear Hpbinds'; subst pbinds'.
+        repeat match goal with
+               | H : _ /\ _ |- _ => destruct H
+               end.
+        match goal with
+        | H : to_op :: tmp = _ |- _ => rewrite H in *; clear tmp H
+        end.
+        subst pbinds.
+        specialize (IHcycles (ltac:(eauto))
+                             (rev
+                                ((rev prelude)
+                                   ++ (renumber_bindings pred middle)
+                                   ++ renumber_op (plus (length middle)) from_op
+                                   :: (renumber_bindings
+                                         (cycle (length middle) 0)
+                                         coda)))
+                             (renumber_op
+                                (offset_renumbering
+                                   (length coda)
+                                   (cycle (length middle) 0))
+                                phead)
+                             (renumber_bindings
+                                (offset_renumbering
+                                   (S (length coda))
+                                   (cycle (length middle) 0))
+                                ptail)
+                             (renumber_op
+                                (offset_renumbering
+                                   (S (length coda) + length ptail)
+                                   (cycle (length middle) 0))
+                                prog_end)
+                             new_pbinds).
+        listrew.
+
+        replace (length middle) in *.
+        specialize (IHcycles Hnew_pbinds).
+
+        etransitivity; [|etransitivity];
+          [clear IHcycles|eapply IHcycles|clear IHcycles].
+
+        - etransitivity.
+          + clear dependent cycles.
+            clear new_pbinds.
+
+            crush_Mequiv.
+            eapply interp_bindings_Mequiv; intros ??.
+            change (from_op :: middle ++ coda)
+              with ((from_op :: middle) ++ coda).
+            setoid_rewrite interp_bindings_app at 1.
+
+            set (ks j ctxt ctx :=
+                   interp_expr_cast ctxt ctx
+                                    (renumber_expr
+                                       (cycle (length middle) j)
+                                       (coda ++ phead :: ptail, prog_end))
+                                    t).
+
+            etransitivity; [|eapply commute_many with
+                                 (ks := cycle_expr_continuation
+                                          (length middle)
+                                          (coda ++ phead :: ptail, prog_end)
+                                          t)].
+            * cbv [cycle_expr_continuation].
+
+              crush_Mequiv.
+              erewrite renumber_expr_ext by (eapply cycle_trivial).
+              rewrite renumber_id_expr.
+              cbv [interp_expr_cast interp_expr].
+              crush_Mequiv.
+            * pose proof bindings_refb_ref middle 0;
+                intuition congruence.
+            * intros.
+              eapply cycle_continuation_renumbered; eauto.
+          + cbv [cycle_expr_continuation].
+            replace (length middle).
+            crush_Mequiv.
+            cbv [interp_expr_cast interp_expr].
+
+            rewrite renumber_expr_renumber_bindings.
+
+            crush_Mequiv.
+            rewrite renumber_bindings_app.
+            crush_Mequiv.
+            cbn [renumber_bindings interp_bindings].
+            crush_Mequiv.
+
+            erewrite renumber_bindings_ext
+              by (intros; rewrite <-offset_renumbering_plus; eauto).
+            cbn [plus].
+            crush_Mequiv.
+            listrew.
+            crush_Mequiv.
+        - crush_Mequiv.
+          replace (length coda).
+          cbn [renumber_bindings].
+          erewrite renumber_op_ext by (eapply offset_cycle).
+          repeat erewrite
+                 (renumber_bindings_ext _ _ _
+                                        ltac:(eapply offset_cycle)).
+          cbn [plus].
+          replace (from - to + to) with from by omega.
+          replace (from - to + S to) with (S from) by omega.
+          replace (from + 1) with (S from) by omega.
+          replace (to + 1) with (S to) by omega.
+          crush_Mequiv.
+          rewrite length_renumber.
+          repeat erewrite
+                 (renumber_op_ext _ _ _
+                                  ltac:(eapply offset_cycle)).
+          cbn [plus].
+          replace (from - to + S (to + length ptail))
+            with (from + S (length ptail)) by omega.
+          replace (to + S (length ptail))
+            with (S (to + length ptail)) by omega.
+          crush_Mequiv.
+      Qed.
+
+      Definition replace_lemma
+                 (lbinds fwd_rbinds : list op)
+                 (lhead rhead : op)
+                 (pbinds : list op) (phead : op)
+                 (ptail : list op) (prog_end : op)
+        : list op * op * list op * op + error :=
+        let len_lbinds := length lbinds in
+        let len_rbinds := length fwd_rbinds in
+        _ <-! if expr_omits_rangeb len_lbinds (ptail, prog_end)
+              then ok tt
+              else raise (E_msg "replace_lemma: lbinds not omitted in tail");
+          match Decompose.prefix op_eqb (lhead :: lbinds) (phead :: pbinds) with
+          | Some rest =>
+            let f := shift len_lbinds len_rbinds in
+            ok (rev_append fwd_rbinds rest,
+                rhead,
+                renumber_bindings (offset_renumbering 1 f) ptail,
+                renumber_op (offset_renumbering (S (length ptail)) f)
+                            prog_end)
+          | None =>
+            raise (E_msg "replace_lemma: match failed")
+          end.
+
+      Lemma replace_lemma_correct lbinds fwd_rbinds lhead rhead
+            pbinds phead ptail prog_end :
+        op_type lhead = op_type rhead ->
+        equiv (rev lbinds, lhead) (fwd_rbinds, rhead) ->
+        match replace_lemma lbinds fwd_rbinds lhead rhead
+                            pbinds phead ptail prog_end with
+        | ok (new_pbinds, new_phead, new_ptail, new_prog_end) =>
+          equiv (assemble pbinds phead ptail prog_end)
+                (assemble new_pbinds new_phead new_ptail new_prog_end)
+        | raise _ => True
+        end.
+      Proof.
+        intros L ?.
+        remember (replace_lemma lbinds fwd_rbinds lhead rhead
+                                pbinds phead ptail prog_end) as err;
+          destruct err as
+            [[[[new_pbinds' new_phead'] new_ptail'] new_prog_end']|];
+          eauto.
+        cbv [replace_lemma] in *.
+        pose proof (Decompose.prefix_correct op_eqb op_eqb_eq
+                                             (lhead :: lbinds)
+                                             (phead :: pbinds));
+          destruct (Decompose.prefix op_eqb
+                                     (lhead :: lbinds)
+                                     (phead :: pbinds)) as [rest|];
+          repeat step_err_bind.
+        listrew.
+        match goal with
+        | H : _ :: _ = _ :: _ |- _ => inversion H; clear H
+        end.
+        subst new_pbinds' new_phead' new_ptail' new_prog_end' pbinds phead.
+        cbv [assemble]; listrew.
+
+        eapply equiv_prefix.
+        remember (rev lbinds) as fwd_lbinds.
+        eapply (f_equal (@rev _)) in Heqfwd_lbinds; listrew.
+        subst lbinds; listrew.
+        eapply equiv_suffix; eauto.
+        - pose proof (expr_omits_rangeb_correct (length fwd_lbinds)
+                                                (ptail, prog_end));
+            destruct (expr_omits_rangeb (length fwd_lbinds) (ptail, prog_end));
+            eauto; congruence.
+        - rewrite renumber_expr_renumber_bindings.
+          f_equal.
+          eapply renumber_op_ext.
+          intros.
+          rewrite <-offset_renumbering_plus.
+          f_equal.
+          omega.
+      Qed.
+    End WithMap.
+  End Rewriter.
+
+  Section WithUnused.
+    Context {Mbind_unused :
+               forall {t1 t2} (a : M t1) (b : M t2),
+                 Mequiv (Mbind a (fun _ => b)) b}.
+    Arguments Mbind_unused {t1 t2}.
+
+    Lemma interp_expr_cast_different ctxt ctx e t :
+      t <> expr_type e ->
+      Mequiv (interp_expr_cast ctxt ctx e t)
+             (Mret interp_type_inhabited).
+    Proof.
+      intros; cbv [interp_expr_cast].
+      setoid_rewrite <-(Mbind_unused (interp_expr ctxt ctx e)
+                                     (Mret interp_type_inhabited)).
+      step_Mequiv.
+      rewrite cast_different by eauto; reflexivity.
+    Qed.
+
+    Lemma equiv_under_same_type ctxt ctx e1 e2 :
+      expr_type e1 = expr_type e2 ->
+      Mequiv (interp_expr ctxt ctx e1)
+             (interp_expr_cast ctxt ctx e2 _) ->
+      equiv_under ctxt ctx e1 e2.
+    Proof.
+      setoid_rewrite <-interp_expr_cast_expr_type.
+      cbv [equiv_under].
+      intros.
+      destruct (type_eq_or t (expr_type e1)).
+      - subst; eauto.
+      - setoid_rewrite interp_expr_cast_different; try congruence.
+        reflexivity.
+    Qed.
+  End WithUnused.
+End Language.
+
+Section LanguageImpl.
+  Inductive basetype : Set :=
+  | tnat : basetype
+  | tbool : basetype.
+
+  Definition basetype_eqb (t1 t2 : basetype) : bool :=
+    match t1, t2 with
+    | tnat, tnat => true
+    | tbool, tbool => true
+    | _, _ => false
+    end.
+  Lemma basetype_eqb_eq t1 t2 : basetype_eqb t1 t2 = true <-> t1 = t2.
+  Proof. destruct t1, t2; cbn [basetype_eqb]; intuition congruence. Qed.
+  Instance basetype_eqdec : EqDec basetype :=
+    Build_EqDec basetype_eqb basetype_eqb_eq.
+
+  Definition interp_basetype (b : basetype) : Set :=
+    match b with
+    | tnat => nat
+    | tbool => bool
+    end.
+  Definition interp_basetype_eqb {b} (x y : interp_basetype b)
+    : bool :=
+    match b return interp_basetype b -> interp_basetype b -> bool with
+    | tnat
+    | tbool => fun x y => x ?= y
+    end x y.
+  Lemma interp_basetype_eqb_eq {b} (x y : interp_basetype b) :
+    interp_basetype_eqb x y = true <-> x = y.
+  Proof. destruct b; cbn [interp_basetype_eqb]; crush_deciders idtac. Qed.
+  Instance interp_basetype_eqdec {b} : EqDec (interp_basetype b) :=
+    Build_EqDec interp_basetype_eqb interp_basetype_eqb_eq.
+
+  Definition interp_basetype_inhabited {b} : interp_basetype b :=
+    match b with
+    | tnat => 0
+    | tbool => false
+    end.
+
+  Definition basetype_transport {P : basetype -> Type} {b1} b2 :
+    P b1 -> option (P b2) :=
+    match b1, b2 with
+    | tnat, tnat
+    | tbool, tbool => Some
+    | _, _ => fun _ => None
+    end.
+  Lemma basetype_transport_same {P b} (p : P b) :
+    basetype_transport b p = Some p.
+  Proof. destruct b; cbn [basetype_transport]; congruence. Qed.
+  Lemma basetype_transport_different {P b1 b2} (p : P b1) :
+    b2 <> b1 -> (@basetype_transport _ b1 b2 p) = None.
+  Proof. destruct b1, b2; cbn [basetype_transport]; congruence. Qed.
+
+  Notation type := (@type basetype).
+  Notation interp_type := (@interp_type basetype interp_basetype).
+
+  Definition M t := Comp (interp_type t).
+  Definition Mret {t : type} : interp_type t -> M t :=
+    Ret (EqDec_dec interp_type_eqdec).
+  Definition Mbind {t1 t2 : type} :
+    M t1 ->
+    (interp_type t1 -> M t2) -> M t2 :=
+    @Bind _ _.
+  Definition Mequiv {t} : M t -> M t -> Prop := Comp_eq.
+
+  Inductive const : Type :=
+  | coin.
+  Definition const_eqb (c1 c2 : const) : bool :=
+    match c1, c2 with
+    | coin, coin => true
+    end.
+  Lemma const_eqb_eq (c1 c2 : const) : const_eqb c1 c2 = true <-> c1 = c2.
+  Proof. destruct c1, c2; intuition eauto. Qed.
+  Instance const_eqdec : EqDec const := Build_EqDec const_eqb const_eqb_eq.
+
+  Definition cdom c : type :=
+    match c with
+    | coin => tunit
+    end.
+
+  Definition ccod c : type :=
+    match c with
+    | coin => tbase tbool
+    end.
+
+  Definition interp_const c : interp_type (cdom c) -> M (ccod c) :=
+    match c with
+    | coin => fun _ => x <-$ Rnd 1; ret (Vector.nth x Fin.F1)
+    end.
+
+  Inductive retconst : Type :=
+  | xor'
+  | zero
+  | id (t : type).
+
+  Definition retconst_eqb (c c' : retconst) : bool :=
+    match c, c' with
+    | xor', xor' => true
+    | zero, zero => true
+    | id t1, id t2 => type_eqb t1 t2
+    | _, _ => false
+    end.
+  Lemma retconst_eqb_eq c1 c2 : retconst_eqb c1 c2 = true <-> c1 = c2.
+  Proof.
+    destruct c1, c2; cbv [retconst_eqb]; rewrite ?type_eqb_eq;
+      intuition congruence.
+  Qed.
+  Instance retconst_eqdec : EqDec retconst :=
+    Build_EqDec retconst_eqb retconst_eqb_eq.
+
+  Definition rcdom c : type :=
+    match c with
+    | xor' => tprod (tbase tbool) (tbase tbool)
+    | zero => tunit
+    | id t => t
+    end.
+
+  Definition rccod c : type :=
+    match c with
+    | xor' => tbase tbool
+    | zero => tbase tbool
+    | id t => t
+    end.
+
+  Definition interp_retconst c :
+    interp_type (rcdom c) -> interp_type (rccod c) :=
+    match c with
+    | xor' => fun '(x, y) => xorb x y
+    | zero => fun _ => false
+    | id _ => fun x => x
+    end.
+
+  Lemma Proper_Mbind {t1 t2} :
+    Proper
+      (Mequiv ==> (pointwise_relation _ Mequiv) ==> Mequiv)
+      (@Mbind t1 t2).
+  Proof. eapply Proper_Bind. Qed.
+
+  Lemma Mbind_assoc {t1 t2 t3} (f : M t1)
+        (g : interp_type t1 -> M t2) (h : interp_type t2 -> M t3) :
+    Mequiv (Mbind (Mbind f g) h)
+           (Mbind f (fun x => Mbind (g x) h)).
+  Proof. symmetry; eapply Bind_assoc. Qed.
+
+  Lemma Mbind_comm (t1 t2 t3 : type) (c1 : M t1) (c2 : M t2)
+        (c3 : interp_type t1 -> interp_type t2 -> M t3) :
+    Mequiv (Mbind c1 (fun a => Mbind c2 (fun b => c3 a b)))
+           (Mbind c2 (fun b => Mbind c1 (fun a => c3 a b))).
+  Proof. eapply Bind_comm. Qed.
+
+  Lemma Mbind_Mret_l {t1 t2} x (f : interp_type t1 -> M t2) :
+    Mequiv (Mbind (Mret x) f) (f x).
+  Proof. eapply Bind_Ret_l. Qed.
+
+  Lemma Mbind_Mret_r {t} (x : M t) : Mequiv (Mbind x Mret) x.
+  Proof. eapply Bind_Ret_r. Qed.
+
+  Instance Mequiv_equiv {t} : Equivalence (@Mequiv t).
+  Proof. typeclasses eauto. Qed.
+
+  (** Reification *)
+  Ltac reify_type t :=
+    lazymatch t with
+    | prod ?ta ?tb =>
+      let ta := reify_type ta in
+      let tb := reify_type tb in
+      uconstr:(tprod ta tb)
+    | bool => uconstr:(tbase tbool)
+    | unit => uconstr:(tbase tunit)
+    | interp_type ?t => t
+    | _ => fail "UNKNOWN TYPE" t
+    end.
+
+  Ltac pindexof x ctx :=
+    lazymatch ctx with
+    | (x, _) => uconstr:(O)
+    | (_, ?ctx) =>
+      let i := pindexof x ctx in
+      uconstr:(S i)
+    | _ => fail "NOT FOUND" x
+    end.
+
+  Ltac reify_ref ctx r :=
+    lazymatch r with
+    | pair ?a ?b =>
+      let a := reify_ref ctx a in
+      let b := reify_ref ctx b in
+      uconstr:(ref_pair a b)
+    | ?x =>
+      let r := pindexof r ctx in
+      uconstr:(ref_index r)
+    end.
+
+  Ltac reify_op ctx o :=
+    lazymatch o with
+    | ret tt => uconstr:(op_unit)
+    | interp_const coin ?a =>
+      let a := pindexof a ctx in
+      uconstr:(op_app coin (ref_index a))
+    | ret xorb ?a ?b =>
+      let a := pindexof a ctx in
+      let b := pindexof b ctx in
+      uconstr:(op_retapp xor' (ref_pair (ref_index a) (ref_index b)))
+    | ret ?x =>
+      let t := lazymatch type of x with ?T => reify_type T end in
+      let x := reify_ref ctx x in
+      uconstr:(op_retapp (id t) x)
+    | ?O => fail "UNKNOWN OP" O
+    end.
+
+  Ltac reify_to_list ctx e :=
+    lazymatch e with
+    | (x <-$ ?o; ?f) =>
+      let T := lazymatch type of o with
+               | Comp ?T => T
+               | M ?T => constr:(interp_type T)
+               | ?X => fail "XX" X
+               end in
+      let o := reify_op ctx o in
+      let _y := fresh in let y := fresh in (* andres thinks this might work around a coq bug but does not remember which one :( *)
+      lazymatch constr:(fun (y:T) => ltac:(
+          let r := reify_to_list
+            constr:(pair y ctx)
+            constr:(match y return _ with x => f end) in
+          exact r
+       )) with
+      | fun _ => ?r => uconstr:(@cons op o r)
+      | _ => fail "FUNDEP"
+      end
+    | ?o =>
+      let o := reify_op ctx o in
+      uconstr:(@cons op o (@nil op))
+    | ?O => fail "UNKNOWN EXPR" O
+    end.
+
+  Ltac reify e :=
+    let e := reify_to_list tt e in
+    let e := eval cbv in (List.removelast e, List.last e op_unit) in
+        constr:(e).
+
+  Section ExampleCoins.
+    Import CrossCrypto.fmap.list_of_pairs.
+    Local Notation map := (list_of_pairs Nat.eqb).
+
+    Notation expr := (@expr const retconst).
+
+    Definition example_coin_lemma_lhs : expr :=
+      (op_unit
+         :: op_unit
+         :: (op_app coin (ref_index 1))
+         :: (op_app coin (ref_index 1))
+         :: nil,
+       op_retapp xor' (ref_pair (ref_index 0) (ref_index 1))).
+
+    Definition example_coin_lemma_rhs : expr :=
+      ((op_unit :: nil), op_app coin (ref_index 0)).
+
+    Lemma Mbind_unused {t1 t2} (a : M t1) (b : M t2) :
+      Mequiv (Mbind a (fun _ => b)) b.
+    Proof. eapply Bind_unused. Qed.
+
+    Notation equiv :=
+      (@equiv basetype interp_basetype (@interp_basetype_inhabited)
+              (@basetype_transport)
+              M (@Mret) (@Mbind) (@Mequiv)
+              const cdom ccod interp_const retconst
+              rcdom rccod interp_retconst).
+
+    Notation equiv_under_same_type :=
+      (@equiv_under_same_type
+         basetype basetype_eqdec interp_basetype (@interp_basetype_inhabited)
+         (@basetype_transport) (@basetype_transport_same)
+         (@basetype_transport_different) M (@Mret) (@Mbind) (@Mequiv)
+         (@Mequiv_equiv) (@Proper_Mbind) (@Mbind_Mret_r)
+         const cdom ccod interp_const
+         retconst rcdom rccod interp_retconst
+         (@Mbind_unused)).
+
+    Lemma example_coin_lemma :
+      equiv example_coin_lemma_lhs example_coin_lemma_rhs.
+    Proof.
+      intros ??.
+      eapply equiv_under_same_type; eauto.
+      cbv -[Comp_eq
+              interp_const interp_retconst
+              interp_type_eqdec interp_basetype_eqdec];
+        cbn [interp_const interp_retconst].
+
+      (* anomalies if we accidentally unfold interp_basetype_eqdec *)
+      repeat (setoid_rewrite Bind_Ret_l || setoid_rewrite <-Bind_assoc).
+      cbv [Comp_eq image_relation pointwise_relation evalDist getSupport
+                   getAllBvectors].
+      cbn [List.map app sumList fold_left
+                    Vector.nth xorb Vector.caseS
+                    expnat Nat.mul Nat.add].
+      intros a.
+      repeat lazymatch goal with
+             | |- context[(@EqDec_dec bool ?x)] =>
+               let d := fresh in
+               pose (EqDec_dec x) as d;
+                 change (EqDec_dec x) with d;
+                 destruct (d true a), (d false a)
+             end;
+        try congruence; reflexivity.
+    Qed.
+
+    Notation commute_matches_correct :=
+      (@commute_matches_correct
+         basetype interp_basetype (@interp_basetype_inhabited)
+         (@basetype_transport)
+         M (@Mret) (@Mbind) (@Mequiv) (@Mequiv_equiv)
+         (@Proper_Mbind) (@Mbind_assoc) (@Mbind_comm)
+         const const_eqdec cdom ccod interp_const
+         retconst retconst_eqdec rcdom rccod interp_retconst
+         map).
+
+    Notation replace_lemma_correct :=
+      (@replace_lemma_correct
+         basetype interp_basetype (@interp_basetype_inhabited)
+         (@basetype_transport) (@basetype_transport_same)
+         M (@Mret) (@Mbind) (@Mequiv) (@Mequiv_equiv)
+         (@Proper_Mbind) (@Mbind_assoc) (@Mbind_Mret_r)
+         const const_eqdec cdom ccod interp_const
+         retconst retconst_eqdec rcdom rccod interp_retconst).
+
+    Existing Instance equiv_equiv.
+
+    Definition coins_example : expr :=
+      (op_unit :: op_app coin (ref_index 0)
+               :: op_unit :: op_app coin (ref_index 0)
+               :: op_unit :: op_app coin (ref_index 0)
+               :: op_retapp xor' (ref_pair (ref_index 4) (ref_index 0))
+               :: nil,
+       op_retapp
+         (id (tprod (tprod (tbase tbool) (tbase tbool)) (tbase tbool)))
+         (ref_pair (ref_pair (ref_index 0) (ref_index 3)) (ref_index 3))).
+    Derive coins_endpoint
+           SuchThat (equiv coins_example coins_endpoint)
+           As coins_example_rewrite.
+    Proof.
+      set (lbinds := rev (fst example_coin_lemma_lhs)).
+      set (lhead := snd example_coin_lemma_lhs).
+      pose proof (commute_matches_correct lbinds lhead coins_example) as HC.
+      set (C := commute_matches _ _ _ _) in HC; cbv in C.
+      cbv [C assemble] in HC.
+      eapply Forall_inv in HC.
+      cbv [rev_append] in HC.
+      setoid_rewrite HC; clear HC.
+
+      set (fwd_rbinds := fst example_coin_lemma_rhs).
+      set (rhead := snd example_coin_lemma_rhs).
+
+      pose proof (replace_lemma_correct
+                    lbinds fwd_rbinds lhead rhead
+                    (op_app coin (ref_index 1)
+                            :: op_app coin (ref_index 1)
+                            :: op_unit :: op_unit
+                            :: op_app coin (ref_index 0) :: op_unit :: nil)
+                    (op_retapp xor' (ref_pair (ref_index 0) (ref_index 1)))
+                    nil
+                    (op_retapp (id (tprod (tprod (tbase tbool) (tbase tbool))
+                                          (tbase tbool)))
+                               (ref_pair (ref_pair (ref_index 0)
+                                                   (ref_index 5))
+                                         (ref_index 5)))
+                    eq_refl
+                    example_coin_lemma) as HR.
+      set (R := replace_lemma _ _ _ _ _ _ _ _) in HR; cbv in R.
+      cbv [R assemble rev_append] in HR.
+      setoid_rewrite HR; clear HR.
+      subst coins_endpoint; reflexivity.
+    Qed.
+    Print coins_endpoint.
+
+    (*
+  Eval cbv [interp_expr coins_example interp_bindings Mbind Mret interp_op_silent interp_op lookup_ref lookup transport type_eq_or type_rec type_rect op_type cdom eq_rect_r eq_rect eq_sym rcdom ccod rccod interp_retconst] in
+      interp_expr tunit tt coins_example.
+     *)
+
+    (* reification not yet ported because of modularity issues *)
+
+    (* Definition coins_example' := *)
+    (*   x <-$ ret tt; *)
+    (*     x0 <-$ interp_const coin x; *)
+    (*     x1 <-$ ret tt; *)
+    (*     x2 <-$ interp_const coin x1; *)
+    (*     x3 <-$ ret tt; *)
+    (*     x4 <-$ interp_const coin x3; *)
+    (*     x5 <-$ ret xorb x0 x4; *)
+    (*     ret (x5, x2, x2). *)
+    (* Derive reified_coins_example *)
+    (*        SuchThat (reified_coins_example = coins_example') *)
+    (*        As reified_coins_example'_correct. *)
+    (* Proof. *)
+    (*   cbv [coins_example']. *)
+
+    (*   let x := reified_coins_example in *)
+    (*   let x := eval unfold x in x in *)
+    (*       let e := match goal with |- ?LHS = ?RHS => RHS end in *)
+    (*       let e := reify e in *)
+    (*       unify x (interp_expr tunit tt e). *)
+
+    (*   reflexivity. *)
+    (* Qed. *)
+    (* Print reified_coins_example. *)
+  End ExampleCoins.
+End LanguageImpl.
