src/NatUtil.v
@@ -1,0 +1,24 @@
+Require Import Omega.
+
+Fixpoint optsub (n m : nat) {struct m} : option nat :=
+  match m with
+  | 0 => Some n
+  | S m => match n with
+           | 0 => None
+           | S n => optsub n m
+           end
+  end.
+
+Notation "a -? b" := (optsub a b) (left associativity, at level 50).
+
+Lemma optsub_plus a b :
+  match a -? b with
+  | Some c => a = b + c
+  | None => a < b
+  end.
+Proof.
+  revert a; induction b; intros a; cbn [optsub plus]; eauto.
+  destruct a; try omega.
+  specialize (IHb a).
+  destruct (a -? b); omega.
+Qed.
